@prefix : <http://www.americanartcollaborative.org/ontology/aac-ont.owl#> .
@prefix DOLCE-Lite: <http://www.loa-cnr.it/ontologies/DOLCE-Lite.owl#> .
@prefix ElementsGr2: <http://rdvocab.info/ElementsGr2/> .
@prefix aac-ont: <http://www.americanartcollaborative.org/ontology/> .
@prefix abc: <http://metadata.net/harmony/abc#> .
@prefix crm: <http://www.cidoc-crm.org/rdfs/cidoc-crm#> .
@prefix dc: <http://purl.org/dc/elements/1.1/> .
@prefix dcam: <http://purl.org/dc/dcam/> .
@prefix dcmitype: <http://purl.org/dc/dcmitype/> .
@prefix dct: <http://purl.org/dc/terms/> .
@prefix edm: <http://www.europeana.eu/schemas/edm/> .
@prefix foaf: <http://xmlns.com/foaf/0.1/> .
@prefix frbr: <http://rdvocab.info/uri/schema/FRBRentitiesRDA/> .
@prefix frbr_core: <http://purl.org/vocab/frbr/core#> .
@prefix gn: <http://www.geonames.org/ontology#> .
@prefix msg0: <http://web.resource.org/cc/> .
@prefix ore: <http://www.openarchives.org/ore/terms/> .
@prefix owl: <http://www.w3.org/2002/07/owl#> .
@prefix owl2xml: <http://www.w3.org/2006/12/owl2-xml#> .
@prefix rdf: <http://www.w3.org/1999/02/22-rdf-syntax-ns#> .
@prefix rdfg: <http://www.w3.org/2004/03/trix/rdfg-1/> .
@prefix rdfs: <http://www.w3.org/2000/01/rdf-schema#> .
@prefix reg: <http://metadataregistry.org/uri/profile/RegAp/> .
@prefix saam-ont: <http://americanart.si.edu/ontology/> .
@prefix schema: <http://schema.org/> .
@prefix skos: <http://www.w3.org/2008/05/skos#> .
@prefix status: <http://metadataregistry.org/uri/RegStatus/> .
@prefix vann: <http://purl.org/vocab/vann/> .
@prefix vs: <http://www.w3.org/2003/06/sw-vocab-status/ns#> .
@prefix wgs84_pos: <http://www.w3.org/2003/01/geo/wgs84_pos#> .
@prefix wot: <http://xmlns.com/wot/0.1/> .
@prefix xsd: <http://www.w3.org/2001/XMLSchema#> .

rdf:type a owl:AnnotationProperty, owl:ObjectProperty .

rdf:Property a owl:Class .

rdfs:Class a rdfs:Class, owl:Class .

rdfs:Resource a rdfs:Class, owl:Class .

rdf:subject a owl:AnnotationProperty, owl:ObjectProperty .

rdf:predicate a owl:AnnotationProperty, owl:ObjectProperty .

rdf:object a owl:AnnotationProperty, owl:ObjectProperty .

rdf:first a owl:AnnotationProperty, owl:ObjectProperty .

rdf:rest a owl:AnnotationProperty, owl:ObjectProperty .

rdf:value a owl:AnnotationProperty, owl:DatatypeProperty, owl:ObjectProperty .

rdf:List a owl:Class .

rdf:Statement a owl:Class .

rdfs:comment a rdf:Property .

rdfs:Literal a rdfs:Class, owl:Class .

rdfs:label a rdf:Property .

rdf:Alt a owl:Class .

rdfs:Container a rdfs:Class, owl:Class .

rdf:Bag a owl:Class .

rdf:Seq a owl:Class .

rdfs:ContainerMembershipProperty a rdfs:Class .

rdfs:isDefinedBy a rdf:Property .

rdfs:seeAlso a rdf:Property .

rdf:XMLLiteral a owl:Class .

rdfs:Datatype a rdfs:Class .

aac-ont:aac-ont.owl a owl:Ontology .

dct:creator a owl:AnnotationProperty, owl:ObjectProperty .

edm:Agent a owl:Class .

aac-ont:creatorOf a owl:ObjectProperty .

ElementsGr2:placeOfBirth a rdf:Property, owl:ObjectProperty .

aac-ont:Person a owl:Class .

aac-ont:Place a owl:Class .

aac-ont:associatedPlace a owl:ObjectProperty .

ElementsGr2:placeOfDeath a rdf:Property, owl:ObjectProperty .

aac-ont:sitter a owl:ObjectProperty .

aac-ont:CulturalHeritageObject a owl:Class .

edm:ProvidedCHO a owl:Class .

aac-ont:objectId a owl:DatatypeProperty .

aac-ont:accessionNumber a owl:DatatypeProperty .

frbr:Person a owl:Class .

schema:Place a owl:Class .

skos:Concept a owl:Class, owl:NamedIndividual .

aac-ont:Organization a owl:Class .

foaf:Person a rdfs:Class, owl:Class .

edm:Place a owl:Class .

<http://www.w3.org/2008/05/skos> a owl:Ontology .

dc:creator a owl:ObjectProperty .

dc:description a owl:AnnotationProperty .

dc:contributor a owl:DatatypeProperty, owl:ObjectProperty .

dc:title a owl:AnnotationProperty, owl:DatatypeProperty .

skos:altLabel a owl:AnnotationProperty, owl:DatatypeProperty, owl:NamedIndividual .

dct:issued a owl:AnnotationProperty .

skos:definition a owl:AnnotationProperty, owl:NamedIndividual, owl:ObjectProperty .

skos:hiddenLabel a owl:AnnotationProperty, owl:DatatypeProperty, owl:NamedIndividual .

skos:prefLabel a owl:AnnotationProperty, owl:DatatypeProperty, owl:NamedIndividual .

skos:broadMatch a owl:NamedIndividual, owl:ObjectProperty .

skos:broader a owl:NamedIndividual, owl:ObjectProperty .

skos:mappingRelation a owl:NamedIndividual, owl:ObjectProperty .

skos:broaderTransitive a owl:NamedIndividual, owl:ObjectProperty, owl:TransitiveProperty .

skos:narrower a owl:NamedIndividual, owl:ObjectProperty .

skos:narrowerTransitive a owl:NamedIndividual, owl:ObjectProperty, owl:TransitiveProperty .

skos:semanticRelation a owl:NamedIndividual, owl:ObjectProperty .

skos:changeNote a owl:NamedIndividual, owl:ObjectProperty .

skos:note a owl:AnnotationProperty, owl:NamedIndividual, owl:ObjectProperty .

skos:closeMatch a owl:NamedIndividual, owl:ObjectProperty, owl:SymmetricProperty .

skos:editorialNote a owl:NamedIndividual, owl:ObjectProperty .

skos:exactMatch a owl:NamedIndividual, owl:ObjectProperty, owl:SymmetricProperty,
    owl:TransitiveProperty .

skos:example a owl:AnnotationProperty, owl:NamedIndividual, owl:ObjectProperty .

skos:hasTopConcept a owl:NamedIndividual, owl:ObjectProperty .

skos:ConceptScheme a owl:Class, owl:NamedIndividual .

skos:historyNote a owl:NamedIndividual, owl:ObjectProperty .

skos:inScheme a owl:NamedIndividual, owl:ObjectProperty .

skos:member a owl:NamedIndividual, owl:ObjectProperty .

skos:Collection a owl:Class, owl:NamedIndividual .

skos:memberList a owl:FunctionalProperty, owl:NamedIndividual, owl:ObjectProperty .

skos:OrderedCollection a owl:Class, owl:NamedIndividual .

skos:narrowMatch a owl:NamedIndividual, owl:ObjectProperty .

skos:related a owl:NamedIndividual, owl:ObjectProperty, owl:SymmetricProperty .

skos:relatedMatch a owl:NamedIndividual, owl:ObjectProperty, owl:SymmetricProperty .

skos:scopeNote a owl:AnnotationProperty, owl:NamedIndividual, owl:ObjectProperty .

skos:topConceptOf a owl:NamedIndividual, owl:ObjectProperty .

skos:notation a owl:DatatypeProperty, owl:NamedIndividual .

<http://americanart.si.edu/ontology/> a <http://americanart.si.edu/ontology/>, owl:Class,
    owl:NamedIndividual, owl:Ontology .

dct:modified a owl:AnnotationProperty .

dct:title a owl:AnnotationProperty .

dct:description a owl:AnnotationProperty .

saam-ont:seeAlsoInSmithsonianAmericanArt a owl:AnnotationProperty .

saam-ont:seeAlsoWikipedia a owl:AnnotationProperty, owl:ObjectProperty .

saam-ont:constituentId a owl:AnnotationProperty, owl:DatatypeProperty .

saam-ont:objectId a owl:AnnotationProperty, owl:DatatypeProperty .

saam-ont:seeAlsoNytimes a owl:AnnotationProperty, owl:ObjectProperty .

saam-ont:seeAlsoSmithsonianAmericanArt a owl:ObjectProperty .

dc:identifier a owl:DatatypeProperty .

<http://www.europeana.eu/schemas/edm/> a owl:Ontology .

edm:year a owl:AnnotationProperty .

dct:temporal a owl:AnnotationProperty .

edm:dataProvider a owl:AnnotationProperty, owl:ObjectProperty .

dct:provenance a owl:AnnotationProperty .

ore:Aggregation a rdfs:Class, owl:Class .

crm:P12F.occurred_in_the_presence_of a owl:AnnotationProperty .

edm:country a owl:AnnotationProperty .

edm:userTag a owl:AnnotationProperty .

edm:hasMet a owl:ObjectProperty .

dc:coverage a owl:ObjectProperty .

dc:date a owl:AnnotationProperty, owl:DatatypeProperty, owl:ObjectProperty .

dc:format a owl:ObjectProperty .

edm:hasType a owl:ObjectProperty .

dc:language a owl:ObjectProperty .

dc:publisher a owl:ObjectProperty .

dc:relation a owl:ObjectProperty .

edm:isRelatedTo a owl:ObjectProperty .

dc:source a owl:ObjectProperty .

edm:isDerivativeOf a owl:ObjectProperty .

dc:subject a owl:ObjectProperty .

dc:type a owl:AnnotationProperty, owl:ObjectProperty .

dct:hasFormat a owl:AnnotationProperty, owl:ObjectProperty .

dct:hasVersion a owl:AnnotationProperty, owl:ObjectProperty .

dct:isFormatOf a owl:AnnotationProperty, owl:ObjectProperty .

dct:isReplacedBy a owl:AnnotationProperty, owl:ObjectProperty .

dct:isVersionOf a owl:AnnotationProperty, owl:ObjectProperty .

dct:replaces a owl:AnnotationProperty, owl:ObjectProperty .

dct:spatial a owl:AnnotationProperty, owl:ObjectProperty .

dct:tableOfContents a owl:AnnotationProperty, owl:ObjectProperty .

edm:hasView a owl:ObjectProperty .

crm:P129F.is_about a owl:ObjectProperty .

crm:P138F.represents a owl:ObjectProperty .

crm:P67F.refers_to a owl:ObjectProperty .

edm:aggregatedCHO a owl:ObjectProperty .

ore:aggregates a rdf:Property, owl:ObjectProperty .

edm:currentLocation a owl:ObjectProperty .

ore:Proxy a rdfs:Class, owl:Class .

ore:proxyFor a rdf:Property, owl:ObjectProperty .

edm:happenedAt a owl:ObjectProperty .

edm:Event a owl:Class .

edm:NonInformationResource a owl:Class .

edm:WebResource a owl:Class .

edm:incorporates a owl:ObjectProperty .

edm:isSimilarTo a owl:ObjectProperty .

edm:isAnnotationOf a owl:ObjectProperty .

edm:EuropeanaObject a owl:Class .

edm:isNextInSequence a owl:ObjectProperty .

edm:isRepresentationOf a owl:ObjectProperty .

edm:InformationResource a owl:Class .

edm:isShownAt a owl:ObjectProperty .

edm:landingPage a owl:ObjectProperty .

edm:isShownBy a owl:ObjectProperty .

edm:isSuccessorOf a owl:ObjectProperty .

edm:object a owl:ObjectProperty .

edm:occurredAt a owl:ObjectProperty .

edm:TimeSpan a owl:Class .

edm:provider a owl:ObjectProperty .

edm:realizes a owl:ObjectProperty .

edm:PhysicalThing a owl:Class .

edm:rights a owl:ObjectProperty .

edm:uri a owl:ObjectProperty .

edm:wasPresentAt a owl:ObjectProperty .

edm:type a owl:DatatypeProperty .

edm:ugc a owl:DatatypeProperty .

abc:Place a owl:Class .

abc:Temporality a owl:Class .

abc:Time a owl:Class .

dct:PeriodOfTime a owl:Class .

frbr_core:Event a owl:Class .

frbr_core:Expression a owl:Class .

frbr_core:Manifestation a owl:Class .

frbr_core:Place a owl:Class .

frbr_core:Work a owl:Class .

crm:E18.Physical_Thing a owl:Class .

crm:E39.Actor a owl:Class .

crm:E4.Period a owl:Class .

crm:E52.Time-Span a owl:Class .

crm:E53.Place a owl:Class .

crm:E89.Propositional_Object a owl:Class .

edm:EuropeanaAggregation a owl:Class .

DOLCE-Lite:space-region a owl:Class .

DOLCE-Lite:time-interval a owl:Class .

dct:publisher a owl:AnnotationProperty .

ore:AggregatedResource a rdfs:Class .

ore:ResourceMap a rdfs:Class .

dct:hasPart a owl:AnnotationProperty .

ore:isAggregatedBy a rdf:Property .

dct:isPartOf a owl:AnnotationProperty .

ore:describes a rdf:Property .

ore:isDescribedBy a rdf:Property .

ore:lineage a rdf:Property .

ore:proxyIn a rdf:Property .

ore:similarTo a rdf:Property .

ElementsGr2:addressOfTheCorporateBody a rdf:Property .

status:1002 a skos:Concept .

ElementsGr2:addressOfThePerson a rdf:Property .

ElementsGr2:affiliation a rdf:Property .

ElementsGr2:associatedInstitution a rdf:Property .

ElementsGr2:biographicalInformation a rdf:Property .

ElementsGr2:corporateHistory a rdf:Property .

ElementsGr2:countryAssociatedWithThePerson a rdf:Property .

ElementsGr2:dateAssociatedWithTheCorporateBody a rdf:Property .

ElementsGr2:dateOfEstablishment a rdf:Property .

ElementsGr2:dateOfConferenceEtc a rdf:Property .

ElementsGr2:dateOfTermination a rdf:Property .

ElementsGr2:dateAssociatedWithTheFamily a rdf:Property .

ElementsGr2:dateAssociatedWithThePerson a rdf:Property .

ElementsGr2:dateOfBirth a rdf:Property .

ElementsGr2:dateOfDeath a rdf:Property .

ElementsGr2:periodOfActivityOfThePerson a rdf:Property .

ElementsGr2:dateOfUsage a rdf:Property .

ElementsGr2:familyHistory a rdf:Property .

ElementsGr2:fieldOfActivityOfTheCorporateBody a rdf:Property .

ElementsGr2:fieldOfActivityOfThePerson a rdf:Property .

ElementsGr2:fullerFormOfName a rdf:Property .

ElementsGr2:fullerFormOfNamePerson a rdf:Property .

ElementsGr2:gender a rdf:Property .

ElementsGr2:hereditaryTitle a rdf:Property .

ElementsGr2:identifierForTheCorporateBody a rdf:Property .

ElementsGr2:identifierForTheFamily a rdf:Property .

ElementsGr2:identifierForThePerson a rdf:Property .

ElementsGr2:languageOfTheCorporateBody a rdf:Property .

ElementsGr2:languageOfThePerson a rdf:Property .

ElementsGr2:locationOfConferenceEtc a rdf:Property .

ElementsGr2:placeAssociatedWithTheCorporateBody a rdf:Property .

ElementsGr2:locationOfHeadquarters a rdf:Property .

ElementsGr2:name a rdf:Property .

ElementsGr2:nameOfTheCorporateBody a rdf:Property .

ElementsGr2:preferredNameForTheCorporateBody a rdf:Property .

ElementsGr2:variantNameForTheCorporateBody a rdf:Property .

ElementsGr2:nameOfTheFamily a rdf:Property .

ElementsGr2:preferredNameForTheFamily a rdf:Property .

ElementsGr2:variantNameForTheFamily a rdf:Property .

ElementsGr2:nameOfThePerson a rdf:Property .

ElementsGr2:preferredNameForThePerson a rdf:Property .

ElementsGr2:variantNameForThePerson a rdf:Property .

ElementsGr2:note a rdf:Property .

ElementsGr2:numberOfAConferenceEtc a rdf:Property .

ElementsGr2:otherDesignationAssociatedWithTheCorporateBody a rdf:Property .

ElementsGr2:otherDesignationAssociatedWithThePerson a rdf:Property .

ElementsGr2:placeAssociatedWithTheFamily a rdf:Property .

ElementsGr2:placeOfResidence a rdf:Property .

ElementsGr2:professionOrOccupation a rdf:Property .

ElementsGr2:prominentMemberOfTheFamily a rdf:Property .

ElementsGr2:scopeOfUsage a rdf:Property .

ElementsGr2:titleOfThePerson a rdf:Property .

ElementsGr2:typeOfFamily a rdf:Property .

ElementsGr2:undifferentiatedNameIndicator a rdf:Property .

ElementsGr2:undifferentiatedNameIndicatorPerson a rdf:Property .

ElementsGr2:undifferentiatedNameIndicatorCorporateBody a rdf:Property .

ElementsGr2:undifferentiatedNameIndicatorFamily a rdf:Property .

<http://vocab.org/frbr/core.rdf> a dcmitype:Text, foaf:Document .

foaf:Document a rdfs:Class, owl:Class .

dcmitype:Text a owl:Class .

foaf:primaryTopic a rdf:Property, owl:FunctionalProperty, owl:ObjectProperty .

<http://purl.org/vocab/frbr/core> a owl:Ontology .

<http://vocab.org/frbr/core.html> a dcmitype:Text, foaf:Document .

<http://vocab.org/frbr/core.json> a dcmitype:Text, foaf:Document .

<http://vocab.org/frbr/core.turtle> a dcmitype:Text, foaf:Document .

foaf:topic a rdf:Property, owl:ObjectProperty .

<http://iandavis.com/id/me> a foaf:Person .

<http://bruce.darcus.name/about#me> a foaf:Person .

dc:rights a owl:DatatypeProperty .

vann:preferredNamespaceUri a owl:AnnotationProperty .

vann:preferredNamespacePrefix a owl:AnnotationProperty .

foaf:name a rdf:Property, owl:DatatypeProperty .

<file:///var/www/vocab.org/www/htdocs/frbr/> a msg0:Work .

msg0:license a owl:AnnotationProperty .

<http://creativecommons.org/licenses/by/2.0/uk/> a msg0:License .

msg0:License a owl:Class .

msg0:permits a owl:ObjectProperty .

msg0:Reproduction a msg0:Permission .

msg0:Distribution a msg0:Permission .

msg0:DerivativeWorks a msg0:Permission .

msg0:requires a owl:ObjectProperty .

msg0:Notice a msg0:Requirement .

msg0:Attribution a msg0:Requirement .

vann:changes a owl:AnnotationProperty .

<http://www.isi.edu/~pan/damltime/time-entry.owl#Event> a owl:Class .

wgs84_pos:SpatialThing a owl:Class .

<http://xmlns.com/wordnet/1.6/Work~2> a owl:Class .

dct:IMT a dcam:VocabularyEncodingScheme, owl:Class .

msg0:Permission a owl:Class .

msg0:Requirement a owl:Class .

frbr_core:Endeavour a owl:Class .

frbr_core:ResponsibleEntity a owl:Class .

frbr_core:Subject a owl:Class .

frbr_core:Item a owl:Class .

frbr_core:CorporateBody a owl:Class .

frbr_core:Person a owl:Class .

foaf:Organization a rdfs:Class, owl:Class .

foaf:Group a rdfs:Class, owl:Class .

frbr_core:Object a owl:Class .

frbr_core:Concept a owl:Class .

frbr_core:ClassicalWork a owl:Class .

frbr_core:LegalWork a owl:Class .

frbr_core:LiteraryWork a owl:Class .

frbr_core:ScholarlyWork a owl:Class .

frbr_core:Text a owl:Class .

frbr_core:Image a owl:Class .

frbr_core:Sound a owl:Class .

frbr_core:MovingImage a owl:Class .

frbr_core:Data a owl:Class .

frbr_core:Performance a owl:Class .

frbr_core:relatedEndeavour a owl:ObjectProperty .

frbr_core:realization a owl:ObjectProperty .

frbr_core:realizationOf a owl:ObjectProperty .

frbr_core:embodiment a owl:ObjectProperty .

frbr_core:embodimentOf a owl:ObjectProperty .

frbr_core:exemplar a owl:ObjectProperty .

frbr_core:exemplarOf a owl:ObjectProperty .

frbr_core:reproduction a owl:ObjectProperty .

frbr_core:reproductionOf a owl:ObjectProperty .

frbr_core:successor a owl:ObjectProperty .

frbr_core:successorOf a owl:ObjectProperty .

frbr_core:supplement a owl:ObjectProperty .

frbr_core:supplementOf a owl:ObjectProperty .

frbr_core:complement a owl:ObjectProperty .

frbr_core:complementOf a owl:ObjectProperty .

frbr_core:summarization a owl:ObjectProperty .

frbr_core:summarizationOf a owl:ObjectProperty .

frbr_core:adaption a owl:ObjectProperty .

frbr_core:adaptionOf a owl:ObjectProperty .

frbr_core:transformation a owl:ObjectProperty .

frbr_core:transformationOf a owl:ObjectProperty .

frbr_core:imitation a owl:ObjectProperty .

frbr_core:imitationOf a owl:ObjectProperty .

frbr_core:abridgement a owl:ObjectProperty .

frbr_core:abridgementOf a owl:ObjectProperty .

frbr_core:revision a owl:ObjectProperty .

frbr_core:revisionOf a owl:ObjectProperty .

frbr_core:translation a owl:ObjectProperty .

frbr_core:translationOf a owl:ObjectProperty .

frbr_core:arrangement a owl:ObjectProperty .

frbr_core:arrangementOf a owl:ObjectProperty .

frbr_core:alternate a owl:ObjectProperty .

frbr_core:alternateOf a owl:ObjectProperty .

frbr_core:reconfiguration a owl:ObjectProperty .

frbr_core:reconfigurationOf a owl:ObjectProperty .

frbr_core:part a owl:ObjectProperty .

frbr_core:partOf a owl:ObjectProperty .

frbr_core:responsibleEntity a owl:ObjectProperty .

frbr_core:responsibleEntityOf a owl:ObjectProperty .

frbr_core:creator a owl:ObjectProperty .

frbr_core:creatorOf a owl:ObjectProperty .

frbr_core:realizer a owl:ObjectProperty .

frbr_core:realizerOf a owl:ObjectProperty .

frbr_core:producer a owl:ObjectProperty .

frbr_core:producerOf a owl:ObjectProperty .

frbr_core:owner a owl:ObjectProperty .

frbr_core:ownerOf a owl:ObjectProperty .

frbr_core:subject a owl:ObjectProperty .

<http://xmlns.com/foaf/0.1/> a owl:Ontology .

wot:assurance a owl:AnnotationProperty .

wot:src_assurance a owl:AnnotationProperty .

vs:term_status a owl:AnnotationProperty .

foaf:LabelProperty a rdfs:Class, owl:Class .

foaf:Agent a rdfs:Class, owl:Class .

<http://www.w3.org/2000/10/swap/pim/contact#Person> a owl:Class .

foaf:Project a rdfs:Class, owl:Class .

dct:Agent a dct:AgentClass, owl:Class .

foaf:Image a rdfs:Class, owl:Class .

foaf:PersonalProfileDocument a rdfs:Class, owl:Class .

foaf:OnlineAccount a rdfs:Class, owl:Class .

foaf:OnlineGamingAccount a rdfs:Class, owl:Class .

foaf:OnlineEcommerceAccount a rdfs:Class, owl:Class .

foaf:OnlineChatAccount a rdfs:Class, owl:Class .

foaf:mbox a rdf:Property, owl:InverseFunctionalProperty, owl:ObjectProperty .

foaf:mbox_sha1sum a rdf:Property, owl:DatatypeProperty, owl:InverseFunctionalProperty .

foaf:gender a rdf:Property, owl:DatatypeProperty, owl:FunctionalProperty .

foaf:geekcode a rdf:Property, owl:DatatypeProperty .

foaf:dnaChecksum a rdf:Property, owl:DatatypeProperty .

foaf:sha1 a rdf:Property, owl:DatatypeProperty .

foaf:based_near a rdf:Property, owl:ObjectProperty .

foaf:title a rdf:Property, owl:DatatypeProperty .

foaf:nick a rdf:Property, owl:DatatypeProperty .

foaf:jabberID a rdf:Property, owl:DatatypeProperty, owl:InverseFunctionalProperty .

foaf:aimChatID a rdf:Property, owl:DatatypeProperty, owl:InverseFunctionalProperty .

foaf:skypeID a rdf:Property, owl:DatatypeProperty .

foaf:icqChatID a rdf:Property, owl:DatatypeProperty, owl:InverseFunctionalProperty .

foaf:yahooChatID a rdf:Property, owl:DatatypeProperty, owl:InverseFunctionalProperty .

foaf:msnChatID a rdf:Property, owl:DatatypeProperty, owl:InverseFunctionalProperty .

foaf:firstName a rdf:Property, owl:DatatypeProperty .

foaf:lastName a rdf:Property, owl:DatatypeProperty .

foaf:givenName a rdf:Property, owl:DatatypeProperty .

foaf:givenname a rdf:Property, owl:DatatypeProperty .

foaf:surname a rdf:Property, owl:DatatypeProperty .

foaf:family_name a rdf:Property, owl:DatatypeProperty .

foaf:familyName a rdf:Property, owl:DatatypeProperty .

foaf:phone a rdf:Property, owl:ObjectProperty .

foaf:homepage a rdf:Property, owl:InverseFunctionalProperty, owl:ObjectProperty .

foaf:page a rdf:Property, owl:ObjectProperty .

foaf:isPrimaryTopicOf a rdf:Property, owl:InverseFunctionalProperty .

foaf:weblog a rdf:Property, owl:InverseFunctionalProperty, owl:ObjectProperty .

foaf:openid a rdf:Property, owl:InverseFunctionalProperty, owl:ObjectProperty .

foaf:tipjar a rdf:Property, owl:ObjectProperty .

foaf:plan a rdf:Property, owl:DatatypeProperty .

foaf:made a rdf:Property, owl:ObjectProperty .

foaf:maker a rdf:Property, owl:ObjectProperty .

foaf:img a rdf:Property, owl:ObjectProperty .

foaf:depiction a rdf:Property, owl:ObjectProperty .

foaf:depicts a rdf:Property, owl:ObjectProperty .

foaf:thumbnail a rdf:Property, owl:ObjectProperty .

foaf:myersBriggs a rdf:Property, owl:DatatypeProperty .

foaf:workplaceHomepage a rdf:Property, owl:ObjectProperty .

foaf:workInfoHomepage a rdf:Property, owl:ObjectProperty .

foaf:schoolHomepage a rdf:Property, owl:ObjectProperty .

foaf:knows a rdf:Property, owl:ObjectProperty .

foaf:interest a rdf:Property, owl:ObjectProperty .

foaf:topic_interest a rdf:Property, owl:ObjectProperty .

foaf:publications a rdf:Property, owl:ObjectProperty .

foaf:currentProject a rdf:Property, owl:ObjectProperty .

foaf:pastProject a rdf:Property, owl:ObjectProperty .

foaf:fundedBy a rdf:Property, owl:ObjectProperty .

foaf:logo a rdf:Property, owl:InverseFunctionalProperty, owl:ObjectProperty .

foaf:focus a rdf:Property, owl:ObjectProperty .

foaf:theme a rdf:Property, owl:ObjectProperty .

foaf:account a rdf:Property, owl:ObjectProperty .

foaf:holdsAccount a rdf:Property, owl:ObjectProperty .

foaf:accountServiceHomepage a rdf:Property, owl:ObjectProperty .

foaf:accountName a rdf:Property, owl:DatatypeProperty .

foaf:member a rdf:Property, owl:ObjectProperty .

foaf:membershipClass a rdf:Property, owl:AnnotationProperty .

foaf:birthday a rdf:Property, owl:DatatypeProperty, owl:FunctionalProperty .

foaf:age a rdf:Property, owl:DatatypeProperty, owl:FunctionalProperty .

foaf:status a rdf:Property, owl:DatatypeProperty .

<http://purl.org/NET/dc_owl2dl/terms> a owl:Ontology .

dct:license a owl:AnnotationProperty .

dct:abstract a owl:AnnotationProperty .

dct:accessRights a owl:AnnotationProperty .

dct:RightsStatement a owl:Class .

dct:rights a owl:AnnotationProperty .

dct:accrualMethod a owl:AnnotationProperty .

dct:MethodOfAccrual a owl:Class .

dct:accrualPeriodicity a owl:AnnotationProperty .

dct:Frequency a owl:Class .

dct:accrualPolicy a owl:AnnotationProperty .

dct:Policy a owl:Class .

dct:alternative a owl:AnnotationProperty .

dct:audience a owl:AnnotationProperty .

dct:AgentClass a owl:Class .

dct:available a owl:AnnotationProperty .

dct:date a owl:AnnotationProperty .

dct:bibliographicCitation a owl:AnnotationProperty .

dct:BibliographicResource a owl:Class .

dct:identifier a owl:AnnotationProperty .

dct:conformsTo a owl:AnnotationProperty .

dct:Standard a owl:Class .

dct:relation a owl:AnnotationProperty .

dct:contributor a owl:AnnotationProperty .

dct:coverage a owl:AnnotationProperty .

dct:LocationPeriodOrJurisdiction a owl:Class .

dct:created a owl:AnnotationProperty .

dct:dateAccepted a owl:AnnotationProperty .

dct:dateCopyrighted a owl:AnnotationProperty .

dct:dateSubmitted a owl:AnnotationProperty .

dct:educationLevel a owl:AnnotationProperty .

dct:extent a owl:AnnotationProperty .

dct:SizeOrDuration a owl:Class .

dct:format a owl:AnnotationProperty .

dct:MediaTypeOrExtent a owl:Class .

dct:instructionalMethod a owl:AnnotationProperty .

dct:MethodOfInstruction a owl:Class .

dct:isReferencedBy a owl:AnnotationProperty .

dct:isRequiredBy a owl:AnnotationProperty .

dct:language a owl:AnnotationProperty .

dct:LinguisticSystem a owl:Class .

dct:LicenseDocument a owl:Class .

dct:mediator a owl:AnnotationProperty .

dct:medium a owl:AnnotationProperty .

dct:PhysicalResource a owl:Class .

dct:PhysicalMedium a owl:Class .

dct:ProvenanceStatement a owl:Class .

dct:references a owl:AnnotationProperty .

dct:requires a owl:AnnotationProperty .

dct:rightsHolder a owl:AnnotationProperty .

dct:source a owl:AnnotationProperty .

dct:Location a owl:Class .

dct:subject a owl:AnnotationProperty .

dct:type a owl:AnnotationProperty .

dct:valid a owl:AnnotationProperty .

dct:DCMIType a dcam:VocabularyEncodingScheme .

dct:DDC a dcam:VocabularyEncodingScheme .

dct:LCC a dcam:VocabularyEncodingScheme .

dct:LCSH a dcam:VocabularyEncodingScheme .

dct:MESH a dcam:VocabularyEncodingScheme .

dct:NLM a dcam:VocabularyEncodingScheme .

dct:TGN a dcam:VocabularyEncodingScheme .

dct:UDC a dcam:VocabularyEncodingScheme .

dct:Box a rdfs:Datatype .

dct:ISO3166 a rdfs:Datatype .

dct:ISO639-2 a rdfs:Datatype .

dct:ISO639-3 a rdfs:Datatype .

dct:Period a rdfs:Datatype .

dct:Point a rdfs:Datatype .

dct:RFC1766 a rdfs:Datatype .

dct:RFC3066 a rdfs:Datatype .

dct:RFC4646 a rdfs:Datatype .

dct:URI a rdfs:Datatype .

dct:W3CDTF a rdfs:Datatype .

dct:FileFormat a owl:Class .

dct:MediaType a owl:Class .

dct:Jurisdiction a owl:Class .

<http://www.w3.org/2000/01/rdf-schema#> a owl:Ontology .

rdfs:member a rdf:Property .

<http://www.w3.org/1999/02/22-rdf-syntax-ns#> a owl:Ontology .

rdf:PlainLiteral a rdfs:Datatype, owl:Class .

dct:creator rdfs:subPropertyOf dc:creator, dct:contributor .

ElementsGr2:placeOfBirth rdfs:subPropertyOf aac-ont:associatedPlace .

ElementsGr2:placeOfDeath rdfs:subPropertyOf aac-ont:associatedPlace .

dc:creator rdfs:subPropertyOf edm:hasMet .

dc:contributor rdfs:subPropertyOf edm:hasMet .

skos:altLabel rdfs:subPropertyOf rdfs:label .

dct:issued rdfs:subPropertyOf dct:date .

skos:definition rdfs:subPropertyOf skos:note .

skos:hiddenLabel rdfs:subPropertyOf rdfs:label .

skos:prefLabel rdfs:subPropertyOf rdfs:label .

skos:broadMatch rdfs:subPropertyOf skos:broader, skos:mappingRelation .

skos:broader rdfs:subPropertyOf skos:broaderTransitive .

skos:broaderTransitive rdfs:subPropertyOf skos:semanticRelation .

skos:narrower rdfs:subPropertyOf skos:narrowerTransitive .

skos:narrowerTransitive rdfs:subPropertyOf skos:semanticRelation .

skos:changeNote rdfs:subPropertyOf skos:note .

skos:closeMatch rdfs:subPropertyOf skos:mappingRelation .

skos:editorialNote rdfs:subPropertyOf skos:note .

skos:exactMatch rdfs:subPropertyOf skos:closeMatch .

skos:example rdfs:subPropertyOf skos:note .

skos:historyNote rdfs:subPropertyOf skos:note .

skos:narrowMatch rdfs:subPropertyOf skos:mappingRelation, skos:narrower .

skos:related rdfs:subPropertyOf skos:semanticRelation .

skos:relatedMatch rdfs:subPropertyOf skos:mappingRelation, skos:related .

skos:scopeNote rdfs:subPropertyOf skos:note .

skos:topConceptOf rdfs:subPropertyOf skos:inScheme .

dct:modified rdfs:subPropertyOf dct:date .

dct:title rdfs:subPropertyOf dc:title .

dct:description rdfs:subPropertyOf dc:description .

saam-ont:seeAlsoInSmithsonianAmericanArt rdfs:subPropertyOf rdfs:seeAlso .

saam-ont:seeAlsoWikipedia rdfs:subPropertyOf rdfs:seeAlso .

saam-ont:constituentId rdfs:subPropertyOf dc:identifier .

saam-ont:objectId rdfs:subPropertyOf dc:identifier .

saam-ont:seeAlsoNytimes rdfs:subPropertyOf rdfs:seeAlso .

edm:year rdfs:subPropertyOf dct:temporal .

dct:temporal rdfs:subPropertyOf dct:coverage .

edm:dataProvider rdfs:subPropertyOf dct:provenance .

edm:country rdfs:subPropertyOf crm:P12F.occurred_in_the_presence_of .

edm:userTag rdfs:subPropertyOf dc:description .

edm:hasMet rdfs:subPropertyOf dc:relation .

dc:coverage rdfs:subPropertyOf edm:hasMet .

dc:date rdfs:subPropertyOf edm:hasMet .

dc:format rdfs:subPropertyOf edm:hasType .

edm:hasType rdfs:subPropertyOf edm:isRelatedTo .

dc:language rdfs:subPropertyOf edm:hasType .

dc:publisher rdfs:subPropertyOf edm:hasMet .

dc:relation rdfs:subPropertyOf edm:isRelatedTo .

dc:source rdfs:subPropertyOf edm:isDerivativeOf .

edm:isDerivativeOf rdfs:subPropertyOf edm:isSimilarTo .

dc:subject rdfs:subPropertyOf edm:isRelatedTo .

dc:type rdfs:subPropertyOf edm:hasType .

dct:hasFormat rdfs:subPropertyOf dct:relation, _:node33 .

dct:hasVersion rdfs:subPropertyOf dct:relation, _:node34 .

dct:isFormatOf rdfs:subPropertyOf dct:relation, edm:isDerivativeOf .

dct:isReplacedBy rdfs:subPropertyOf dct:relation, _:node35 .

dct:isVersionOf rdfs:subPropertyOf dct:relation, edm:isDerivativeOf .

dct:replaces rdfs:subPropertyOf dct:relation, edm:isDerivativeOf .

dct:spatial rdfs:subPropertyOf dct:coverage .

dct:tableOfContents rdfs:subPropertyOf dct:description, edm:hasView .

edm:hasView rdfs:subPropertyOf ore:aggregates .

edm:aggregatedCHO rdfs:subPropertyOf dc:subject, crm:P129F.is_about, ore:aggregates .

ore:aggregates rdfs:subPropertyOf dct:hasPart .

edm:currentLocation rdfs:subPropertyOf dct:spatial .

edm:happenedAt rdfs:subPropertyOf dc:relation .

edm:incorporates rdfs:subPropertyOf edm:isSimilarTo .

edm:isSimilarTo rdfs:subPropertyOf dc:relation .

edm:isAnnotationOf rdfs:subPropertyOf dc:subject, crm:P67F.refers_to .

edm:isNextInSequence rdfs:subPropertyOf dc:relation .

edm:isRepresentationOf rdfs:subPropertyOf dc:subject, crm:P138F.represents .

edm:isShownAt rdfs:subPropertyOf edm:landingPage .

edm:landingPage rdfs:subPropertyOf ore:aggregates .

edm:isShownBy rdfs:subPropertyOf edm:hasView .

edm:isSuccessorOf rdfs:subPropertyOf edm:isSimilarTo .

edm:object rdfs:subPropertyOf edm:hasView .

edm:occurredAt rdfs:subPropertyOf dc:relation .

edm:provider rdfs:subPropertyOf edm:hasMet .

edm:realizes rdfs:subPropertyOf edm:isRelatedTo .

edm:wasPresentAt rdfs:subPropertyOf dc:relation .

edm:type rdfs:subPropertyOf dc:type .

dct:publisher rdfs:subPropertyOf dc:publisher .

dct:hasPart rdfs:subPropertyOf dct:relation .

ore:isAggregatedBy rdfs:subPropertyOf dct:isPartOf .

dct:isPartOf rdfs:subPropertyOf dct:relation .

ElementsGr2:dateOfEstablishment rdfs:subPropertyOf ElementsGr2:dateAssociatedWithTheCorporateBody .

ElementsGr2:dateOfConferenceEtc rdfs:subPropertyOf ElementsGr2:dateAssociatedWithTheCorporateBody .

ElementsGr2:dateOfTermination rdfs:subPropertyOf ElementsGr2:dateAssociatedWithTheCorporateBody .

ElementsGr2:dateOfBirth rdfs:subPropertyOf ElementsGr2:DateAssociatedWithThePerson .

ElementsGr2:dateOfDeath rdfs:subPropertyOf ElementsGr2:DateAssociatedWithThePerson .

ElementsGr2:periodOfActivityOfThePerson rdfs:subPropertyOf ElementsGr2:DateAssociatedWithThePerson .

ElementsGr2:fullerFormOfNamePerson rdfs:subPropertyOf ElementsGr2:fullerFormOfName .

ElementsGr2:locationOfConferenceEtc rdfs:subPropertyOf ElementsGr2:placeAssociatedWithTheCorporateBody .

ElementsGr2:locationOfHeadquarters rdfs:subPropertyOf ElementsGr2:placeAssociatedWithTheCorporateBody .

ElementsGr2:preferredNameForTheCorporateBody rdfs:subPropertyOf ElementsGr2:nameOfTheCorporateBody .

ElementsGr2:variantNameForTheCorporateBody rdfs:subPropertyOf ElementsGr2:nameOfTheCorporateBody .

ElementsGr2:preferredNameForTheFamily rdfs:subPropertyOf ElementsGr2:nameOfTheFamily .

ElementsGr2:variantNameForTheFamily rdfs:subPropertyOf ElementsGr2:nameOfTheFamily .

ElementsGr2:preferredNameForThePerson rdfs:subPropertyOf ElementsGr2:nameOfThePerson .

ElementsGr2:variantNameForThePerson rdfs:subPropertyOf ElementsGr2:nameOfThePerson .

ElementsGr2:undifferentiatedNameIndicatorPerson rdfs:subPropertyOf ElementsGr2:undifferentiatedNameIndicator .

ElementsGr2:undifferentiatedNameIndicatorCorporateBody rdfs:subPropertyOf ElementsGr2:undifferentiatedNameIndicator .

ElementsGr2:undifferentiatedNameIndicatorFamily rdfs:subPropertyOf ElementsGr2:undifferentiatedNameIndicator .

foaf:name rdfs:subPropertyOf rdfs:label .

frbr_core:realization rdfs:subPropertyOf frbr_core:relatedEndeavour .

frbr_core:realizationOf rdfs:subPropertyOf frbr_core:relatedEndeavour .

frbr_core:embodiment rdfs:subPropertyOf frbr_core:relatedEndeavour .

frbr_core:embodimentOf rdfs:subPropertyOf frbr_core:relatedEndeavour .

frbr_core:exemplar rdfs:subPropertyOf frbr_core:relatedEndeavour .

frbr_core:exemplarOf rdfs:subPropertyOf frbr_core:relatedEndeavour .

frbr_core:reproduction rdfs:subPropertyOf frbr_core:relatedEndeavour .

frbr_core:reproductionOf rdfs:subPropertyOf frbr_core:relatedEndeavour .

frbr_core:successor rdfs:subPropertyOf frbr_core:relatedEndeavour .

frbr_core:successorOf rdfs:subPropertyOf frbr_core:relatedEndeavour .

frbr_core:supplement rdfs:subPropertyOf frbr_core:relatedEndeavour .

frbr_core:supplementOf rdfs:subPropertyOf frbr_core:relatedEndeavour .

frbr_core:complement rdfs:subPropertyOf frbr_core:relatedEndeavour .

frbr_core:complementOf rdfs:subPropertyOf frbr_core:relatedEndeavour .

frbr_core:summarization rdfs:subPropertyOf frbr_core:relatedEndeavour .

frbr_core:summarizationOf rdfs:subPropertyOf frbr_core:relatedEndeavour .

frbr_core:adaption rdfs:subPropertyOf frbr_core:relatedEndeavour .

frbr_core:adaptionOf rdfs:subPropertyOf frbr_core:relatedEndeavour .

frbr_core:transformation rdfs:subPropertyOf frbr_core:relatedEndeavour .

frbr_core:transformationOf rdfs:subPropertyOf frbr_core:relatedEndeavour .

frbr_core:imitation rdfs:subPropertyOf frbr_core:relatedEndeavour .

frbr_core:imitationOf rdfs:subPropertyOf frbr_core:relatedEndeavour .

frbr_core:abridgement rdfs:subPropertyOf frbr_core:relatedEndeavour .

frbr_core:abridgementOf rdfs:subPropertyOf frbr_core:relatedEndeavour .

frbr_core:revision rdfs:subPropertyOf frbr_core:relatedEndeavour .

frbr_core:revisionOf rdfs:subPropertyOf frbr_core:relatedEndeavour .

frbr_core:translation rdfs:subPropertyOf frbr_core:relatedEndeavour .

frbr_core:translationOf rdfs:subPropertyOf frbr_core:relatedEndeavour .

frbr_core:arrangement rdfs:subPropertyOf frbr_core:relatedEndeavour .

frbr_core:arrangementOf rdfs:subPropertyOf frbr_core:relatedEndeavour .

frbr_core:alternate rdfs:subPropertyOf frbr_core:relatedEndeavour .

frbr_core:alternateOf rdfs:subPropertyOf frbr_core:relatedEndeavour .

frbr_core:reconfiguration rdfs:subPropertyOf frbr_core:relatedEndeavour .

frbr_core:reconfigurationOf rdfs:subPropertyOf frbr_core:relatedEndeavour .

frbr_core:part rdfs:subPropertyOf frbr_core:relatedEndeavour .

frbr_core:partOf rdfs:subPropertyOf frbr_core:relatedEndeavour .

frbr_core:creator rdfs:subPropertyOf frbr_core:responsibleEntity .

frbr_core:creatorOf rdfs:subPropertyOf frbr_core:responsibleEntityOf .

frbr_core:realizer rdfs:subPropertyOf frbr_core:responsibleEntity .

frbr_core:realizerOf rdfs:subPropertyOf frbr_core:responsibleEntityOf .

frbr_core:producer rdfs:subPropertyOf frbr_core:responsibleEntity .

frbr_core:producerOf rdfs:subPropertyOf frbr_core:responsibleEntityOf .

frbr_core:owner rdfs:subPropertyOf frbr_core:responsibleEntity .

frbr_core:ownerOf rdfs:subPropertyOf frbr_core:responsibleEntityOf .

foaf:aimChatID rdfs:subPropertyOf foaf:nick .

foaf:skypeID rdfs:subPropertyOf foaf:nick .

foaf:icqChatID rdfs:subPropertyOf foaf:nick .

foaf:yahooChatID rdfs:subPropertyOf foaf:nick .

foaf:msnChatID rdfs:subPropertyOf foaf:nick .

foaf:homepage rdfs:subPropertyOf foaf:isPrimaryTopicOf, foaf:page .

foaf:isPrimaryTopicOf rdfs:subPropertyOf foaf:page .

foaf:weblog rdfs:subPropertyOf foaf:page .

foaf:openid rdfs:subPropertyOf foaf:isPrimaryTopicOf .

foaf:tipjar rdfs:subPropertyOf foaf:page .

foaf:img rdfs:subPropertyOf foaf:depiction .

dct:license rdfs:subPropertyOf dct:rights .

dct:abstract rdfs:subPropertyOf dct:description .

dct:accessRights rdfs:subPropertyOf dct:rights .

dct:rights rdfs:subPropertyOf dc:rights .

dct:alternative rdfs:subPropertyOf dct:title .

dct:available rdfs:subPropertyOf dct:date .

dct:date rdfs:subPropertyOf dc:date .

dct:bibliographicCitation rdfs:subPropertyOf dct:identifier .

dct:identifier rdfs:subPropertyOf dc:identifier .

dct:conformsTo rdfs:subPropertyOf dct:relation .

dct:relation rdfs:subPropertyOf dc:relation .

dct:contributor rdfs:subPropertyOf dc:contributor .

dct:coverage rdfs:subPropertyOf dc:coverage .

dct:created rdfs:subPropertyOf dct:date .

dct:dateAccepted rdfs:subPropertyOf dct:date .

dct:dateCopyrighted rdfs:subPropertyOf dct:date .

dct:dateSubmitted rdfs:subPropertyOf dct:date .

dct:educationLevel rdfs:subPropertyOf dct:audience .

dct:extent rdfs:subPropertyOf dct:format .

dct:format rdfs:subPropertyOf dc:format .

dct:isReferencedBy rdfs:subPropertyOf dct:relation .

dct:isRequiredBy rdfs:subPropertyOf dct:relation .

dct:language rdfs:subPropertyOf dc:language .

dct:mediator rdfs:subPropertyOf dct:audience .

dct:medium rdfs:subPropertyOf dct:format .

dct:references rdfs:subPropertyOf dct:relation .

dct:requires rdfs:subPropertyOf dct:relation .

dct:source rdfs:subPropertyOf dc:source, dct:relation .

dct:subject rdfs:subPropertyOf dc:subject .

dct:type rdfs:subPropertyOf dc:type .

dct:valid rdfs:subPropertyOf dct:date .

rdf:Property rdfs:subClassOf rdfs:Resource .

rdfs:Class rdfs:subClassOf rdfs:Resource .

rdf:List rdfs:subClassOf rdfs:Resource .

rdf:Statement rdfs:subClassOf rdfs:Resource .

rdfs:Literal rdfs:subClassOf rdfs:Resource .

rdfs:Container rdfs:subClassOf rdfs:Resource .

edm:Agent rdfs:subClassOf edm:NonInformationResource .

aac-ont:Person rdfs:subClassOf frbr:Person, edm:Agent, skos:Concept, foaf:Person .

aac-ont:Place rdfs:subClassOf schema:Place, edm:Place, skos:Concept .

aac-ont:CulturalHeritageObject rdfs:subClassOf edm:ProvidedCHO, skos:Concept .

edm:ProvidedCHO rdfs:subClassOf _:node90 .

_:node90 a owl:Restriction .

skos:Concept rdfs:subClassOf edm:NonInformationResource .

aac-ont:Organization rdfs:subClassOf edm:Agent, skos:Concept .

foaf:Person rdfs:subClassOf frbr_core:ResponsibleEntity, <http://www.w3.org/2000/10/swap/pim/contact#Person>,
    wgs84_pos:SpatialThing, foaf:Agent .

edm:Place rdfs:subClassOf edm:NonInformationResource .

skos:OrderedCollection rdfs:subClassOf skos:Collection .

ore:Aggregation rdfs:subClassOf dcmitype:Collection .

edm:Event rdfs:subClassOf edm:NonInformationResource, _:node84 .

_:node84 a owl:Restriction .

edm:WebResource rdfs:subClassOf edm:InformationResource .

edm:EuropeanaObject rdfs:subClassOf edm:WebResource .

edm:TimeSpan rdfs:subClassOf dct:PeriodOfTime, edm:NonInformationResource .

edm:PhysicalThing rdfs:subClassOf edm:NonInformationResource .

dct:PeriodOfTime rdfs:subClassOf dct:LocationPeriodOrJurisdiction .

frbr_core:Event rdfs:subClassOf frbr_core:Subject, <http://www.isi.edu/~pan/damltime/time-entry.owl#Event> .

frbr_core:Expression rdfs:subClassOf frbr_core:Endeavour .

frbr_core:Manifestation rdfs:subClassOf frbr_core:Endeavour .

frbr_core:Place rdfs:subClassOf frbr_core:Subject, wgs84_pos:SpatialThing .

frbr_core:Work rdfs:subClassOf frbr_core:Endeavour, <http://xmlns.com/wordnet/1.6/Work~2> .

edm:EuropeanaAggregation rdfs:subClassOf edm:EuropeanaObject, ore:Aggregation .

ore:ResourceMap rdfs:subClassOf rdfg:Graph .

frbr_core:Item rdfs:subClassOf frbr_core:Endeavour .

frbr_core:CorporateBody rdfs:subClassOf frbr_core:ResponsibleEntity .

foaf:Organization rdfs:subClassOf frbr_core:CorporateBody, foaf:Agent .

foaf:Group rdfs:subClassOf frbr_core:CorporateBody, foaf:Agent .

frbr_core:Object rdfs:subClassOf frbr_core:Subject, wgs84_pos:SpatialThing .

frbr_core:Concept rdfs:subClassOf frbr_core:Subject, skos:Concept .

frbr_core:ClassicalWork rdfs:subClassOf frbr_core:Work .

frbr_core:LegalWork rdfs:subClassOf frbr_core:Work .

frbr_core:LiteraryWork rdfs:subClassOf frbr_core:Work .

frbr_core:ScholarlyWork rdfs:subClassOf frbr_core:Work .

frbr_core:Text rdfs:subClassOf frbr_core:Expression .

frbr_core:Image rdfs:subClassOf frbr_core:Expression .

frbr_core:Sound rdfs:subClassOf frbr_core:Expression .

frbr_core:MovingImage rdfs:subClassOf frbr_core:Expression .

frbr_core:Data rdfs:subClassOf frbr_core:Expression .

frbr_core:Performance rdfs:subClassOf frbr_core:Expression .

foaf:Image rdfs:subClassOf foaf:Document .

foaf:PersonalProfileDocument rdfs:subClassOf foaf:Document .

foaf:OnlineAccount rdfs:subClassOf owl:Thing .

foaf:OnlineGamingAccount rdfs:subClassOf foaf:OnlineAccount .

foaf:OnlineEcommerceAccount rdfs:subClassOf foaf:OnlineAccount .

foaf:OnlineChatAccount rdfs:subClassOf foaf:OnlineAccount .

dct:SizeOrDuration rdfs:subClassOf dct:MediaTypeOrExtent .

dct:LicenseDocument rdfs:subClassOf dct:RightsStatement .

dct:PhysicalMedium rdfs:subClassOf dct:MediaType .

dct:Location rdfs:subClassOf dct:LocationPeriodOrJurisdiction .

dct:FileFormat rdfs:subClassOf dct:MediaType .

dct:MediaType rdfs:subClassOf dct:MediaTypeOrExtent .

dct:Jurisdiction rdfs:subClassOf dct:LocationPeriodOrJurisdiction .

rdf:PlainLiteral rdfs:subClassOf rdfs:Literal .

rdf:type rdfs:domain rdfs:Resource .

rdfs:subPropertyOf rdfs:domain rdf:Property .

rdfs:domain rdfs:domain rdf:Property .

rdfs:range rdfs:domain rdf:Property .

rdf:value rdfs:domain rdfs:Resource .

rdfs:comment rdfs:domain rdfs:Resource .

rdfs:label rdfs:domain rdfs:Resource .

rdfs:isDefinedBy rdfs:domain rdfs:Resource .

rdfs:seeAlso rdfs:domain rdfs:Resource .

aac-ont:creatorOf rdfs:domain edm:Agent .

ElementsGr2:placeOfBirth rdfs:domain frbr:Person, aac-ont:Person .

ElementsGr2:placeOfDeath rdfs:domain frbr:Person, aac-ont:Person .

aac-ont:sitter rdfs:domain aac-ont:CulturalHeritageObject, edm:ProvidedCHO .

aac-ont:objectId rdfs:domain aac-ont:CulturalHeritageObject .

aac-ont:accessionNumber rdfs:domain aac-ont:CulturalHeritageObject .

skos:mappingRelation rdfs:domain skos:Concept .

skos:semanticRelation rdfs:domain skos:Concept .

skos:hasTopConcept rdfs:domain skos:ConceptScheme .

skos:member rdfs:domain skos:Collection .

skos:memberList rdfs:domain skos:OrderedCollection .

skos:topConceptOf rdfs:domain skos:Concept .

saam-ont:constituentId rdfs:domain aac-ont:Person .

saam-ont:objectId rdfs:domain aac-ont:CulturalHeritageObject .

edm:dataProvider rdfs:domain ore:Aggregation .

edm:hasMet rdfs:domain _:node43 .

_:node43 a owl:Class .

edm:hasType rdfs:domain _:node50 .

_:node50 a owl:Class .

edm:isRelatedTo rdfs:domain _:node64 .

_:node64 a owl:Class .

edm:hasView rdfs:domain ore:Aggregation .

edm:aggregatedCHO rdfs:domain ore:Aggregation .

ore:aggregates rdfs:domain ore:Aggregation .

edm:currentLocation rdfs:domain _:node36 .

_:node36 a owl:Class .

ore:proxyFor rdfs:domain ore:Proxy .

edm:happenedAt rdfs:domain edm:Event .

edm:isAnnotationOf rdfs:domain edm:EuropeanaObject .

edm:isRepresentationOf rdfs:domain edm:InformationResource .

edm:occurredAt rdfs:domain edm:Event .

edm:realizes rdfs:domain edm:PhysicalThing .

edm:wasPresentAt rdfs:domain _:node71 .

_:node71 a owl:Class .

ore:isAggregatedBy rdfs:domain ore:AggregatedResource .

ore:describes rdfs:domain ore:ResourceMap .

ore:isDescribedBy rdfs:domain ore:Aggregation .

ore:lineage rdfs:domain ore:Proxy .

ore:proxyIn rdfs:domain ore:Proxy .

ore:similarTo rdfs:domain ore:Aggregation .

ElementsGr2:addressOfTheCorporateBody rdfs:domain frbr:CorporateBody .

ElementsGr2:addressOfThePerson rdfs:domain frbr:Person .

ElementsGr2:affiliation rdfs:domain frbr:Person .

ElementsGr2:associatedInstitution rdfs:domain frbr:CorporateBody .

ElementsGr2:biographicalInformation rdfs:domain frbr:Person .

ElementsGr2:corporateHistory rdfs:domain frbr:CorporateBody .

ElementsGr2:countryAssociatedWithThePerson rdfs:domain frbr:Person .

ElementsGr2:dateAssociatedWithTheCorporateBody rdfs:domain frbr:CorporateBody .

ElementsGr2:dateOfEstablishment rdfs:domain frbr:CorporateBody .

ElementsGr2:dateOfConferenceEtc rdfs:domain frbr:CorporateBody .

ElementsGr2:dateOfTermination rdfs:domain frbr:CorporateBody .

ElementsGr2:dateAssociatedWithTheFamily rdfs:domain frbr:Family .

ElementsGr2:dateAssociatedWithThePerson rdfs:domain frbr:Person .

ElementsGr2:dateOfBirth rdfs:domain frbr:Person .

ElementsGr2:dateOfDeath rdfs:domain frbr:Person .

ElementsGr2:periodOfActivityOfThePerson rdfs:domain frbr:Person .

ElementsGr2:dateOfUsage rdfs:domain frbr:Name .

ElementsGr2:familyHistory rdfs:domain frbr:Family .

ElementsGr2:fieldOfActivityOfTheCorporateBody rdfs:domain frbr:CorporateBody .

ElementsGr2:fieldOfActivityOfThePerson rdfs:domain frbr:Person .

ElementsGr2:fullerFormOfNamePerson rdfs:domain frbr:Person .

ElementsGr2:gender rdfs:domain frbr:Person .

ElementsGr2:hereditaryTitle rdfs:domain frbr:Family .

ElementsGr2:identifierForTheCorporateBody rdfs:domain frbr:CorporateBody .

ElementsGr2:identifierForTheFamily rdfs:domain frbr:Family .

ElementsGr2:identifierForThePerson rdfs:domain frbr:Person .

ElementsGr2:languageOfTheCorporateBody rdfs:domain frbr:CorporateBody .

ElementsGr2:languageOfThePerson rdfs:domain frbr:Person .

ElementsGr2:locationOfConferenceEtc rdfs:domain frbr:CorporateBody .

ElementsGr2:placeAssociatedWithTheCorporateBody rdfs:domain frbr:CorporateBody .

ElementsGr2:locationOfHeadquarters rdfs:domain frbr:CorporateBody .

ElementsGr2:name rdfs:domain frbr:Agent .

ElementsGr2:nameOfTheCorporateBody rdfs:domain frbr:CorporateBody .

ElementsGr2:preferredNameForTheCorporateBody rdfs:domain frbr:CorporateBody .

ElementsGr2:variantNameForTheCorporateBody rdfs:domain frbr:CorporateBody .

ElementsGr2:nameOfTheFamily rdfs:domain frbr:Family .

ElementsGr2:preferredNameForTheFamily rdfs:domain frbr:Family .

ElementsGr2:variantNameForTheFamily rdfs:domain frbr:Family .

ElementsGr2:nameOfThePerson rdfs:domain frbr:Person .

ElementsGr2:preferredNameForThePerson rdfs:domain frbr:Person .

ElementsGr2:variantNameForThePerson rdfs:domain frbr:Person .

ElementsGr2:numberOfAConferenceEtc rdfs:domain frbr:CorporateBody .

ElementsGr2:otherDesignationAssociatedWithTheCorporateBody rdfs:domain frbr:CorporateBody .

ElementsGr2:otherDesignationAssociatedWithThePerson rdfs:domain frbr:Person .

ElementsGr2:placeAssociatedWithTheFamily rdfs:domain frbr:Family .

ElementsGr2:placeOfResidence rdfs:domain frbr:Person .

ElementsGr2:professionOrOccupation rdfs:domain frbr:Person .

ElementsGr2:prominentMemberOfTheFamily rdfs:domain frbr:Family .

ElementsGr2:scopeOfUsage rdfs:domain frbr:Name .

ElementsGr2:titleOfThePerson rdfs:domain frbr:Person .

ElementsGr2:typeOfFamily rdfs:domain frbr:Family .

ElementsGr2:undifferentiatedNameIndicatorPerson rdfs:domain frbr:Person .

ElementsGr2:undifferentiatedNameIndicatorCorporateBody rdfs:domain frbr:CorporateBody .

ElementsGr2:undifferentiatedNameIndicatorFamily rdfs:domain frbr:Family .

foaf:primaryTopic rdfs:domain foaf:Document .

foaf:topic rdfs:domain foaf:Document .

foaf:name rdfs:domain owl:Thing .

frbr_core:relatedEndeavour rdfs:domain frbr_core:Endeavour .

frbr_core:realization rdfs:domain frbr_core:Work .

frbr_core:realizationOf rdfs:domain frbr_core:Expression .

frbr_core:embodiment rdfs:domain frbr_core:Expression .

frbr_core:embodimentOf rdfs:domain frbr_core:Manifestation .

frbr_core:exemplar rdfs:domain frbr_core:Manifestation .

frbr_core:exemplarOf rdfs:domain frbr_core:Item .

frbr_core:reproduction rdfs:domain _:genid-38640ccbd5eb49418600e8d7df2cf451-mor50bd147e3fa74 .

_:genid-38640ccbd5eb49418600e8d7df2cf451-mor50bd147e3fa74 a owl:Class .

frbr_core:reproductionOf rdfs:domain _:genid-38640ccbd5eb49418600e8d7df2cf451-mor50bd147e3fd1d .

_:genid-38640ccbd5eb49418600e8d7df2cf451-mor50bd147e3fd1d a owl:Class .

frbr_core:successor rdfs:domain _:genid-38640ccbd5eb49418600e8d7df2cf451-mor50bd147e3ffcb .

_:genid-38640ccbd5eb49418600e8d7df2cf451-mor50bd147e3ffcb a owl:Class .

frbr_core:successorOf rdfs:domain _:genid-38640ccbd5eb49418600e8d7df2cf451-mor50bd147e40268 .

_:genid-38640ccbd5eb49418600e8d7df2cf451-mor50bd147e40268 a owl:Class .

frbr_core:supplement rdfs:domain _:genid-38640ccbd5eb49418600e8d7df2cf451-mor50bd147e40518 .

_:genid-38640ccbd5eb49418600e8d7df2cf451-mor50bd147e40518 a owl:Class .

frbr_core:supplementOf rdfs:domain _:genid-38640ccbd5eb49418600e8d7df2cf451-mor50bd147e407b8 .

_:genid-38640ccbd5eb49418600e8d7df2cf451-mor50bd147e407b8 a owl:Class .

frbr_core:complement rdfs:domain _:genid-38640ccbd5eb49418600e8d7df2cf451-mor50bd147e40a5a .

_:genid-38640ccbd5eb49418600e8d7df2cf451-mor50bd147e40a5a a owl:Class .

frbr_core:complementOf rdfs:domain _:genid-38640ccbd5eb49418600e8d7df2cf451-mor50bd147e40cf8 .

_:genid-38640ccbd5eb49418600e8d7df2cf451-mor50bd147e40cf8 a owl:Class .

frbr_core:summarization rdfs:domain _:genid-38640ccbd5eb49418600e8d7df2cf451-mor50bd147e40f9b .

_:genid-38640ccbd5eb49418600e8d7df2cf451-mor50bd147e40f9b a owl:Class .

frbr_core:summarizationOf rdfs:domain _:genid-38640ccbd5eb49418600e8d7df2cf451-mor50bd147e41242 .

_:genid-38640ccbd5eb49418600e8d7df2cf451-mor50bd147e41242 a owl:Class .

frbr_core:adaption rdfs:domain _:genid-38640ccbd5eb49418600e8d7df2cf451-mor50bd147e414ef .

_:genid-38640ccbd5eb49418600e8d7df2cf451-mor50bd147e414ef a owl:Class .

frbr_core:adaptionOf rdfs:domain _:genid-38640ccbd5eb49418600e8d7df2cf451-mor50bd147e4179c .

_:genid-38640ccbd5eb49418600e8d7df2cf451-mor50bd147e4179c a owl:Class .

frbr_core:transformation rdfs:domain _:genid-38640ccbd5eb49418600e8d7df2cf451-mor50bd147e41a3a .

_:genid-38640ccbd5eb49418600e8d7df2cf451-mor50bd147e41a3a a owl:Class .

frbr_core:transformationOf rdfs:domain _:genid-38640ccbd5eb49418600e8d7df2cf451-mor50bd147e41cd7 .

_:genid-38640ccbd5eb49418600e8d7df2cf451-mor50bd147e41cd7 a owl:Class .

frbr_core:imitation rdfs:domain _:genid-38640ccbd5eb49418600e8d7df2cf451-mor50bd147e41f77 .

_:genid-38640ccbd5eb49418600e8d7df2cf451-mor50bd147e41f77 a owl:Class .

frbr_core:imitationOf rdfs:domain _:genid-38640ccbd5eb49418600e8d7df2cf451-mor50bd147e42224 .

_:genid-38640ccbd5eb49418600e8d7df2cf451-mor50bd147e42224 a owl:Class .

frbr_core:abridgement rdfs:domain frbr_core:Expression .

frbr_core:abridgementOf rdfs:domain frbr_core:Expression .

frbr_core:revision rdfs:domain frbr_core:Expression .

frbr_core:revisionOf rdfs:domain frbr_core:Expression .

frbr_core:translation rdfs:domain frbr_core:Expression .

frbr_core:translationOf rdfs:domain frbr_core:Expression .

frbr_core:arrangement rdfs:domain frbr_core:Expression .

frbr_core:arrangementOf rdfs:domain frbr_core:Expression .

frbr_core:alternate rdfs:domain frbr_core:Manifestation .

frbr_core:alternateOf rdfs:domain frbr_core:Manifestation .

frbr_core:reconfiguration rdfs:domain frbr_core:Item .

frbr_core:reconfigurationOf rdfs:domain frbr_core:Item .

frbr_core:responsibleEntity rdfs:domain frbr_core:Endeavour .

frbr_core:responsibleEntityOf rdfs:domain frbr_core:ResponsibleEntity .

frbr_core:creator rdfs:domain frbr_core:Work .

frbr_core:creatorOf rdfs:domain frbr_core:ResponsibleEntity .

frbr_core:realizer rdfs:domain frbr_core:Expression .

frbr_core:realizerOf rdfs:domain frbr_core:ResponsibleEntity .

frbr_core:producer rdfs:domain frbr_core:Manifestation .

frbr_core:producerOf rdfs:domain frbr_core:ResponsibleEntity .

frbr_core:owner rdfs:domain frbr_core:Item .

frbr_core:ownerOf rdfs:domain frbr_core:ResponsibleEntity .

frbr_core:subject rdfs:domain frbr_core:Work .

foaf:mbox rdfs:domain foaf:Agent .

foaf:mbox_sha1sum rdfs:domain foaf:Agent .

foaf:gender rdfs:domain foaf:Agent .

foaf:geekcode rdfs:domain foaf:Person .

foaf:sha1 rdfs:domain foaf:Document .

foaf:based_near rdfs:domain wgs84_pos:SpatialThing .

foaf:jabberID rdfs:domain foaf:Agent .

foaf:aimChatID rdfs:domain foaf:Agent .

foaf:skypeID rdfs:domain foaf:Agent .

foaf:icqChatID rdfs:domain foaf:Agent .

foaf:yahooChatID rdfs:domain foaf:Agent .

foaf:msnChatID rdfs:domain foaf:Agent .

foaf:firstName rdfs:domain foaf:Person .

foaf:lastName rdfs:domain foaf:Person .

foaf:surname rdfs:domain foaf:Person .

foaf:family_name rdfs:domain foaf:Person .

foaf:familyName rdfs:domain foaf:Person .

foaf:homepage rdfs:domain owl:Thing .

foaf:page rdfs:domain owl:Thing .

foaf:isPrimaryTopicOf rdfs:domain owl:Thing .

foaf:weblog rdfs:domain foaf:Agent .

foaf:openid rdfs:domain foaf:Agent .

foaf:tipjar rdfs:domain foaf:Agent .

foaf:plan rdfs:domain foaf:Person .

foaf:made rdfs:domain foaf:Agent .

foaf:maker rdfs:domain owl:Thing .

foaf:img rdfs:domain foaf:Person .

foaf:depiction rdfs:domain owl:Thing .

foaf:depicts rdfs:domain foaf:Image .

foaf:thumbnail rdfs:domain foaf:Image .

foaf:myersBriggs rdfs:domain foaf:Person .

foaf:workplaceHomepage rdfs:domain foaf:Person .

foaf:workInfoHomepage rdfs:domain foaf:Person .

foaf:schoolHomepage rdfs:domain foaf:Person .

foaf:knows rdfs:domain foaf:Person .

foaf:interest rdfs:domain foaf:Agent .

foaf:topic_interest rdfs:domain foaf:Agent .

foaf:publications rdfs:domain foaf:Person .

foaf:currentProject rdfs:domain foaf:Person .

foaf:pastProject rdfs:domain foaf:Person .

foaf:fundedBy rdfs:domain owl:Thing .

foaf:logo rdfs:domain owl:Thing .

foaf:focus rdfs:domain <http://www.w3.org/2004/02/skos/core#Concept> .

foaf:theme rdfs:domain owl:Thing .

foaf:account rdfs:domain foaf:Agent .

foaf:holdsAccount rdfs:domain foaf:Agent .

foaf:accountServiceHomepage rdfs:domain foaf:OnlineAccount .

foaf:accountName rdfs:domain foaf:OnlineAccount .

foaf:member rdfs:domain foaf:Group .

foaf:birthday rdfs:domain foaf:Agent .

foaf:age rdfs:domain foaf:Agent .

foaf:status rdfs:domain foaf:Agent .

dct:accrualMethod rdfs:domain dcmitype:Collection .

dct:accrualPeriodicity rdfs:domain dcmitype:Collection .

dct:accrualPolicy rdfs:domain dcmitype:Collection .

dct:bibliographicCitation rdfs:domain dct:BibliographicResource .

dct:medium rdfs:domain dct:PhysicalResource .

rdfs:member rdfs:domain rdfs:Resource .

rdf:type rdfs:range rdfs:Class .

rdfs:subPropertyOf rdfs:range rdf:Property .

rdf:subject rdfs:range rdfs:Resource .

rdf:predicate rdfs:range rdfs:Resource .

rdf:object rdfs:range rdfs:Resource .

rdf:first rdfs:range rdfs:Resource .

rdf:value rdfs:range rdfs:Resource .

rdfs:isDefinedBy rdfs:range rdfs:Resource .

rdfs:seeAlso rdfs:range rdfs:Resource .

dct:creator rdfs:range dct:Agent, edm:Agent .

ElementsGr2:placeOfBirth rdfs:range <http://americanart.si.edu/saam/SaamPlace>, aac-ont:Place .

aac-ont:associatedPlace rdfs:range aac-ont:Place .

ElementsGr2:placeOfDeath rdfs:range aac-ont:Place .

aac-ont:sitter rdfs:range aac-ont:Person .

dct:issued rdfs:range rdfs:Literal .

skos:mappingRelation rdfs:range skos:Concept .

skos:semanticRelation rdfs:range skos:Concept .

skos:hasTopConcept rdfs:range skos:Concept .

skos:inScheme rdfs:range skos:ConceptScheme .

skos:memberList rdfs:range rdf:List .

skos:topConceptOf rdfs:range skos:ConceptScheme .

dct:modified rdfs:range rdfs:Literal .

dct:temporal rdfs:range dct:PeriodOfTime .

edm:dataProvider rdfs:range edm:Agent .

dct:provenance rdfs:range dct:ProvenanceStatement .

edm:hasType rdfs:range edm:NonInformationResource .

dct:spatial rdfs:range dct:Location .

edm:hasView rdfs:range edm:WebResource .

edm:aggregatedCHO rdfs:range edm:ProvidedCHO .

ore:aggregates rdfs:range ore:AggregatedResource .

edm:currentLocation rdfs:range edm:Place .

ore:proxyFor rdfs:range ore:AggregatedResource .

edm:happenedAt rdfs:range edm:Place .

edm:isAnnotationOf rdfs:range _:node57 .

_:node57 a owl:Class .

edm:isShownAt rdfs:range edm:WebResource .

edm:landingPage rdfs:range edm:WebResource .

edm:isShownBy rdfs:range edm:WebResource .

edm:object rdfs:range edm:WebResource .

edm:occurredAt rdfs:range edm:TimeSpan .

edm:provider rdfs:range edm:Agent .

edm:realizes rdfs:range edm:InformationResource .

edm:wasPresentAt rdfs:range edm:Event .

edm:type rdfs:range _:node75 .

_:node75 a rdfs:Datatype .

edm:ugc rdfs:range _:node81 .

_:node81 a rdfs:Datatype .

dct:publisher rdfs:range dct:Agent .

ore:isAggregatedBy rdfs:range ore:Aggregation .

ore:describes rdfs:range ore:Aggregation .

ore:isDescribedBy rdfs:range ore:ResourceMap .

ore:lineage rdfs:range ore:Proxy .

ore:proxyIn rdfs:range ore:Aggregation .

ElementsGr2:name rdfs:range frbr:Name .

foaf:primaryTopic rdfs:range owl:Thing .

foaf:topic rdfs:range owl:Thing .

foaf:name rdfs:range rdfs:Literal .

frbr_core:relatedEndeavour rdfs:range frbr_core:Endeavour .

frbr_core:realization rdfs:range frbr_core:Expression .

frbr_core:realizationOf rdfs:range frbr_core:Work .

frbr_core:embodiment rdfs:range frbr_core:Manifestation .

frbr_core:embodimentOf rdfs:range frbr_core:Expression .

frbr_core:exemplar rdfs:range frbr_core:Item .

frbr_core:exemplarOf rdfs:range frbr_core:Manifestation .

frbr_core:reproduction rdfs:range _:genid-38640ccbd5eb49418600e8d7df2cf451-mor50bd147e3fb4c .

_:genid-38640ccbd5eb49418600e8d7df2cf451-mor50bd147e3fb4c a owl:Class .

frbr_core:reproductionOf rdfs:range _:genid-38640ccbd5eb49418600e8d7df2cf451-mor50bd147e3fdf6 .

_:genid-38640ccbd5eb49418600e8d7df2cf451-mor50bd147e3fdf6 a owl:Class .

frbr_core:successor rdfs:range _:genid-38640ccbd5eb49418600e8d7df2cf451-mor50bd147e4009b .

_:genid-38640ccbd5eb49418600e8d7df2cf451-mor50bd147e4009b a owl:Class .

frbr_core:successorOf rdfs:range _:genid-38640ccbd5eb49418600e8d7df2cf451-mor50bd147e4033f .

_:genid-38640ccbd5eb49418600e8d7df2cf451-mor50bd147e4033f a owl:Class .

frbr_core:supplement rdfs:range _:genid-38640ccbd5eb49418600e8d7df2cf451-mor50bd147e405e9 .

_:genid-38640ccbd5eb49418600e8d7df2cf451-mor50bd147e405e9 a owl:Class .

frbr_core:supplementOf rdfs:range _:genid-38640ccbd5eb49418600e8d7df2cf451-mor50bd147e4088a .

_:genid-38640ccbd5eb49418600e8d7df2cf451-mor50bd147e4088a a owl:Class .

frbr_core:complement rdfs:range _:genid-38640ccbd5eb49418600e8d7df2cf451-mor50bd147e40b2b .

_:genid-38640ccbd5eb49418600e8d7df2cf451-mor50bd147e40b2b a owl:Class .

frbr_core:complementOf rdfs:range _:genid-38640ccbd5eb49418600e8d7df2cf451-mor50bd147e40dca .

_:genid-38640ccbd5eb49418600e8d7df2cf451-mor50bd147e40dca a owl:Class .

frbr_core:summarization rdfs:range _:genid-38640ccbd5eb49418600e8d7df2cf451-mor50bd147e4106d .

_:genid-38640ccbd5eb49418600e8d7df2cf451-mor50bd147e4106d a owl:Class .

frbr_core:summarizationOf rdfs:range _:genid-38640ccbd5eb49418600e8d7df2cf451-mor50bd147e41321 .

_:genid-38640ccbd5eb49418600e8d7df2cf451-mor50bd147e41321 a owl:Class .

frbr_core:adaption rdfs:range _:genid-38640ccbd5eb49418600e8d7df2cf451-mor50bd147e415c4 .

_:genid-38640ccbd5eb49418600e8d7df2cf451-mor50bd147e415c4 a owl:Class .

frbr_core:adaptionOf rdfs:range _:genid-38640ccbd5eb49418600e8d7df2cf451-mor50bd147e4186b .

_:genid-38640ccbd5eb49418600e8d7df2cf451-mor50bd147e4186b a owl:Class .

frbr_core:transformation rdfs:range _:genid-38640ccbd5eb49418600e8d7df2cf451-mor50bd147e41b0c .

_:genid-38640ccbd5eb49418600e8d7df2cf451-mor50bd147e41b0c a owl:Class .

frbr_core:transformationOf rdfs:range _:genid-38640ccbd5eb49418600e8d7df2cf451-mor50bd147e41daa .

_:genid-38640ccbd5eb49418600e8d7df2cf451-mor50bd147e41daa a owl:Class .

frbr_core:imitation rdfs:range _:genid-38640ccbd5eb49418600e8d7df2cf451-mor50bd147e42048 .

_:genid-38640ccbd5eb49418600e8d7df2cf451-mor50bd147e42048 a owl:Class .

frbr_core:imitationOf rdfs:range _:genid-38640ccbd5eb49418600e8d7df2cf451-mor50bd147e422f7 .

_:genid-38640ccbd5eb49418600e8d7df2cf451-mor50bd147e422f7 a owl:Class .

frbr_core:abridgement rdfs:range frbr_core:Expression .

frbr_core:abridgementOf rdfs:range frbr_core:Expression .

frbr_core:revision rdfs:range frbr_core:Expression .

frbr_core:revisionOf rdfs:range frbr_core:Expression .

frbr_core:translation rdfs:range frbr_core:Expression .

frbr_core:translationOf rdfs:range frbr_core:Expression .

frbr_core:arrangement rdfs:range frbr_core:Expression .

frbr_core:arrangementOf rdfs:range frbr_core:Expression .

frbr_core:alternate rdfs:range frbr_core:Manifestation .

frbr_core:alternateOf rdfs:range frbr_core:Manifestation .

frbr_core:reconfiguration rdfs:range frbr_core:Item .

frbr_core:reconfigurationOf rdfs:range frbr_core:Item .

frbr_core:responsibleEntity rdfs:range frbr_core:ResponsibleEntity .

frbr_core:responsibleEntityOf rdfs:range frbr_core:Endeavour .

frbr_core:creator rdfs:range frbr_core:ResponsibleEntity .

frbr_core:creatorOf rdfs:range frbr_core:Work .

frbr_core:realizer rdfs:range frbr_core:ResponsibleEntity .

frbr_core:realizerOf rdfs:range frbr_core:Expression .

frbr_core:producer rdfs:range frbr_core:ResponsibleEntity .

frbr_core:producerOf rdfs:range frbr_core:Manifestation .

frbr_core:owner rdfs:range frbr_core:ResponsibleEntity .

frbr_core:ownerOf rdfs:range frbr_core:Item .

frbr_core:subject rdfs:range _:genid-38640ccbd5eb49418600e8d7df2cf451-mor50bd147e4365e .

_:genid-38640ccbd5eb49418600e8d7df2cf451-mor50bd147e4365e a owl:Class .

foaf:mbox rdfs:range owl:Thing .

foaf:mbox_sha1sum rdfs:range rdfs:Literal .

foaf:gender rdfs:range rdfs:Literal .

foaf:geekcode rdfs:range rdfs:Literal .

foaf:dnaChecksum rdfs:range rdfs:Literal .

foaf:based_near rdfs:range wgs84_pos:SpatialThing .

foaf:jabberID rdfs:range rdfs:Literal .

foaf:aimChatID rdfs:range rdfs:Literal .

foaf:skypeID rdfs:range rdfs:Literal .

foaf:icqChatID rdfs:range rdfs:Literal .

foaf:yahooChatID rdfs:range rdfs:Literal .

foaf:msnChatID rdfs:range rdfs:Literal .

foaf:firstName rdfs:range rdfs:Literal .

foaf:lastName rdfs:range rdfs:Literal .

foaf:surname rdfs:range rdfs:Literal .

foaf:family_name rdfs:range rdfs:Literal .

foaf:familyName rdfs:range rdfs:Literal .

foaf:homepage rdfs:range foaf:Document .

foaf:page rdfs:range foaf:Document .

foaf:isPrimaryTopicOf rdfs:range foaf:Document .

foaf:weblog rdfs:range foaf:Document .

foaf:openid rdfs:range foaf:Document .

foaf:tipjar rdfs:range foaf:Document .

foaf:plan rdfs:range rdfs:Literal .

foaf:made rdfs:range owl:Thing .

foaf:maker rdfs:range foaf:Agent;
  owl:equivalentProperty dct:creator .

foaf:img rdfs:range foaf:Image .

foaf:depiction rdfs:range foaf:Image .

foaf:depicts rdfs:range owl:Thing .

foaf:thumbnail rdfs:range foaf:Image .

foaf:myersBriggs rdfs:range rdfs:Literal .

foaf:workplaceHomepage rdfs:range foaf:Document .

foaf:workInfoHomepage rdfs:range foaf:Document .

foaf:schoolHomepage rdfs:range foaf:Document .

foaf:knows rdfs:range foaf:Person .

foaf:interest rdfs:range foaf:Document .

foaf:topic_interest rdfs:range owl:Thing .

foaf:publications rdfs:range foaf:Document .

foaf:currentProject rdfs:range owl:Thing .

foaf:pastProject rdfs:range owl:Thing .

foaf:fundedBy rdfs:range owl:Thing .

foaf:logo rdfs:range owl:Thing .

foaf:focus rdfs:range owl:Thing .

foaf:theme rdfs:range owl:Thing .

foaf:account rdfs:range foaf:OnlineAccount .

foaf:holdsAccount rdfs:range foaf:OnlineAccount .

foaf:accountServiceHomepage rdfs:range foaf:Document .

foaf:accountName rdfs:range rdfs:Literal .

foaf:member rdfs:range foaf:Agent .

foaf:birthday rdfs:range rdfs:Literal .

foaf:age rdfs:range rdfs:Literal .

foaf:status rdfs:range rdfs:Literal .

dct:license rdfs:range dct:LicenseDocument .

dct:accessRights rdfs:range dct:RightsStatement .

dct:rights rdfs:range dct:RightsStatement .

dct:accrualMethod rdfs:range dct:MethodOfAccrual .

dct:accrualPeriodicity rdfs:range dct:Frequency .

dct:accrualPolicy rdfs:range dct:Policy .

dct:audience rdfs:range dct:AgentClass .

dct:available rdfs:range rdfs:Literal .

dct:date rdfs:range rdfs:Literal .

dct:bibliographicCitation rdfs:range rdfs:Literal .

dct:identifier rdfs:range rdfs:Literal .

dct:conformsTo rdfs:range dct:Standard .

dct:contributor rdfs:range dct:Agent .

dct:coverage rdfs:range dct:LocationPeriodOrJurisdiction .

dct:created rdfs:range rdfs:Literal .

dct:dateAccepted rdfs:range rdfs:Literal .

dct:dateCopyrighted rdfs:range rdfs:Literal .

dct:dateSubmitted rdfs:range rdfs:Literal .

dct:educationLevel rdfs:range dct:AgentClass .

dct:extent rdfs:range dct:SizeOrDuration .

dct:format rdfs:range dct:MediaTypeOrExtent .

dct:instructionalMethod rdfs:range dct:MethodOfInstruction .

dct:language rdfs:range dct:LinguisticSystem .

dct:mediator rdfs:range dct:AgentClass .

dct:medium rdfs:range dct:PhysicalMedium .

dct:rightsHolder rdfs:range dct:Agent .

dct:type rdfs:range owl:Class .

dct:valid rdfs:range rdfs:Literal .

rdfs:member rdfs:range rdfs:Resource .

edm:Place owl:equivalentClass DOLCE-Lite:space-region .

edm:NonInformationResource owl:equivalentClass _:node89 .

_:node89 a owl:Class .

edm:InformationResource owl:equivalentClass _:node85 .

_:node85 a owl:Class .

edm:TimeSpan owl:equivalentClass DOLCE-Lite:time-interval .

abc:Place owl:equivalentClass edm:Place .

abc:Temporality owl:equivalentClass edm:Event .

abc:Time owl:equivalentClass edm:TimeSpan .

frbr_core:Event owl:equivalentClass edm:Event .

frbr_core:Place owl:equivalentClass edm:Place .

crm:E18.Physical_Thing owl:equivalentClass edm:PhysicalThing .

crm:E39.Actor owl:equivalentClass edm:Agent .

crm:E4.Period owl:equivalentClass edm:Event .

crm:E52.Time-Span owl:equivalentClass edm:TimeSpan .

crm:E53.Place owl:equivalentClass edm:Place .

crm:E89.Propositional_Object owl:equivalentClass edm:InformationResource .

edm:EuropeanaAggregation owl:equivalentClass _:node83 .

_:node83 a owl:Restriction .

frbr_core:Endeavour owl:equivalentClass _:genid-38640ccbd5eb49418600e8d7df2cf451-mor50bd147e3e0bd .

_:genid-38640ccbd5eb49418600e8d7df2cf451-mor50bd147e3e0bd a owl:Class .

frbr_core:ResponsibleEntity owl:equivalentClass _:genid-38640ccbd5eb49418600e8d7df2cf451-mor50bd147e3e84b .

_:genid-38640ccbd5eb49418600e8d7df2cf451-mor50bd147e3e84b a owl:Class .

frbr_core:Subject owl:equivalentClass _:genid-38640ccbd5eb49418600e8d7df2cf451-mor50bd147e3ed08 .

_:genid-38640ccbd5eb49418600e8d7df2cf451-mor50bd147e3ed08 a owl:Class .

frbr_core:CorporateBody owl:equivalentClass _:genid-38640ccbd5eb49418600e8d7df2cf451-mor50bd147e3eb2e .

_:genid-38640ccbd5eb49418600e8d7df2cf451-mor50bd147e3eb2e a owl:Class .

frbr_core:Person owl:equivalentClass foaf:Person .

foaf:Agent owl:equivalentClass dct:Agent .

aac-ont:creatorOf owl:inverseOf dct:creator .

skos:broader owl:inverseOf skos:narrower .

skos:broaderTransitive owl:inverseOf skos:narrowerTransitive .

skos:narrowMatch owl:inverseOf skos:broadMatch .

skos:topConceptOf owl:inverseOf skos:hasTopConcept .

ore:aggregates owl:inverseOf ore:isAggregatedBy .

ore:isAggregatedBy owl:inverseOf ore:aggregates .

ore:describes owl:inverseOf ore:isDescribedBy .

ore:isDescribedBy owl:inverseOf ore:describes .

foaf:primaryTopic owl:inverseOf foaf:isPrimaryTopicOf .

foaf:topic owl:inverseOf foaf:page .

frbr_core:realization owl:inverseOf frbr_core:realizationOf .

frbr_core:realizationOf owl:inverseOf frbr_core:realization .

frbr_core:embodiment owl:inverseOf frbr_core:embodimentOf .

frbr_core:embodimentOf owl:inverseOf frbr_core:embodiment .

frbr_core:exemplar owl:inverseOf frbr_core:exemplarOf .

frbr_core:exemplarOf owl:inverseOf frbr_core:exemplar .

frbr_core:reproduction owl:inverseOf frbr_core:reproductionOf .

frbr_core:reproductionOf owl:inverseOf frbr_core:reproduction .

frbr_core:successor owl:inverseOf frbr_core:successorOf .

frbr_core:successorOf owl:inverseOf frbr_core:successor .

frbr_core:supplement owl:inverseOf frbr_core:supplementOf .

frbr_core:supplementOf owl:inverseOf frbr_core:supplement .

frbr_core:complement owl:inverseOf frbr_core:complementOf .

frbr_core:complementOf owl:inverseOf frbr_core:complement .

frbr_core:summarization owl:inverseOf frbr_core:summarizationOf .

frbr_core:summarizationOf owl:inverseOf frbr_core:summarization .

frbr_core:adaption owl:inverseOf frbr_core:adaptionOf .

frbr_core:adaptionOf owl:inverseOf frbr_core:adaption .

frbr_core:transformation owl:inverseOf frbr_core:transformationOf .

frbr_core:transformationOf owl:inverseOf frbr_core:transformation .

frbr_core:imitation owl:inverseOf frbr_core:imitationOf .

frbr_core:imitationOf owl:inverseOf frbr_core:imitation .

frbr_core:abridgement owl:inverseOf frbr_core:abridgementOf .

frbr_core:abridgementOf owl:inverseOf frbr_core:abridgement .

frbr_core:revision owl:inverseOf frbr_core:revisionOf .

frbr_core:revisionOf owl:inverseOf frbr_core:revision .

frbr_core:translation owl:inverseOf frbr_core:translationOf .

frbr_core:translationOf owl:inverseOf frbr_core:translation .

frbr_core:arrangement owl:inverseOf frbr_core:arrangementOf .

frbr_core:arrangementOf owl:inverseOf frbr_core:arrangement .

frbr_core:alternate owl:inverseOf frbr_core:alternateOf .

frbr_core:alternateOf owl:inverseOf frbr_core:alternate .

frbr_core:reconfiguration owl:inverseOf frbr_core:reconfigurationOf .

frbr_core:reconfigurationOf owl:inverseOf frbr_core:reconfiguration .

frbr_core:part owl:inverseOf frbr_core:partOf .

frbr_core:partOf owl:inverseOf frbr_core:part .

frbr_core:responsibleEntity owl:inverseOf frbr_core:responsibleEntityOf .

frbr_core:responsibleEntityOf owl:inverseOf frbr_core:responsibleEntity .

frbr_core:creator owl:inverseOf frbr_core:creatorOf .

frbr_core:creatorOf owl:inverseOf frbr_core:creator .

frbr_core:realizer owl:inverseOf frbr_core:realizerOf .

frbr_core:realizerOf owl:inverseOf frbr_core:realizer .

frbr_core:producer owl:inverseOf frbr_core:producerOf .

frbr_core:producerOf owl:inverseOf frbr_core:producer .

frbr_core:owner owl:inverseOf frbr_core:ownerOf .

frbr_core:ownerOf owl:inverseOf frbr_core:owner .

foaf:page owl:inverseOf foaf:topic .

foaf:isPrimaryTopicOf owl:inverseOf foaf:primaryTopic .

foaf:made owl:inverseOf foaf:maker .

foaf:maker owl:inverseOf foaf:made .

foaf:depiction owl:inverseOf foaf:depicts .

foaf:depicts owl:inverseOf foaf:depiction .

_:node38 a owl:Class .

_:node41 a owl:Restriction .

_:node45 a owl:Class .

_:node48 a owl:Restriction .

_:node52 a owl:Class .

_:node55 a owl:Restriction .

_:node59 a owl:Class .

_:node62 a owl:Restriction .

_:node66 a owl:Class .

_:node69 a owl:Restriction .

_:node76 a rdf:List;
  rdf:first "3D" .

_:node77 a rdf:List;
  rdf:first "IMAGE" .

_:node78 a rdf:List;
  rdf:first "SOUND" .

_:node79 a rdf:List;
  rdf:first "TEXT" .

_:node80 a rdf:List;
  rdf:first "VIDEO" .

_:node82 a rdf:List;
  rdf:first "TRUE" .

_:genid-38640ccbd5eb49418600e8d7df2cf451-mor50bd147e3df08 a foaf:Person .

_:node33 owl:inverseOf edm:isDerivativeOf .

_:node34 owl:inverseOf edm:isDerivativeOf .

_:node35 owl:inverseOf edm:isDerivativeOf .

_:node91 owl:inverseOf edm:aggregatedCHO .

_:node37 rdf:first edm:ProvidedCHO .

_:node39 rdf:first _:node38 .

_:node40 rdf:first ore:Proxy .

_:node42 rdf:first _:node41 .

_:node44 rdf:first edm:ProvidedCHO .

_:node46 rdf:first _:node45 .

_:node47 rdf:first ore:Proxy .

_:node49 rdf:first _:node48 .

_:node51 rdf:first edm:ProvidedCHO .

_:node53 rdf:first _:node52 .

_:node54 rdf:first ore:Proxy .

_:node56 rdf:first _:node55 .

_:node58 rdf:first edm:ProvidedCHO .

_:node60 rdf:first _:node59 .

_:node61 rdf:first ore:Proxy .

_:node63 rdf:first _:node62 .

_:node65 rdf:first edm:ProvidedCHO .

_:node67 rdf:first _:node66 .

_:node68 rdf:first ore:Proxy .

_:node70 rdf:first _:node69 .

_:node72 rdf:first edm:Agent .

_:node73 rdf:first edm:InformationResource .

_:node74 rdf:first edm:PhysicalThing .

_:node86 rdf:first frbr_core:Expression .

_:node87 rdf:first frbr_core:Manifestation .

_:node88 rdf:first frbr_core:Work .

_:genid-38640ccbd5eb49418600e8d7df2cf451-mor50bd147e3e105 rdf:first frbr_core:Expression .

_:genid-38640ccbd5eb49418600e8d7df2cf451-mor50bd147e3e14a rdf:first frbr_core:Item .

_:genid-38640ccbd5eb49418600e8d7df2cf451-mor50bd147e3e190 rdf:first frbr_core:Manifestation .

_:genid-38640ccbd5eb49418600e8d7df2cf451-mor50bd147e3e1d5 rdf:first frbr_core:Work .

_:genid-38640ccbd5eb49418600e8d7df2cf451-mor50bd147e3e892 rdf:first frbr_core:CorporateBody .

_:genid-38640ccbd5eb49418600e8d7df2cf451-mor50bd147e3e8d7 rdf:first foaf:Person .

_:genid-38640ccbd5eb49418600e8d7df2cf451-mor50bd147e3eb74 rdf:first foaf:Organization .

_:genid-38640ccbd5eb49418600e8d7df2cf451-mor50bd147e3ebba rdf:first foaf:Group .

_:genid-38640ccbd5eb49418600e8d7df2cf451-mor50bd147e3ed4e rdf:first frbr_core:Event .

_:genid-38640ccbd5eb49418600e8d7df2cf451-mor50bd147e3ed94 rdf:first frbr_core:Object .

_:genid-38640ccbd5eb49418600e8d7df2cf451-mor50bd147e3edda rdf:first frbr_core:Place .

_:genid-38640ccbd5eb49418600e8d7df2cf451-mor50bd147e3ee1f rdf:first frbr_core:Concept .

_:genid-38640ccbd5eb49418600e8d7df2cf451-mor50bd147e3faba rdf:first frbr_core:Manifestation .

_:genid-38640ccbd5eb49418600e8d7df2cf451-mor50bd147e3fb01 rdf:first frbr_core:Item .

_:genid-38640ccbd5eb49418600e8d7df2cf451-mor50bd147e3fb92 rdf:first frbr_core:Manifestation .

_:genid-38640ccbd5eb49418600e8d7df2cf451-mor50bd147e3fbd7 rdf:first frbr_core:Item .

_:genid-38640ccbd5eb49418600e8d7df2cf451-mor50bd147e3fd63 rdf:first frbr_core:Manifestation .

_:genid-38640ccbd5eb49418600e8d7df2cf451-mor50bd147e3fdab rdf:first frbr_core:Item .

_:genid-38640ccbd5eb49418600e8d7df2cf451-mor50bd147e3fe3c rdf:first frbr_core:Manifestation .

_:genid-38640ccbd5eb49418600e8d7df2cf451-mor50bd147e3fe82 rdf:first frbr_core:Item .

_:genid-38640ccbd5eb49418600e8d7df2cf451-mor50bd147e4000c rdf:first frbr_core:Work .

_:genid-38640ccbd5eb49418600e8d7df2cf451-mor50bd147e40050 rdf:first frbr_core:Expression .

_:genid-38640ccbd5eb49418600e8d7df2cf451-mor50bd147e400dc rdf:first frbr_core:Work .

_:genid-38640ccbd5eb49418600e8d7df2cf451-mor50bd147e40122 rdf:first frbr_core:Expression .

_:genid-38640ccbd5eb49418600e8d7df2cf451-mor50bd147e402a9 rdf:first frbr_core:Work .

_:genid-38640ccbd5eb49418600e8d7df2cf451-mor50bd147e402ed rdf:first frbr_core:Expression .

_:genid-38640ccbd5eb49418600e8d7df2cf451-mor50bd147e40380 rdf:first frbr_core:Work .

_:genid-38640ccbd5eb49418600e8d7df2cf451-mor50bd147e403c8 rdf:first frbr_core:Expression .

_:genid-38640ccbd5eb49418600e8d7df2cf451-mor50bd147e40559 rdf:first frbr_core:Work .

_:genid-38640ccbd5eb49418600e8d7df2cf451-mor50bd147e4059f rdf:first frbr_core:Expression .

_:genid-38640ccbd5eb49418600e8d7df2cf451-mor50bd147e4062b rdf:first frbr_core:Work .

_:genid-38640ccbd5eb49418600e8d7df2cf451-mor50bd147e4066f rdf:first frbr_core:Expression .

_:genid-38640ccbd5eb49418600e8d7df2cf451-mor50bd147e407f9 rdf:first frbr_core:Work .

_:genid-38640ccbd5eb49418600e8d7df2cf451-mor50bd147e40840 rdf:first frbr_core:Expression .

_:genid-38640ccbd5eb49418600e8d7df2cf451-mor50bd147e408cb rdf:first frbr_core:Work .

_:genid-38640ccbd5eb49418600e8d7df2cf451-mor50bd147e40910 rdf:first frbr_core:Expression .

_:genid-38640ccbd5eb49418600e8d7df2cf451-mor50bd147e40a9b rdf:first frbr_core:Work .

_:genid-38640ccbd5eb49418600e8d7df2cf451-mor50bd147e40ae1 rdf:first frbr_core:Expression .

_:genid-38640ccbd5eb49418600e8d7df2cf451-mor50bd147e40b6a rdf:first frbr_core:Work .

_:genid-38640ccbd5eb49418600e8d7df2cf451-mor50bd147e40baf rdf:first frbr_core:Expression .

_:genid-38640ccbd5eb49418600e8d7df2cf451-mor50bd147e40d3a rdf:first frbr_core:Work .

_:genid-38640ccbd5eb49418600e8d7df2cf451-mor50bd147e40d80 rdf:first frbr_core:Expression .

_:genid-38640ccbd5eb49418600e8d7df2cf451-mor50bd147e40e0b rdf:first frbr_core:Work .

_:genid-38640ccbd5eb49418600e8d7df2cf451-mor50bd147e40e50 rdf:first frbr_core:Expression .

_:genid-38640ccbd5eb49418600e8d7df2cf451-mor50bd147e40fdc rdf:first frbr_core:Work .

_:genid-38640ccbd5eb49418600e8d7df2cf451-mor50bd147e41022 rdf:first frbr_core:Expression .

_:genid-38640ccbd5eb49418600e8d7df2cf451-mor50bd147e410ae rdf:first frbr_core:Work .

_:genid-38640ccbd5eb49418600e8d7df2cf451-mor50bd147e410f3 rdf:first frbr_core:Expression .

_:genid-38640ccbd5eb49418600e8d7df2cf451-mor50bd147e41285 rdf:first frbr_core:Work .

_:genid-38640ccbd5eb49418600e8d7df2cf451-mor50bd147e412d7 rdf:first frbr_core:Expression .

_:genid-38640ccbd5eb49418600e8d7df2cf451-mor50bd147e41362 rdf:first frbr_core:Work .

_:genid-38640ccbd5eb49418600e8d7df2cf451-mor50bd147e413a8 rdf:first frbr_core:Expression .

_:genid-38640ccbd5eb49418600e8d7df2cf451-mor50bd147e41531 rdf:first frbr_core:Work .

_:genid-38640ccbd5eb49418600e8d7df2cf451-mor50bd147e41578 rdf:first frbr_core:Expression .

_:genid-38640ccbd5eb49418600e8d7df2cf451-mor50bd147e41604 rdf:first frbr_core:Work .

_:genid-38640ccbd5eb49418600e8d7df2cf451-mor50bd147e41652 rdf:first frbr_core:Expression .

_:genid-38640ccbd5eb49418600e8d7df2cf451-mor50bd147e417db rdf:first frbr_core:Work .

_:genid-38640ccbd5eb49418600e8d7df2cf451-mor50bd147e41821 rdf:first frbr_core:Expression .

_:genid-38640ccbd5eb49418600e8d7df2cf451-mor50bd147e418ab rdf:first frbr_core:Work .

_:genid-38640ccbd5eb49418600e8d7df2cf451-mor50bd147e418f1 rdf:first frbr_core:Expression .

_:genid-38640ccbd5eb49418600e8d7df2cf451-mor50bd147e41a7c rdf:first frbr_core:Work .

_:genid-38640ccbd5eb49418600e8d7df2cf451-mor50bd147e41ac2 rdf:first frbr_core:Expression .

_:genid-38640ccbd5eb49418600e8d7df2cf451-mor50bd147e41b4b rdf:first frbr_core:Work .

_:genid-38640ccbd5eb49418600e8d7df2cf451-mor50bd147e41b91 rdf:first frbr_core:Expression .

_:genid-38640ccbd5eb49418600e8d7df2cf451-mor50bd147e41d18 rdf:first frbr_core:Work .

_:genid-38640ccbd5eb49418600e8d7df2cf451-mor50bd147e41d5e rdf:first frbr_core:Expression .

_:genid-38640ccbd5eb49418600e8d7df2cf451-mor50bd147e41dea rdf:first frbr_core:Work .

_:genid-38640ccbd5eb49418600e8d7df2cf451-mor50bd147e41e30 rdf:first frbr_core:Expression .

_:genid-38640ccbd5eb49418600e8d7df2cf451-mor50bd147e41fb9 rdf:first frbr_core:Work .

_:genid-38640ccbd5eb49418600e8d7df2cf451-mor50bd147e41ffe rdf:first frbr_core:Expression .

_:genid-38640ccbd5eb49418600e8d7df2cf451-mor50bd147e42089 rdf:first frbr_core:Work .

_:genid-38640ccbd5eb49418600e8d7df2cf451-mor50bd147e420d2 rdf:first frbr_core:Expression .

_:genid-38640ccbd5eb49418600e8d7df2cf451-mor50bd147e42266 rdf:first frbr_core:Work .

_:genid-38640ccbd5eb49418600e8d7df2cf451-mor50bd147e422ac rdf:first frbr_core:Expression .

_:genid-38640ccbd5eb49418600e8d7df2cf451-mor50bd147e42338 rdf:first frbr_core:Work .

_:genid-38640ccbd5eb49418600e8d7df2cf451-mor50bd147e4237e rdf:first frbr_core:Expression .

_:genid-38640ccbd5eb49418600e8d7df2cf451-mor50bd147e4369f rdf:first frbr_core:Endeavour .

_:genid-38640ccbd5eb49418600e8d7df2cf451-mor50bd147e436e6 rdf:first frbr_core:ResponsibleEntity .

_:genid-38640ccbd5eb49418600e8d7df2cf451-mor50bd147e4372d rdf:first frbr_core:Subject .

_:node37 rdf:rest _:node39 .

_:node39 rdf:rest rdf:nil .

_:node40 rdf:rest _:node42 .

_:node42 rdf:rest rdf:nil .

_:node44 rdf:rest _:node46 .

_:node46 rdf:rest rdf:nil .

_:node47 rdf:rest _:node49 .

_:node49 rdf:rest rdf:nil .

_:node51 rdf:rest _:node53 .

_:node53 rdf:rest rdf:nil .

_:node54 rdf:rest _:node56 .

_:node56 rdf:rest rdf:nil .

_:node58 rdf:rest _:node60 .

_:node60 rdf:rest rdf:nil .

_:node61 rdf:rest _:node63 .

_:node63 rdf:rest rdf:nil .

_:node65 rdf:rest _:node67 .

_:node67 rdf:rest rdf:nil .

_:node68 rdf:rest _:node70 .

_:node70 rdf:rest rdf:nil .

_:node72 rdf:rest _:node73 .

_:node73 rdf:rest _:node74 .

_:node74 rdf:rest rdf:nil .

_:node76 rdf:rest _:node77 .

_:node77 rdf:rest _:node78 .

_:node78 rdf:rest _:node79 .

_:node79 rdf:rest _:node80 .

_:node80 rdf:rest rdf:nil .

_:node82 rdf:rest rdf:nil .

_:node86 rdf:rest _:node87 .

_:node87 rdf:rest _:node88 .

_:node88 rdf:rest rdf:nil .

_:genid-38640ccbd5eb49418600e8d7df2cf451-mor50bd147e3e105 rdf:rest _:genid-38640ccbd5eb49418600e8d7df2cf451-mor50bd147e3e14a .

_:genid-38640ccbd5eb49418600e8d7df2cf451-mor50bd147e3e14a rdf:rest _:genid-38640ccbd5eb49418600e8d7df2cf451-mor50bd147e3e190 .

_:genid-38640ccbd5eb49418600e8d7df2cf451-mor50bd147e3e190 rdf:rest _:genid-38640ccbd5eb49418600e8d7df2cf451-mor50bd147e3e1d5 .

_:genid-38640ccbd5eb49418600e8d7df2cf451-mor50bd147e3e1d5 rdf:rest rdf:nil .

_:genid-38640ccbd5eb49418600e8d7df2cf451-mor50bd147e3e892 rdf:rest _:genid-38640ccbd5eb49418600e8d7df2cf451-mor50bd147e3e8d7 .

_:genid-38640ccbd5eb49418600e8d7df2cf451-mor50bd147e3e8d7 rdf:rest rdf:nil .

_:genid-38640ccbd5eb49418600e8d7df2cf451-mor50bd147e3eb74 rdf:rest _:genid-38640ccbd5eb49418600e8d7df2cf451-mor50bd147e3ebba .

_:genid-38640ccbd5eb49418600e8d7df2cf451-mor50bd147e3ebba rdf:rest rdf:nil .

_:genid-38640ccbd5eb49418600e8d7df2cf451-mor50bd147e3ed4e rdf:rest _:genid-38640ccbd5eb49418600e8d7df2cf451-mor50bd147e3ed94 .

_:genid-38640ccbd5eb49418600e8d7df2cf451-mor50bd147e3ed94 rdf:rest _:genid-38640ccbd5eb49418600e8d7df2cf451-mor50bd147e3edda .

_:genid-38640ccbd5eb49418600e8d7df2cf451-mor50bd147e3edda rdf:rest _:genid-38640ccbd5eb49418600e8d7df2cf451-mor50bd147e3ee1f .

_:genid-38640ccbd5eb49418600e8d7df2cf451-mor50bd147e3ee1f rdf:rest rdf:nil .

_:genid-38640ccbd5eb49418600e8d7df2cf451-mor50bd147e3faba rdf:rest _:genid-38640ccbd5eb49418600e8d7df2cf451-mor50bd147e3fb01 .

_:genid-38640ccbd5eb49418600e8d7df2cf451-mor50bd147e3fb01 rdf:rest rdf:nil .

_:genid-38640ccbd5eb49418600e8d7df2cf451-mor50bd147e3fb92 rdf:rest _:genid-38640ccbd5eb49418600e8d7df2cf451-mor50bd147e3fbd7 .

_:genid-38640ccbd5eb49418600e8d7df2cf451-mor50bd147e3fbd7 rdf:rest rdf:nil .

_:genid-38640ccbd5eb49418600e8d7df2cf451-mor50bd147e3fd63 rdf:rest _:genid-38640ccbd5eb49418600e8d7df2cf451-mor50bd147e3fdab .

_:genid-38640ccbd5eb49418600e8d7df2cf451-mor50bd147e3fdab rdf:rest rdf:nil .

_:genid-38640ccbd5eb49418600e8d7df2cf451-mor50bd147e3fe3c rdf:rest _:genid-38640ccbd5eb49418600e8d7df2cf451-mor50bd147e3fe82 .

_:genid-38640ccbd5eb49418600e8d7df2cf451-mor50bd147e3fe82 rdf:rest rdf:nil .

_:genid-38640ccbd5eb49418600e8d7df2cf451-mor50bd147e4000c rdf:rest _:genid-38640ccbd5eb49418600e8d7df2cf451-mor50bd147e40050 .

_:genid-38640ccbd5eb49418600e8d7df2cf451-mor50bd147e40050 rdf:rest rdf:nil .

_:genid-38640ccbd5eb49418600e8d7df2cf451-mor50bd147e400dc rdf:rest _:genid-38640ccbd5eb49418600e8d7df2cf451-mor50bd147e40122 .

_:genid-38640ccbd5eb49418600e8d7df2cf451-mor50bd147e40122 rdf:rest rdf:nil .

_:genid-38640ccbd5eb49418600e8d7df2cf451-mor50bd147e402a9 rdf:rest _:genid-38640ccbd5eb49418600e8d7df2cf451-mor50bd147e402ed .

_:genid-38640ccbd5eb49418600e8d7df2cf451-mor50bd147e402ed rdf:rest rdf:nil .

_:genid-38640ccbd5eb49418600e8d7df2cf451-mor50bd147e40380 rdf:rest _:genid-38640ccbd5eb49418600e8d7df2cf451-mor50bd147e403c8 .

_:genid-38640ccbd5eb49418600e8d7df2cf451-mor50bd147e403c8 rdf:rest rdf:nil .

_:genid-38640ccbd5eb49418600e8d7df2cf451-mor50bd147e40559 rdf:rest _:genid-38640ccbd5eb49418600e8d7df2cf451-mor50bd147e4059f .

_:genid-38640ccbd5eb49418600e8d7df2cf451-mor50bd147e4059f rdf:rest rdf:nil .

_:genid-38640ccbd5eb49418600e8d7df2cf451-mor50bd147e4062b rdf:rest _:genid-38640ccbd5eb49418600e8d7df2cf451-mor50bd147e4066f .

_:genid-38640ccbd5eb49418600e8d7df2cf451-mor50bd147e4066f rdf:rest rdf:nil .

_:genid-38640ccbd5eb49418600e8d7df2cf451-mor50bd147e407f9 rdf:rest _:genid-38640ccbd5eb49418600e8d7df2cf451-mor50bd147e40840 .

_:genid-38640ccbd5eb49418600e8d7df2cf451-mor50bd147e40840 rdf:rest rdf:nil .

_:genid-38640ccbd5eb49418600e8d7df2cf451-mor50bd147e408cb rdf:rest _:genid-38640ccbd5eb49418600e8d7df2cf451-mor50bd147e40910 .

_:genid-38640ccbd5eb49418600e8d7df2cf451-mor50bd147e40910 rdf:rest rdf:nil .

_:genid-38640ccbd5eb49418600e8d7df2cf451-mor50bd147e40a9b rdf:rest _:genid-38640ccbd5eb49418600e8d7df2cf451-mor50bd147e40ae1 .

_:genid-38640ccbd5eb49418600e8d7df2cf451-mor50bd147e40ae1 rdf:rest rdf:nil .

_:genid-38640ccbd5eb49418600e8d7df2cf451-mor50bd147e40b6a rdf:rest _:genid-38640ccbd5eb49418600e8d7df2cf451-mor50bd147e40baf .

_:genid-38640ccbd5eb49418600e8d7df2cf451-mor50bd147e40baf rdf:rest rdf:nil .

_:genid-38640ccbd5eb49418600e8d7df2cf451-mor50bd147e40d3a rdf:rest _:genid-38640ccbd5eb49418600e8d7df2cf451-mor50bd147e40d80 .

_:genid-38640ccbd5eb49418600e8d7df2cf451-mor50bd147e40d80 rdf:rest rdf:nil .

_:genid-38640ccbd5eb49418600e8d7df2cf451-mor50bd147e40e0b rdf:rest _:genid-38640ccbd5eb49418600e8d7df2cf451-mor50bd147e40e50 .

_:genid-38640ccbd5eb49418600e8d7df2cf451-mor50bd147e40e50 rdf:rest rdf:nil .

_:genid-38640ccbd5eb49418600e8d7df2cf451-mor50bd147e40fdc rdf:rest _:genid-38640ccbd5eb49418600e8d7df2cf451-mor50bd147e41022 .

_:genid-38640ccbd5eb49418600e8d7df2cf451-mor50bd147e41022 rdf:rest rdf:nil .

_:genid-38640ccbd5eb49418600e8d7df2cf451-mor50bd147e410ae rdf:rest _:genid-38640ccbd5eb49418600e8d7df2cf451-mor50bd147e410f3 .

_:genid-38640ccbd5eb49418600e8d7df2cf451-mor50bd147e410f3 rdf:rest rdf:nil .

_:genid-38640ccbd5eb49418600e8d7df2cf451-mor50bd147e41285 rdf:rest _:genid-38640ccbd5eb49418600e8d7df2cf451-mor50bd147e412d7 .

_:genid-38640ccbd5eb49418600e8d7df2cf451-mor50bd147e412d7 rdf:rest rdf:nil .

_:genid-38640ccbd5eb49418600e8d7df2cf451-mor50bd147e41362 rdf:rest _:genid-38640ccbd5eb49418600e8d7df2cf451-mor50bd147e413a8 .

_:genid-38640ccbd5eb49418600e8d7df2cf451-mor50bd147e413a8 rdf:rest rdf:nil .

_:genid-38640ccbd5eb49418600e8d7df2cf451-mor50bd147e41531 rdf:rest _:genid-38640ccbd5eb49418600e8d7df2cf451-mor50bd147e41578 .

_:genid-38640ccbd5eb49418600e8d7df2cf451-mor50bd147e41578 rdf:rest rdf:nil .

_:genid-38640ccbd5eb49418600e8d7df2cf451-mor50bd147e41604 rdf:rest _:genid-38640ccbd5eb49418600e8d7df2cf451-mor50bd147e41652 .

_:genid-38640ccbd5eb49418600e8d7df2cf451-mor50bd147e41652 rdf:rest rdf:nil .

_:genid-38640ccbd5eb49418600e8d7df2cf451-mor50bd147e417db rdf:rest _:genid-38640ccbd5eb49418600e8d7df2cf451-mor50bd147e41821 .

_:genid-38640ccbd5eb49418600e8d7df2cf451-mor50bd147e41821 rdf:rest rdf:nil .

_:genid-38640ccbd5eb49418600e8d7df2cf451-mor50bd147e418ab rdf:rest _:genid-38640ccbd5eb49418600e8d7df2cf451-mor50bd147e418f1 .

_:genid-38640ccbd5eb49418600e8d7df2cf451-mor50bd147e418f1 rdf:rest rdf:nil .

_:genid-38640ccbd5eb49418600e8d7df2cf451-mor50bd147e41a7c rdf:rest _:genid-38640ccbd5eb49418600e8d7df2cf451-mor50bd147e41ac2 .

_:genid-38640ccbd5eb49418600e8d7df2cf451-mor50bd147e41ac2 rdf:rest rdf:nil .

_:genid-38640ccbd5eb49418600e8d7df2cf451-mor50bd147e41b4b rdf:rest _:genid-38640ccbd5eb49418600e8d7df2cf451-mor50bd147e41b91 .

_:genid-38640ccbd5eb49418600e8d7df2cf451-mor50bd147e41b91 rdf:rest rdf:nil .

_:genid-38640ccbd5eb49418600e8d7df2cf451-mor50bd147e41d18 rdf:rest _:genid-38640ccbd5eb49418600e8d7df2cf451-mor50bd147e41d5e .

_:genid-38640ccbd5eb49418600e8d7df2cf451-mor50bd147e41d5e rdf:rest rdf:nil .

_:genid-38640ccbd5eb49418600e8d7df2cf451-mor50bd147e41dea rdf:rest _:genid-38640ccbd5eb49418600e8d7df2cf451-mor50bd147e41e30 .

_:genid-38640ccbd5eb49418600e8d7df2cf451-mor50bd147e41e30 rdf:rest rdf:nil .

_:genid-38640ccbd5eb49418600e8d7df2cf451-mor50bd147e41fb9 rdf:rest _:genid-38640ccbd5eb49418600e8d7df2cf451-mor50bd147e41ffe .

_:genid-38640ccbd5eb49418600e8d7df2cf451-mor50bd147e41ffe rdf:rest rdf:nil .

_:genid-38640ccbd5eb49418600e8d7df2cf451-mor50bd147e42089 rdf:rest _:genid-38640ccbd5eb49418600e8d7df2cf451-mor50bd147e420d2 .

_:genid-38640ccbd5eb49418600e8d7df2cf451-mor50bd147e420d2 rdf:rest rdf:nil .

_:genid-38640ccbd5eb49418600e8d7df2cf451-mor50bd147e42266 rdf:rest _:genid-38640ccbd5eb49418600e8d7df2cf451-mor50bd147e422ac .

_:genid-38640ccbd5eb49418600e8d7df2cf451-mor50bd147e422ac rdf:rest rdf:nil .

_:genid-38640ccbd5eb49418600e8d7df2cf451-mor50bd147e42338 rdf:rest _:genid-38640ccbd5eb49418600e8d7df2cf451-mor50bd147e4237e .

_:genid-38640ccbd5eb49418600e8d7df2cf451-mor50bd147e4237e rdf:rest rdf:nil .

_:genid-38640ccbd5eb49418600e8d7df2cf451-mor50bd147e4369f rdf:rest _:genid-38640ccbd5eb49418600e8d7df2cf451-mor50bd147e436e6 .

_:genid-38640ccbd5eb49418600e8d7df2cf451-mor50bd147e436e6 rdf:rest _:genid-38640ccbd5eb49418600e8d7df2cf451-mor50bd147e4372d .

_:genid-38640ccbd5eb49418600e8d7df2cf451-mor50bd147e4372d rdf:rest rdf:nil .

_:genid-38640ccbd5eb49418600e8d7df2cf451-mor50bd147e3e223 rdf:value "Added isDefinedBy property referring to FRBR core namespace" .

_:genid-38640ccbd5eb49418600e8d7df2cf451-mor50bd147e3e26f rdf:value "Added comment" .

_:genid-38640ccbd5eb49418600e8d7df2cf451-mor50bd147e3e2bf rdf:value "Extracted definition from existing comment" .

_:genid-38640ccbd5eb49418600e8d7df2cf451-mor50bd147e3e496 rdf:value "Added isDefinedBy property referring to FRBR core namespace" .

_:genid-38640ccbd5eb49418600e8d7df2cf451-mor50bd147e3e4e2 rdf:value "Added comment" .

_:genid-38640ccbd5eb49418600e8d7df2cf451-mor50bd147e3e52e rdf:value "Extracted definition from existing comment" .

_:genid-38640ccbd5eb49418600e8d7df2cf451-mor50bd147e3e6b4 rdf:value "Added isDefinedBy property referring to FRBR core namespace" .

_:genid-38640ccbd5eb49418600e8d7df2cf451-mor50bd147e3e74b rdf:value "Added comment" .

_:genid-38640ccbd5eb49418600e8d7df2cf451-mor50bd147e3e798 rdf:value "Extracted definition from existing comment" .

_:genid-38640ccbd5eb49418600e8d7df2cf451-mor50bd147e3e700 rdf:value "Made subclass of geo:SpatialThing" .

_:genid-38640ccbd5eb49418600e8d7df2cf451-mor50bd147e3e7e4 rdf:value "Removed subclass of geo:SpatialThing" .

_:genid-38640ccbd5eb49418600e8d7df2cf451-mor50bd147e3e5a5 rdf:value "Added isDefinedBy property referring to FRBR core namespace" .

_:genid-38640ccbd5eb49418600e8d7df2cf451-mor50bd147e3e5f3 rdf:value "Added comment" .

_:genid-38640ccbd5eb49418600e8d7df2cf451-mor50bd147e3e641 rdf:value "Extracted definition from existing comment" .

_:genid-38640ccbd5eb49418600e8d7df2cf451-mor50bd147e3e336 rdf:value "Added isDefinedBy property referring to FRBR core namespace" .

_:genid-38640ccbd5eb49418600e8d7df2cf451-mor50bd147e3e383 rdf:value "Added comment" .

_:genid-38640ccbd5eb49418600e8d7df2cf451-mor50bd147e3e424 rdf:value "Extracted definition from existing comment" .

_:genid-38640ccbd5eb49418600e8d7df2cf451-mor50bd147e3e3d8 rdf:value "Made subclass of wordnet:Work~2" .

_:genid-38640ccbd5eb49418600e8d7df2cf451-mor50bd147e3e925 rdf:value "Added isDefinedBy property referring to FRBR core namespace" .

_:genid-38640ccbd5eb49418600e8d7df2cf451-mor50bd147e3e971 rdf:value "Added comment" .

_:genid-38640ccbd5eb49418600e8d7df2cf451-mor50bd147e3e9bd rdf:value "Extracted definition from existing comment" .

_:genid-38640ccbd5eb49418600e8d7df2cf451-mor50bd147e3ec08 rdf:value "Added isDefinedBy property referring to FRBR core namespace" .

_:genid-38640ccbd5eb49418600e8d7df2cf451-mor50bd147e3ec53 rdf:value "Added comment" .

_:genid-38640ccbd5eb49418600e8d7df2cf451-mor50bd147e3ec9f rdf:value "Extracted definition from existing comment" .

_:genid-38640ccbd5eb49418600e8d7df2cf451-mor50bd147e3ea2b rdf:value "Added isDefinedBy property referring to FRBR core namespace" .

_:genid-38640ccbd5eb49418600e8d7df2cf451-mor50bd147e3ea78 rdf:value "Added comment" .

_:genid-38640ccbd5eb49418600e8d7df2cf451-mor50bd147e3eac9 rdf:value "Extracted definition from existing comment" .

_:genid-38640ccbd5eb49418600e8d7df2cf451-mor50bd147e3ee70 rdf:value "Added isDefinedBy property referring to FRBR core namespace" .

_:genid-38640ccbd5eb49418600e8d7df2cf451-mor50bd147e3eebb rdf:value "Added comment" .

_:genid-38640ccbd5eb49418600e8d7df2cf451-mor50bd147e3ef08 rdf:value "Extracted definition from existing comment" .

_:genid-38640ccbd5eb49418600e8d7df2cf451-mor50bd147e3f23c rdf:value "Added comment" .

_:genid-38640ccbd5eb49418600e8d7df2cf451-mor50bd147e3f2de rdf:value "Extracted definition from existing comment" .

_:genid-38640ccbd5eb49418600e8d7df2cf451-mor50bd147e3f292 rdf:value "Made subclass of owltime:Event" .

_:genid-38640ccbd5eb49418600e8d7df2cf451-mor50bd147e3f0e2 rdf:value "Added isDefinedBy property referring to FRBR core namespace" .

_:genid-38640ccbd5eb49418600e8d7df2cf451-mor50bd147e3f12e rdf:value "Added comment" .

_:genid-38640ccbd5eb49418600e8d7df2cf451-mor50bd147e3f1c4 rdf:value "Extracted definition from existing comment" .

_:genid-38640ccbd5eb49418600e8d7df2cf451-mor50bd147e3f17a rdf:value "Made subclass of geo:SpatialThing" .

_:genid-38640ccbd5eb49418600e8d7df2cf451-mor50bd147e3f354 rdf:value "Added isDefinedBy property referring to FRBR core namespace" .

_:genid-38640ccbd5eb49418600e8d7df2cf451-mor50bd147e3f3a9 rdf:value "Added comment" .

_:genid-38640ccbd5eb49418600e8d7df2cf451-mor50bd147e3f43f rdf:value "Extracted definition from existing comment" .

_:genid-38640ccbd5eb49418600e8d7df2cf451-mor50bd147e3f3f4 rdf:value "Made subclass of geo:SpatialThing" .

_:genid-38640ccbd5eb49418600e8d7df2cf451-mor50bd147e3ef7f rdf:value "Added isDefinedBy property referring to FRBR core namespace" .

_:genid-38640ccbd5eb49418600e8d7df2cf451-mor50bd147e3efcc rdf:value "Added comment" .

_:genid-38640ccbd5eb49418600e8d7df2cf451-mor50bd147e3f065 rdf:value "Extracted definition from existing comment" .

_:genid-38640ccbd5eb49418600e8d7df2cf451-mor50bd147e3f019 rdf:value "Made subclass of skos:Concept" .

_:genid-38640ccbd5eb49418600e8d7df2cf451-mor50bd147e3f566 rdf:value "Added isDefinedBy property referring to FRBR core namespace" .

_:genid-38640ccbd5eb49418600e8d7df2cf451-mor50bd147e3f5b4 rdf:value "Added definition" .

_:genid-38640ccbd5eb49418600e8d7df2cf451-mor50bd147e3f622 rdf:value "Added isDefinedBy property referring to FRBR core namespace" .

_:genid-38640ccbd5eb49418600e8d7df2cf451-mor50bd147e3f66c rdf:value "Added definition" .

_:genid-38640ccbd5eb49418600e8d7df2cf451-mor50bd147e3f6da rdf:value "Added isDefinedBy property referring to FRBR core namespace" .

_:genid-38640ccbd5eb49418600e8d7df2cf451-mor50bd147e3f729 rdf:value "Added definition" .

_:genid-38640ccbd5eb49418600e8d7df2cf451-mor50bd147e3f797 rdf:value "Added isDefinedBy property referring to FRBR core namespace" .

_:genid-38640ccbd5eb49418600e8d7df2cf451-mor50bd147e3f7e2 rdf:value "Added definition" .

_:genid-38640ccbd5eb49418600e8d7df2cf451-mor50bd147e3f852 rdf:value "Added isDefinedBy property referring to FRBR core namespace" .

_:genid-38640ccbd5eb49418600e8d7df2cf451-mor50bd147e3f89d rdf:value "Added definition" .

_:genid-38640ccbd5eb49418600e8d7df2cf451-mor50bd147e3f90e rdf:value "Added isDefinedBy property referring to FRBR core namespace" .

_:genid-38640ccbd5eb49418600e8d7df2cf451-mor50bd147e3f95a rdf:value "Added definition" .

rdf:type rdfs:comment "The subject is an instance of a class." .

rdf:Property rdfs:comment "The class of RDF properties." .

rdfs:Class rdfs:comment "The class of classes." .

rdfs:Resource rdfs:comment "The class resource, everything." .

rdfs:subPropertyOf rdfs:comment "The subject is a subproperty of a property." .

rdfs:subClassOf rdfs:comment "The subject is a subclass of a class." .

rdfs:domain rdfs:comment "A domain of the subject property." .

rdfs:range rdfs:comment "A range of the subject property." .

rdf:subject rdfs:comment "The subject of the subject RDF statement." .

rdf:predicate rdfs:comment "The predicate of the subject RDF statement." .

rdf:object rdfs:comment "The object of the subject RDF statement." .

rdf:first rdfs:comment "The first item in the subject RDF list." .

rdf:rest rdfs:comment "The rest of the subject RDF list after the first item." .

rdf:value rdfs:comment "Idiomatic property used for structured values." .

rdf:nil rdfs:comment "The empty list, with no items in it. If the rest of a list is nil then the list has no more items in it." .

rdf:List rdfs:comment "The class of RDF Lists." .

rdf:Statement rdfs:comment "The class of RDF statements." .

rdfs:comment rdfs:comment "A description of the subject resource." .

rdfs:Literal rdfs:comment "The class of literal values, eg. textual strings and integers." .

rdfs:label rdfs:comment "A human-readable name for the subject." .

rdf:Alt rdfs:comment "The class of containers of alternatives." .

rdfs:Container rdfs:comment "The class of RDF containers." .

rdf:Bag rdfs:comment "The class of unordered containers." .

rdf:Seq rdfs:comment "The class of ordered containers." .

rdfs:ContainerMembershipProperty rdfs:comment """The class of container membership properties, rdf:_1, rdf:_2, ...,
                    all of which are sub-properties of 'member'.""" .

rdfs:isDefinedBy rdfs:comment "The defininition of the subject resource." .

rdfs:seeAlso rdfs:comment "Further information about the subject resource." .

rdf:XMLLiteral rdfs:comment "The class of XML literal values." .

rdfs:Datatype rdfs:comment "The class of RDF datatypes." .

dct:creator rdfs:comment "Examples of a Creator include a person, an organization, or a service. Typically, the name of a Creator should be used to indicate the entity."@en-us .

aac-ont:associatedPlace rdfs:comment "Associated places with a person or a cultural heritage."@en .

aac-ont:sitter rdfs:comment "The person depicted in an art work."@en .

aac-ont:objectId rdfs:comment "The internal identifier of a cultural heritage object."@en .

aac-ont:accessionNumber rdfs:comment "The identifier of a cultural heritage object in SAAM"@en .

foaf:Person rdfs:comment "A person." .

skos:altLabel rdfs:comment "Acronyms, abbreviations, spelling variants, and irregular plural/singular forms may be included among the alternative labels for a concept.  Mis-spelled terms are normally included as hidden labels (see skos:hiddenLabel)."@en,
    "The range of skos:altLabel is the class of RDF plain literals."@en, "skos:prefLabel, skos:altLabel and skos:hiddenLabel are pairwise disjoint properties."@en .

skos:hiddenLabel rdfs:comment "skos:prefLabel, skos:altLabel and skos:hiddenLabel are pairwise disjoint properties."@en,
    "The range of skos:hiddenLabel is the class of RDF plain literals."@en .

skos:prefLabel rdfs:comment "skos:prefLabel, skos:altLabel and skos:hiddenLabel are pairwise disjoint properties."@en,
    "No two concepts in the same concept scheme may have the same value for skos:prefLabel in a given language."@en,
    "The range of skos:prefLabel is the class of RDF plain literals."@en .

skos:broader rdfs:comment "Broader concepts are typically rendered as parents in a concept hierarchy (tree)."@en,
    "By convention, skos:broader is only used to assert an immediate (i.e. direct) hierarchical link between two conceptual resources."@en .

skos:mappingRelation rdfs:comment "These concept mapping relations mirror semantic relations, and the data model defined below is similar (with the exception of skos:exactMatch) to the data model defined for semantic relations. A distinct vocabulary is provided for concept mapping relations, to provide a convenient way to differentiate links within a concept scheme from links between concept schemes. However, this pattern of usage is not a formal requirement of the SKOS data model, and relies on informal definitions of best practice."@en .

skos:broaderTransitive rdfs:comment "By convention, skos:broaderTransitive is not used to make assertions. Rather, the properties can be used to draw inferences about the transitive closure of the hierarchical relation, which is useful e.g. when implementing a simple query expansion algorithm in a search application."@en .

skos:narrower rdfs:comment "By convention, skos:broader is only used to assert an immediate (i.e. direct) hierarchical link between two conceptual resources."@en,
    "Narrower concepts are typically rendered as children in a concept hierarchy (tree)."@en .

skos:narrowerTransitive rdfs:comment "By convention, skos:narrowerTransitive is not used to make assertions. Rather, the properties can be used to draw inferences about the transitive closure of the hierarchical relation, which is useful e.g. when implementing a simple query expansion algorithm in a search application."@en .

skos:semanticRelation rdfs:comment "This property should not be used directly, but as a super-property for all properties denoting a relationship of meaning between concepts."@en .

skos:note rdfs:comment "This property may be used directly, or as a super-property for more specific note types."@en .

skos:exactMatch rdfs:comment "skos:exactMatch is disjoint with each of the properties skos:broadMatch and skos:relatedMatch."@en .

skos:ConceptScheme rdfs:comment "A concept scheme may be defined to include concepts from different sources."@en,
    "Thesauri, classification schemes, subject heading lists, taxonomies, 'folksonomies', and other types of controlled vocabulary are all examples of concept schemes.  Concept schemes are also embedded in glossaries and terminologies."@en .

skos:inScheme rdfs:comment "A concept may be a member of more than one concept scheme."@en .

skos:Collection rdfs:comment "Labelled collections can be used with collectable semantic relation properties e.g. skos:narrower, where you would like a set of concepts to be displayed under a 'node label' in the hierarchy."@en .

skos:memberList rdfs:comment "For any resource, every item in the list given as the value of the skos:memberList property is also a value of the skos:member property."@en .

skos:OrderedCollection rdfs:comment "Ordered collections can be used with collectable semantic relation properties, where you would like a set of concepts to be displayed in a specific order, and optionally under a 'node label'."@en .

skos:related rdfs:comment "skos:related is disjoint with skos:broaderTransitive"@en .

skos:notation rdfs:comment "By convention, skos:notation is used with a typed literal in the object position of the triple."@en .

<http://americanart.si.edu/ontology/> rdfs:comment """
	====================================
	v5.0  change log  -- revised on 2012.11.29
	----------------
	1. A full revision to this ontology to make it compliant with EDM(Europeana Data Model) specifications.
	====================================
	
	====================================
	v5.1  change log  -- revised on 2012.12.3
	----------------
	1. Appending an identifier for http://americanart.si.edu/ontology/SAAMCHO and http://www.europeana.eu/schemas/edm/Agent.
	====================================
	
	====================================
	v5.2  change log  -- revised on 2012.12.4
	----------------
	1. Adding 'rdfs:range' constraints to property 'placeOfBirth' and 'placeOfDeath' in the rdaGr2 ontology.
	2. Define a new property 'associatedPlace' for the places associated with a saam-ont:SaamPerson .
	====================================
	  """@en .

dct:description rdfs:comment "Description may include but is not limited to: an abstract, a table of contents, a graphical representation, or a free-text account of the resource."@en-us .

saam-ont:constituentId rdfs:comment "The identical ID number of a constituent object in SAAM."@en .

saam-ont:objectId rdfs:comment "The identical ID of a collection object in SAAM."@en .

<http://www.europeana.eu/schemas/edm/> rdfs:comment """
=======
Changes between EDM-v53-120123.owl
and EDM-v52-100730.owl
=======
1. Update of formal specification to v5.2.3
2. Changed CRM namespace 
3. Added or changed formal axioms for Event, aggregatedCHO, currentLocation, hasMet, hasType, isAnnotationOf
4. Property labels upper-cased
5. Added language tags
6. Checked Martin's latest mappings to CRM
7. Added metadata on the owl:Ontology instance
=======
Remaining TODOs for EDM-v53-120123.owl
=======
- change FRBR namespace and mappings using http://metadataregistry.org/schema/show/id/5.html or FRBRoo
- add Martin's mapping to FRBR(oo) for edm:incorporates (equivalent to crm:R14F.incorporates) and edm:WebResource (subclass of F24 Publication Expression)
- try to capture formal cardinality constraints resulting from \"Obligation and Occurrence\" documentation, which should be attached to non-EDM constructs (esp. ore:Aggregation)
- continue adding documentation values (skos:scopeNote, skos:example, etc, according to 1.), starting from edm:InformationResource. Add all Europeana examples and rationale notes for non-EDM constructs
- keep specific EDM-doc properties for \"rationale\" and \"obligation and occurrence\". Use skos:definition for \"Europeana definition\", skos:example for \"Example\", skos:note for \"Europeana note\"
      """@en,
    "The present specification is based on the document \"Definition of the Europeana Data Model elements\", originally edited by Carlo Meghini. It is aligned with the version 5.2.3 of these EDM Definitions."@en .

dct:provenance rdfs:comment "The statement may include a description of any changes successive custodians made to the resource."@en-us .

ore:Aggregation rdfs:comment "A set of related resources (Aggregated Resources), grouped together such that the set can be treated as a single resource. This is the entity described within the ORE interoperability framework by a Resource Map." .

dct:isVersionOf rdfs:comment "Changes in version imply substantive changes in content rather than differences in format."@en-us .

ore:aggregates rdfs:comment "Aggregations, by definition, aggregate resources. The ore:aggregates relationship expresses that the object resource is a member of the set of Aggregated Resources of the subject (the Aggregation). This relationship between the Aggregation and its Aggregated Resources is thus more specific than a simple part/whole relationship, as expressed by dcterms:hasPart for example." .

ore:Proxy rdfs:comment "A Proxy represents an Aggregated Resource as it exists in a specific Aggregation. All assertions made about an entity are globally true, not only within the context of the Aggregation. As such, in order to make assertions which are only true of a resource as it exists in an Aggregation, a Proxy object is required. For example, one might want to cite an article as it appears in a specific journal, or assign aggregation-specific metadata to a Resource." .

ore:proxyFor rdfs:comment "Proxy objects are used to represent a Resource as it is aggregated in a particular Aggregation. The ore:proxyFor relationship is used to link the proxy to the Aggregated Resource it is a proxy for. The subject of the relationship is a Proxy object, and the object of the relationship is the Aggregated Resource." .

frbr_core:Event rdfs:comment "This class corresponds to the FRBR group three entity 'Event'."@en .

frbr_core:Expression rdfs:comment "This class corresponds to the FRBR group one entity 'Expression'."@en .

frbr_core:Manifestation rdfs:comment "This class corresponds to the FRBR group one entity 'Manifestation'."@en .

frbr_core:Place rdfs:comment "This class corresponds to the FRBR group three entity 'Place'."@en .

frbr_core:Work rdfs:comment "This class corresponds to the FRBR group one entity 'Work'."@en .

edm:language rdfs:comment """The recommended best practice is to use a controlled vocabulary such as
RFC 4646 (http://www.rfc-archive.org/getrfc.php?rfc=4646) which, in
conjunction with ISO 639, defines two- and three-letter primary language tags. Either a coded value or text string can be represented here."""@en .

<http://www.openarchives.org/ore/terms/> rdfs:comment "The set of terms provided by the OAI ORE initiative" .

dct:publisher rdfs:comment "Examples of a Publisher include a person, an organization, or a service. Typically, the name of a Publisher should be used to indicate the entity."@en-us .

ore:AggregatedResource rdfs:comment "A resource which is included in an Aggregation. Note that asserting that a resource is a member of the class of Aggregated Resources does not imply anything other than that it is aggregated by at least one Aggregation." .

ore:ResourceMap rdfs:comment "A description of an Aggregation according to the OAI-ORE data model. Resource Maps are serialised to a machine readable format according to the implementation guidelines." .

ore:isAggregatedBy rdfs:comment "The inverse relationship of ore:aggregates, ore:isAggregatedBy asserts that an Aggregated Resource is aggregated by an Aggregation." .

ore:describes rdfs:comment "This relationship asserts that the subject (a Resource Map) describes the object (an Aggregation)." .

ore:isDescribedBy rdfs:comment "The inverse relationship of ore:describes, in this case the object of the relationship is the Resource Map and the subject is the Aggregation which it describes." .

ore:lineage rdfs:comment "ore:lineage is a relationship between two Proxy objects, both of which MUST have the same Resource for which they are proxies. The meaning is that the Resource for which the subject of the relationship is a Proxy was discovered in the Aggregation in which the object Proxy's resource is aggregated." .

ore:proxyIn rdfs:comment "Proxy objects must link to the Aggregation in which the resource being proxied is aggregated. The ore:proxyIn relationship is used for this purpose. The subject of the relationship is a Proxy object, and the object of the relationship is the Aggregation." .

ore:similarTo rdfs:comment "The subject of this relationship MUST be an Aggregation.  This Aggregation should be considered an expression within the ORE context of the object of the relationship, as it is broadly equivalent to the resource. For example, the Aggregation may consist of the resources which, together, make up a journal article which has a DOI assigned to it. The Aggregation is not the article to which the DOI was assigned, but is a representation of it in some manner." .

foaf:Document rdfs:comment "A document." .

foaf:primaryTopic rdfs:comment "The primary topic of some page or document." .

<http://purl.org/vocab/frbr/core> rdfs:comment """
      This vocabulary is an expression in RDF of the concepts and relations described in the
      IFLA report on the Functional Requirements for Bibliographic Records (FRBR). 
    """@en,
    """
      This vocabulary is a work in progress, it includes RDF classes for the group 1, 2 and 3 entities
      described by the FRBR report and properties corresponding to the core relationships between
      those entities. It does not yet describe attributes of the entities. Where possible, appropriate 
      relationships with other vocabularies are included in order to place this vocabulary in the 
      context of existing RDF work.
    """@en .

foaf:topic rdfs:comment "A topic of some page or document." .

foaf:name rdfs:comment "A name for some thing." .

frbr_core:Endeavour rdfs:comment "This class represents any one of the FRBR group one entities."@en .

frbr_core:ResponsibleEntity rdfs:comment "This class represents any of the FRBR group two entities."@en .

frbr_core:Subject rdfs:comment "This class represents any of the FRBR group three entities."@en .

frbr_core:Item rdfs:comment "This class corresponds to the FRBR group one entity 'Item'."@en .

frbr_core:CorporateBody rdfs:comment "This class corresponds to the FRBR group two entity 'Corporate Body'."@en .

frbr_core:Person rdfs:comment "This class corresponds to the FRBR group two entity 'Person'."@en .

foaf:Organization rdfs:comment "An organization." .

foaf:Group rdfs:comment "A class of Agents." .

frbr_core:Object rdfs:comment "This class corresponds to the FRBR group three entity 'Object'."@en .

frbr_core:Concept rdfs:comment "This class corresponds to the FRBR group three entity 'Concept'."@en .

foaf:LabelProperty rdfs:comment "A foaf:LabelProperty is any RDF property with texual values that serve as labels." .

foaf:Agent rdfs:comment "An agent (eg. person, group, software or physical artifact)." .

foaf:Project rdfs:comment "A project (a collective endeavour of some kind)." .

dct:Agent rdfs:comment "Examples of Agent include person, organization, and software agent."@en-us .

foaf:Image rdfs:comment "An image." .

foaf:PersonalProfileDocument rdfs:comment "A personal profile RDF document." .

foaf:OnlineAccount rdfs:comment "An online account." .

foaf:OnlineGamingAccount rdfs:comment "An online gaming account." .

foaf:OnlineEcommerceAccount rdfs:comment "An online e-commerce account." .

foaf:OnlineChatAccount rdfs:comment "An online chat account." .

foaf:mbox rdfs:comment "A  personal mailbox, ie. an Internet mailbox associated with exactly one owner, the first owner of this mailbox. This is a 'static inverse functional property', in that  there is (across time and change) at most one individual that ever has any particular value for foaf:mbox." .

foaf:mbox_sha1sum rdfs:comment "The sha1sum of the URI of an Internet mailbox associated with exactly one owner, the  first owner of the mailbox." .

foaf:gender rdfs:comment "The gender of this Agent (typically but not necessarily 'male' or 'female')." .

foaf:geekcode rdfs:comment "A textual geekcode for this person, see http://www.geekcode.com/geek.html" .

foaf:dnaChecksum rdfs:comment "A checksum for the DNA of some thing. Joke." .

foaf:sha1 rdfs:comment "A sha1sum hash, in hex." .

foaf:based_near rdfs:comment "A location that something is based near, for some broadly human notion of near." .

foaf:title rdfs:comment "Title (Mr, Mrs, Ms, Dr. etc)" .

foaf:nick rdfs:comment "A short informal nickname characterising an agent (includes login identifiers, IRC and other chat nicknames)." .

foaf:jabberID rdfs:comment "A jabber ID for something." .

foaf:aimChatID rdfs:comment "An AIM chat ID" .

foaf:skypeID rdfs:comment "A Skype ID" .

foaf:icqChatID rdfs:comment "An ICQ chat ID" .

foaf:yahooChatID rdfs:comment "A Yahoo chat ID" .

foaf:msnChatID rdfs:comment "An MSN chat ID" .

foaf:firstName rdfs:comment "The first name of a person." .

foaf:lastName rdfs:comment "The last name of a person." .

foaf:givenName rdfs:comment "The given name of some person." .

foaf:givenname rdfs:comment "The given name of some person." .

foaf:surname rdfs:comment "The surname of some person." .

foaf:family_name rdfs:comment "The family name of some person." .

foaf:familyName rdfs:comment "The family name of some person." .

foaf:phone rdfs:comment "A phone,  specified using fully qualified tel: URI scheme (refs: http://www.w3.org/Addressing/schemes.html#tel)." .

foaf:homepage rdfs:comment "A homepage for some thing." .

foaf:page rdfs:comment "A page or document about this thing." .

foaf:isPrimaryTopicOf rdfs:comment "A document that this thing is the primary topic of." .

foaf:weblog rdfs:comment "A weblog of some thing (whether person, group, company etc.)." .

foaf:openid rdfs:comment "An OpenID for an Agent." .

foaf:tipjar rdfs:comment "A tipjar document for this agent, describing means for payment and reward." .

foaf:plan rdfs:comment "A .plan comment, in the tradition of finger and '.plan' files." .

foaf:made rdfs:comment "Something that was made by this agent." .

foaf:maker rdfs:comment "An agent that  made this thing." .

foaf:img rdfs:comment "An image that can be used to represent some thing (ie. those depictions which are particularly representative of something, eg. one's photo on a homepage)." .

foaf:depiction rdfs:comment "A depiction of some thing." .

foaf:depicts rdfs:comment "A thing depicted in this representation." .

foaf:thumbnail rdfs:comment "A derived thumbnail image." .

foaf:myersBriggs rdfs:comment "A Myers Briggs (MBTI) personality classification." .

foaf:workplaceHomepage rdfs:comment "A workplace homepage of some person; the homepage of an organization they work for." .

foaf:workInfoHomepage rdfs:comment "A work info homepage of some person; a page about their work for some organization." .

foaf:schoolHomepage rdfs:comment "A homepage of a school attended by the person." .

foaf:knows rdfs:comment "A person known by this person (indicating some level of reciprocated interaction between the parties)." .

foaf:interest rdfs:comment "A page about a topic of interest to this person." .

foaf:topic_interest rdfs:comment "A thing of interest to this person." .

foaf:publications rdfs:comment "A link to the publications of this person." .

foaf:currentProject rdfs:comment "A current project this person works on." .

foaf:pastProject rdfs:comment "A project this person has previously worked on." .

foaf:fundedBy rdfs:comment "An organization funding a project or person." .

foaf:logo rdfs:comment "A logo representing some thing." .

foaf:focus rdfs:comment "The underlying or 'focal' entity associated with some SKOS-described concept." .

foaf:theme rdfs:comment "A theme." .

foaf:account rdfs:comment "Indicates an account held by this agent." .

foaf:holdsAccount rdfs:comment "Indicates an account held by this agent." .

foaf:accountServiceHomepage rdfs:comment "Indicates a homepage of the service provide for this online account." .

foaf:accountName rdfs:comment "Indicates the name (identifier) associated with this online account." .

foaf:member rdfs:comment "Indicates a member of a Group" .

foaf:membershipClass rdfs:comment "Indicates the class of individuals that are a member of a Group" .

foaf:birthday rdfs:comment "The birthday of this Agent, represented in mm-dd string form, eg. '12-31'." .

foaf:age rdfs:comment "The age in years of some agent." .

foaf:status rdfs:comment "A string expressing what the user is happy for the general public (normally) to know about their current activity." .

<http://purl.org/NET/dc_owl2dl/terms> rdfs:comment "OWL 2 DL ontology for Dublin Core metadata terms from the http://purl.org/dc/terms/ namespace; this version is grounded in the DC elements ontology and only uses annotation properties."@en .

dct:accessRights rdfs:comment "Access Rights may include information regarding access or restrictions based on privacy, security, or other policies."@en-us .

dct:rights rdfs:comment "Typically, rights information includes a statement about various property rights associated with the resource, including intellectual property rights."@en-us .

dct:alternative rdfs:comment "The distinction between titles and alternative titles is application-specific."@en-us .

dct:AgentClass rdfs:comment "Examples of Agent Class include groups seen as classes, such as students, women, charities, lecturers."@en-us .

dct:date rdfs:comment "Date may be used to express temporal information at any level of granularity. Recommended best practice is to use an encoding scheme, such as the W3CDTF profile of ISO 8601 [W3CDTF]."@en-us .

dct:bibliographicCitation rdfs:comment "Recommended practice is to include sufficient bibliographic detail to identify the resource as unambiguously as possible."@en-us .

dct:identifier rdfs:comment "Recommended best practice is to identify the resource by means of a string conforming to a formal identification system."@en-us .

dct:relation rdfs:comment "Recommended best practice is to identify the related resource by means of a string conforming to a formal identification system."@en-us .

dct:contributor rdfs:comment "Examples of a Contributor include a person, an organization, or a service. Typically, the name of a Contributor should be used to indicate the entity."@en-us .

dct:coverage rdfs:comment "Spatial topic and spatial applicability may be a named place or a location specified by its geographic coordinates. Temporal topic may be a named period, date, or date range. A jurisdiction may be a named administrative entity or a geographic place to which the resource applies. Recommended best practice is to use a controlled vocabulary such as the Thesaurus of Geographic Names [TGN]. Where appropriate, named places or time periods can be used in preference to numeric identifiers such as sets of coordinates or date ranges."@en-us .

dct:dateAccepted rdfs:comment "Examples of resources to which a Date Accepted may be relevant are a thesis (accepted by a university department) or an article (accepted by a journal)."@en-us .

dct:dateSubmitted rdfs:comment "Examples of resources to which a Date Submitted may be relevant are a thesis (submitted to a university department) or an article (submitted to a journal)."@en-us .

dct:SizeOrDuration rdfs:comment "Examples include a number of pages, a specification of length, width, and breadth, or a period in hours, minutes, and seconds."@en-us .

dct:format rdfs:comment "Examples of dimensions include size and duration. Recommended best practice is to use a controlled vocabulary such as the list of Internet Media Types [MIME]."@en-us .

dct:instructionalMethod rdfs:comment "Instructional Method will typically include ways of presenting instructional materials or conducting instructional activities, patterns of learner-to-learner and learner-to-instructor interactions, and mechanisms by which group and individual levels of learning are measured. Instructional methods include all aspects of the instruction and learning processes from planning and implementation through evaluation and feedback."@en-us .

dct:language rdfs:comment "Recommended best practice is to use a controlled vocabulary such as RFC 4646 [RFC4646]."@en-us .

dct:LinguisticSystem rdfs:comment "Examples include written, spoken, sign, and computer languages."@en-us .

dct:mediator rdfs:comment "In an educational context, a mediator might be a parent, teacher, teaching assistant, or care-giver."@en-us .

dct:PhysicalMedium rdfs:comment "Examples include paper, canvas, or DVD."@en-us .

dct:source rdfs:comment "The described resource may be derived from the related resource in whole or in part. Recommended best practice is to identify the related resource by means of a string conforming to a formal identification system."@en-us .

dct:subject rdfs:comment "Typically, the subject will be represented using keywords, key phrases, or classification codes. Recommended best practice is to use a controlled vocabulary. To describe the spatial or temporal topic of the resource, use the Coverage element."@en-us .

dct:type rdfs:comment "Recommended best practice is to use a controlled vocabulary such as the DCMI Type Vocabulary [DCMITYPE]. To describe the file format, physical medium, or dimensions of the resource, use the Format element."@en-us .

dct:RFC3066 rdfs:comment "RFC 3066 has been obsoleted by RFC 4646."@en-us .

dct:RFC4646 rdfs:comment "RFC 4646 obsoletes RFC 3066."@en-us .

dct:FileFormat rdfs:comment "Examples include the formats defined by the list of Internet Media Types."@en-us .

rdfs:member rdfs:comment "A member of the subject resource." .

rdf:PlainLiteral rdfs:comment "The class of plain (i.e. untyped) literal values." .

rdf:type rdfs:label "type" .

rdf:Property rdfs:label "Property" .

rdfs:Class rdfs:label "Class" .

rdfs:Resource rdfs:label "Resource" .

rdfs:subPropertyOf rdfs:label "subPropertyOf" .

rdfs:subClassOf rdfs:label "subClassOf" .

rdfs:domain rdfs:label "domain" .

rdfs:range rdfs:label "range" .

rdf:subject rdfs:label "subject" .

rdf:predicate rdfs:label "predicate" .

rdf:object rdfs:label "object" .

rdf:first rdfs:label "first" .

rdf:rest rdfs:label "rest" .

rdf:value rdfs:label "value" .

rdf:nil rdfs:label "nil" .

rdf:List rdfs:label "List" .

rdf:Statement rdfs:label "Statement" .

rdfs:comment rdfs:label "comment" .

rdfs:Literal rdfs:label "Literal" .

rdfs:label rdfs:label "label" .

rdf:Alt rdfs:label "Alt" .

rdfs:Container rdfs:label "Container" .

rdf:Bag rdfs:label "Bag" .

rdf:Seq rdfs:label "Seq" .

rdfs:ContainerMembershipProperty rdfs:label "ContainerMembershipProperty" .

rdfs:isDefinedBy rdfs:label "isDefinedBy" .

rdfs:seeAlso rdfs:label "seeAlso" .

rdf:XMLLiteral rdfs:label "XMLLiteral" .

rdfs:Datatype rdfs:label "Datatype" .

dct:creator rdfs:label "Creator"@en-us .

edm:Agent rdfs:label "Agent"@en .

ElementsGr2:placeOfBirth rdfs:label "Place of birth"@en .

aac-ont:Person rdfs:label "An artist"@en .

aac-ont:associatedPlace rdfs:label "Associated places."@en .

ElementsGr2:placeOfDeath rdfs:label "Place of death"@en .

aac-ont:sitter rdfs:label "Sitter"@en .

aac-ont:CulturalHeritageObject rdfs:label "A cultural heritage object"@en .

edm:ProvidedCHO rdfs:label "Provided CHO"@en .

aac-ont:objectId rdfs:label "Object Id of a cultural heritage object."@en .

aac-ont:accessionNumber rdfs:label "Accession number of a cultural heritage object."@en .

skos:Concept rdfs:label "Concept"@en .

foaf:Person rdfs:label "Person" .

edm:Place rdfs:label "Place"@en .

skos:altLabel rdfs:label "alternative label"@en .

dct:issued rdfs:label "Date Issued"@en-us .

skos:definition rdfs:label "definition"@en .

skos:hiddenLabel rdfs:label "hidden label"@en .

skos:prefLabel rdfs:label "preferred label"@en .

skos:broadMatch rdfs:label "broader match"@en .

skos:broader rdfs:label "has broader"@en .

skos:mappingRelation rdfs:label "mapping relation"@en .

skos:broaderTransitive rdfs:label "broader transitive"@en .

skos:narrower rdfs:label "has narrower"@en .

skos:narrowerTransitive rdfs:label "narrower transitive"@en .

skos:semanticRelation rdfs:label "semantic relation"@en .

skos:changeNote rdfs:label "change note"@en .

skos:note rdfs:label "note"@en .

skos:closeMatch rdfs:label "exact match"@en .

skos:editorialNote rdfs:label "editorial note"@en .

skos:exactMatch rdfs:label "exact match"@en .

skos:example rdfs:label "example"@en .

skos:hasTopConcept rdfs:label "has top concept"@en .

skos:ConceptScheme rdfs:label "Concept Scheme"@en .

skos:historyNote rdfs:label "history note"@en .

skos:inScheme rdfs:label "in scheme"@en .

skos:member rdfs:label "member"@en .

skos:Collection rdfs:label "Collection"@en .

skos:memberList rdfs:label "member list"@en .

skos:OrderedCollection rdfs:label "Ordered Collection"@en .

skos:narrowMatch rdfs:label "narrower match"@en .

skos:related rdfs:label "related to"@en .

skos:relatedMatch rdfs:label "related match"@en .

skos:scopeNote rdfs:label "scope note"@en .

skos:topConceptOf rdfs:label "top concept in scheme"@en .

skos:notation rdfs:label "notation"@en .

dct:modified rdfs:label "Date Modified"@en-us .

dct:title rdfs:label "Title"@en-us .

dct:description rdfs:label "Description"@en-us .

saam-ont:constituentId rdfs:label "Id for a constituent."@en .

saam-ont:objectId rdfs:label "Id for a collection object."@en .

edm:year rdfs:label "Europeana Year"@en .

dct:temporal rdfs:label "Temporal Coverage"@en-us .

edm:dataProvider rdfs:label "Europeana Data Provider"@en .

dct:provenance rdfs:label "Provenance"@en-us .

ore:Aggregation rdfs:label "Aggregation" .

edm:country rdfs:label "Country"@en .

edm:userTag rdfs:label "User Tag"@en .

edm:hasMet rdfs:label "Has Met"@en .

edm:hasType rdfs:label "Has Type"@en .

edm:isRelatedTo rdfs:label "Is Related To"@en .

edm:isDerivativeOf rdfs:label "Is Derivative Of"@en .

dct:hasFormat rdfs:label "Has Format"@en-us .

dct:hasVersion rdfs:label "Has Version"@en-us .

dct:isFormatOf rdfs:label "Is Format Of"@en-us .

dct:isReplacedBy rdfs:label "Is Replaced By"@en-us .

dct:isVersionOf rdfs:label "Is Version Of"@en-us .

dct:replaces rdfs:label "Replaces"@en-us .

dct:spatial rdfs:label "Spatial Coverage"@en-us .

dct:tableOfContents rdfs:label "Table Of Contents"@en-us .

edm:hasView rdfs:label "Has View"@en .

edm:aggregatedCHO rdfs:label "Aggregated Cultural Heritage Object"@en .

ore:aggregates rdfs:label "Aggregates" .

edm:currentLocation rdfs:label "Current Location"@en .

ore:Proxy rdfs:label "Proxy" .

ore:proxyFor rdfs:label "Proxy For" .

edm:happenedAt rdfs:label "Happened At"@en .

edm:Event rdfs:label "Event"@en .

edm:NonInformationResource rdfs:label "Non-Information Resource"@en .

edm:WebResource rdfs:label "Web Resource"@en .

edm:incorporates rdfs:label "Incorporates"@en .

edm:isSimilarTo rdfs:label "Is Similar To"@en .

edm:isAnnotationOf rdfs:label "Is Annotation Of"@en .

edm:EuropeanaObject rdfs:label "Europeana Object"@en .

edm:isNextInSequence rdfs:label "Is Next In Sequence"@en .

edm:isRepresentationOf rdfs:label "Is Representation Of"@en .

edm:InformationResource rdfs:label "Information Resource"@en .

edm:isShownAt rdfs:label "Is Shown At"@en .

edm:landingPage rdfs:label "Landing Page"@en .

edm:isShownBy rdfs:label "Is Shown By"@en .

edm:isSuccessorOf rdfs:label "Is Successor Of"@en .

edm:object rdfs:label "Object"@en .

edm:occurredAt rdfs:label "Occured At"@en .

edm:TimeSpan rdfs:label "Time Span"@en .

edm:provider rdfs:label "Europeana Provider"@en .

edm:realizes rdfs:label "Realizes"@en .

edm:PhysicalThing rdfs:label "Physical Thing"@en .

edm:rights rdfs:label "Europeana Rights"@en .

edm:uri rdfs:label "Europeana URI"@en .

edm:wasPresentAt rdfs:label "Was Present At"@en .

edm:type rdfs:label "Europeana Type"@en .

edm:ugc rdfs:label "UGC"@en .

dct:PeriodOfTime rdfs:label "Period of Time"@en-us .

frbr_core:Event rdfs:label "event"@en .

frbr_core:Expression rdfs:label "expression"@en .

frbr_core:Manifestation rdfs:label "manifestation"@en .

frbr_core:Place rdfs:label "place"@en .

frbr_core:Work rdfs:label "work"@en .

edm:EuropeanaAggregation rdfs:label "Europeana Aggregation" .

edm:unstored rdfs:label "Unstored"@en .

edm:language rdfs:label "Europeana Language"@en .

<http://www.openarchives.org/ore/terms/> rdfs:label "The OAI ORE terms vocabulary" .

dct:publisher rdfs:label "Publisher"@en-us .

_:genid-38640ccbd5eb49418600e8d7df2cf451-mor50bd147e3f9c6 rdf:value "Added isDefinedBy property referring to FRBR core namespace" .

ore:AggregatedResource rdfs:label "Aggregated Resource" .

ore:ResourceMap rdfs:label "Resource Map" .

dct:hasPart rdfs:label "Has Part"@en-us .

ore:isAggregatedBy rdfs:label "Is Aggregated By" .

dct:isPartOf rdfs:label "Is Part Of"@en-us .

ore:describes rdfs:label "Describes" .

ore:isDescribedBy rdfs:label "Is Described By" .

ore:lineage rdfs:label "Lineage" .

ore:proxyIn rdfs:label "Proxy In" .

ore:similarTo rdfs:label "Similar To" .

ElementsGr2:addressOfTheCorporateBody rdfs:label "Address of the corporate body"@en .

ElementsGr2:addressOfThePerson rdfs:label "Address of the person"@en .

ElementsGr2:affiliation rdfs:label "Affiliation"@en .

ElementsGr2:associatedInstitution rdfs:label "Associated institution"@en .

ElementsGr2:biographicalInformation rdfs:label "Biographical information"@en .

ElementsGr2:corporateHistory rdfs:label "Corporate history"@en .

ElementsGr2:countryAssociatedWithThePerson rdfs:label "Country associated with the person"@en .

ElementsGr2:dateAssociatedWithTheCorporateBody rdfs:label "Date associated with the corporate body"@en .

ElementsGr2:dateOfEstablishment rdfs:label "Date of establishment"@en .

ElementsGr2:dateOfConferenceEtc rdfs:label "Date of conference, etc."@en .

ElementsGr2:dateOfTermination rdfs:label "Date of termination"@en .

ElementsGr2:dateAssociatedWithTheFamily rdfs:label "Date associated with the family"@en .

ElementsGr2:dateAssociatedWithThePerson rdfs:label "Date associated with the person"@en .

ElementsGr2:dateOfBirth rdfs:label "Date of birth"@en .

ElementsGr2:dateOfDeath rdfs:label "Date of death"@en .

ElementsGr2:periodOfActivityOfThePerson rdfs:label "Period of activity of the person"@en .

ElementsGr2:dateOfUsage rdfs:label "Date of usage"@en .

ElementsGr2:familyHistory rdfs:label "Family history"@en .

ElementsGr2:fieldOfActivityOfTheCorporateBody rdfs:label "Field of activity of the corporate body"@en .

ElementsGr2:fieldOfActivityOfThePerson rdfs:label "Field of activity of the person"@en .

ElementsGr2:fullerFormOfName rdfs:label "Fuller form of name"@en .

ElementsGr2:fullerFormOfNamePerson rdfs:label "Fuller form of name (Person)"@en .

ElementsGr2:gender rdfs:label "Gender"@en .

ElementsGr2:hereditaryTitle rdfs:label "Hereditary title"@en .

ElementsGr2:identifierForTheCorporateBody rdfs:label "Identifier for the corporate body"@en .

ElementsGr2:identifierForTheFamily rdfs:label "Identifier for the family"@en .

ElementsGr2:identifierForThePerson rdfs:label "Identifier for the person"@en .

ElementsGr2:languageOfTheCorporateBody rdfs:label "Language of the corporate body"@en .

ElementsGr2:languageOfThePerson rdfs:label "Language of the person"@en .

ElementsGr2:locationOfConferenceEtc rdfs:label "Location of conference, etc."@en .

ElementsGr2:placeAssociatedWithTheCorporateBody rdfs:label "Place associated with the corporate body"@en .

ElementsGr2:locationOfHeadquarters rdfs:label "Location of headquarters"@en .

ElementsGr2:name rdfs:label "Name"@en .

ElementsGr2:nameOfTheCorporateBody rdfs:label "Name of the corporate body"@en .

ElementsGr2:preferredNameForTheCorporateBody rdfs:label "Preferred name for the corporate body"@en .

ElementsGr2:variantNameForTheCorporateBody rdfs:label "Variant name for the corporate body"@en .

ElementsGr2:nameOfTheFamily rdfs:label "Name of the family"@en .

ElementsGr2:preferredNameForTheFamily rdfs:label "Preferred name for the family"@en .

ElementsGr2:variantNameForTheFamily rdfs:label "Variant name for the family"@en .

ElementsGr2:nameOfThePerson rdfs:label "Name of the person"@en .

ElementsGr2:preferredNameForThePerson rdfs:label "Preferred name for the person"@en .

ElementsGr2:variantNameForThePerson rdfs:label "Variant name for the person"@en .

ElementsGr2:note rdfs:label "Note"@en .

ElementsGr2:numberOfAConferenceEtc rdfs:label "Number of a conference, etc."@en .

ElementsGr2:otherDesignationAssociatedWithTheCorporateBody rdfs:label "Other designation associated with the corporate body"@en .

ElementsGr2:otherDesignationAssociatedWithThePerson rdfs:label "Other designation associated with the person"@en .

ElementsGr2:placeAssociatedWithTheFamily rdfs:label "Place associated with the family"@en .

ElementsGr2:placeOfResidence rdfs:label "Place of residence"@en .

ElementsGr2:professionOrOccupation rdfs:label "Profession or occupation"@en .

ElementsGr2:prominentMemberOfTheFamily rdfs:label "Prominent member of the family"@en .

ElementsGr2:scopeOfUsage rdfs:label "Scope of usage"@en .

ElementsGr2:titleOfThePerson rdfs:label "Title of the person"@en .

ElementsGr2:typeOfFamily rdfs:label "Type of family"@en .

ElementsGr2:undifferentiatedNameIndicator rdfs:label "Undifferentiated name indicator"@en .

ElementsGr2:undifferentiatedNameIndicatorPerson rdfs:label "Undifferentiated name indicator (Person)"@en .

ElementsGr2:undifferentiatedNameIndicatorCorporateBody rdfs:label "Undifferentiated name indicator (Corporate Body)"@en .

ElementsGr2:undifferentiatedNameIndicatorFamily rdfs:label "Undifferentiated name indicator (Family)"@en .

foaf:Document rdfs:label "Document" .

foaf:primaryTopic rdfs:label "primary topic" .

<http://vocab.org/frbr/core.html> rdfs:label "HTML" .

<http://vocab.org/frbr/core.json> rdfs:label "JSON" .

<http://vocab.org/frbr/core.turtle> rdfs:label "Turtle" .

foaf:topic rdfs:label "topic" .

_:genid-38640ccbd5eb49418600e8d7df2cf451-mor50bd147e3fa11 rdf:value "Added definition" .

_:genid-38640ccbd5eb49418600e8d7df2cf451-mor50bd147e3fc25 rdf:value "Added isDefinedBy property referring to FRBR core namespace" .

foaf:name rdfs:label "name" .

wgs84_pos:SpatialThing rdfs:label "Spatial Thing" .

dct:IMT rdfs:label "IMT"@en-us .

frbr_core:Endeavour rdfs:label "endeavour"@en .

frbr_core:ResponsibleEntity rdfs:label "responsible entity"@en .

frbr_core:Subject rdfs:label "subject"@en .

_:genid-38640ccbd5eb49418600e8d7df2cf451-mor50bd147e3fc70 rdf:value "Added definition" .

frbr_core:Item rdfs:label "item"@en .

_:genid-38640ccbd5eb49418600e8d7df2cf451-mor50bd147e3fcbc rdf:value "Added domain and range of Manifestation or Item" .

frbr_core:CorporateBody rdfs:label "corporate body"@en .

_:genid-38640ccbd5eb49418600e8d7df2cf451-mor50bd147e3fed1 rdf:value "Added isDefinedBy property referring to FRBR core namespace" .

frbr_core:Person rdfs:label "person"@en .

foaf:Organization rdfs:label "Organization" .

foaf:Group rdfs:label "Group" .

_:genid-38640ccbd5eb49418600e8d7df2cf451-mor50bd147e3ff1d rdf:value "Added definition" .

frbr_core:Object rdfs:label "object"@en .

frbr_core:Concept rdfs:label "concept"@en .

frbr_core:ClassicalWork rdfs:label "classical work"@en .

frbr_core:LegalWork rdfs:label "legal work"@en .

frbr_core:LiteraryWork rdfs:label "literary work"@en .

frbr_core:ScholarlyWork rdfs:label "scholarly work"@en .

frbr_core:Text rdfs:label "text"@en .

frbr_core:Image rdfs:label "image"@en .

frbr_core:Sound rdfs:label "sound"@en .

frbr_core:MovingImage rdfs:label "moving image"@en .

frbr_core:Data rdfs:label "data"@en .

frbr_core:Performance rdfs:label "performance"@en .

frbr_core:relatedEndeavour rdfs:label "related endeavour"@en .

frbr_core:realization rdfs:label "realization"@en .

frbr_core:realizationOf rdfs:label "realization of"@en .

frbr_core:embodiment rdfs:label "embodiment"@en .

frbr_core:embodimentOf rdfs:label "embodiment of"@en .

frbr_core:exemplar rdfs:label "exemplar"@en .

frbr_core:exemplarOf rdfs:label "exemplar of"@en .

frbr_core:reproduction rdfs:label "reproduction"@en .

frbr_core:reproductionOf rdfs:label "reproduction of"@en .

_:genid-38640ccbd5eb49418600e8d7df2cf451-mor50bd147e3ff6a rdf:value "Added domain and range of Manifestation or Item" .

_:genid-38640ccbd5eb49418600e8d7df2cf451-mor50bd147e40171 rdf:value "Added isDefinedBy property referring to FRBR core namespace" .

_:genid-38640ccbd5eb49418600e8d7df2cf451-mor50bd147e401bd rdf:value "Added definition" .

_:genid-38640ccbd5eb49418600e8d7df2cf451-mor50bd147e40209 rdf:value "Added domain and range of Work or Expression" .

frbr_core:successor rdfs:label "successor"@en .

frbr_core:successorOf rdfs:label "successor of"@en .

frbr_core:supplement rdfs:label "supplement"@en .

frbr_core:supplementOf rdfs:label "supplement of"@en .

frbr_core:complement rdfs:label "complement"@en .

frbr_core:complementOf rdfs:label "complement of"@en .

frbr_core:summarization rdfs:label "summarization"@en .

frbr_core:summarizationOf rdfs:label "summarization of"@en .

frbr_core:adaption rdfs:label "adaption"@en .

frbr_core:adaptionOf rdfs:label "adaption of"@en .

frbr_core:transformation rdfs:label "transformation"@en .

frbr_core:transformationOf rdfs:label "transformation of"@en .

frbr_core:imitation rdfs:label "imitation"@en .

frbr_core:imitationOf rdfs:label "imitation of"@en .

frbr_core:abridgement rdfs:label "abridgement"@en .

frbr_core:abridgementOf rdfs:label "abridgement of"@en .

frbr_core:revision rdfs:label "revision"@en .

frbr_core:revisionOf rdfs:label "revision of"@en .

frbr_core:translation rdfs:label "translation"@en .

frbr_core:translationOf rdfs:label "translation of"@en .

frbr_core:arrangement rdfs:label "arrangement"@en .

frbr_core:arrangementOf rdfs:label "arrangement of"@en .

frbr_core:alternate rdfs:label "alternate"@en .

frbr_core:alternateOf rdfs:label "alternate of"@en .

frbr_core:reconfiguration rdfs:label "reconfiguration"@en .

frbr_core:reconfigurationOf rdfs:label "reconfiguration of"@en .

frbr_core:part rdfs:label "part"@en .

frbr_core:partOf rdfs:label "part of"@en .

frbr_core:responsibleEntity rdfs:label "responsible entity"@en .

frbr_core:responsibleEntityOf rdfs:label "responsible entity of"@en .

frbr_core:creator rdfs:label "creator"@en .

frbr_core:creatorOf rdfs:label "creator of"@en .

frbr_core:realizer rdfs:label "realizer"@en .

frbr_core:realizerOf rdfs:label "realizer of"@en .

frbr_core:producer rdfs:label "producer"@en .

frbr_core:producerOf rdfs:label "producer of"@en .

frbr_core:owner rdfs:label "owner"@en .

frbr_core:ownerOf rdfs:label "owner of"@en .

frbr_core:subject rdfs:label "subject"@en .

foaf:LabelProperty rdfs:label "Label Property" .

foaf:Agent rdfs:label "Agent" .

<http://www.w3.org/2000/10/swap/pim/contact#Person> rdfs:label "Person" .

foaf:Project rdfs:label "Project" .

dct:Agent rdfs:label "Agent"@en-us .

foaf:Image rdfs:label "Image" .

foaf:PersonalProfileDocument rdfs:label "PersonalProfileDocument" .

foaf:OnlineAccount rdfs:label "Online Account" .

owl:Thing rdfs:label "Thing" .

foaf:OnlineGamingAccount rdfs:label "Online Gaming Account" .

foaf:OnlineEcommerceAccount rdfs:label "Online E-commerce Account" .

foaf:OnlineChatAccount rdfs:label "Online Chat Account" .

foaf:mbox rdfs:label "personal mailbox" .

foaf:mbox_sha1sum rdfs:label "sha1sum of a personal mailbox URI name" .

foaf:gender rdfs:label "gender" .

foaf:geekcode rdfs:label "geekcode" .

foaf:dnaChecksum rdfs:label "DNA checksum" .

foaf:sha1 rdfs:label "sha1sum (hex)" .

foaf:based_near rdfs:label "based near" .

foaf:title rdfs:label "title" .

foaf:nick rdfs:label "nickname" .

foaf:jabberID rdfs:label "jabber ID" .

foaf:aimChatID rdfs:label "AIM chat ID" .

foaf:skypeID rdfs:label "Skype ID" .

foaf:icqChatID rdfs:label "ICQ chat ID" .

foaf:yahooChatID rdfs:label "Yahoo chat ID" .

foaf:msnChatID rdfs:label "MSN chat ID" .

foaf:firstName rdfs:label "firstName" .

foaf:lastName rdfs:label "lastName" .

foaf:givenName rdfs:label "Given name" .

foaf:givenname rdfs:label "Given name" .

foaf:surname rdfs:label "Surname" .

foaf:family_name rdfs:label "family_name" .

foaf:familyName rdfs:label "familyName" .

foaf:phone rdfs:label "phone" .

foaf:homepage rdfs:label "homepage" .

foaf:page rdfs:label "page" .

foaf:isPrimaryTopicOf rdfs:label "is primary topic of" .

foaf:weblog rdfs:label "weblog" .

foaf:openid rdfs:label "openid" .

foaf:tipjar rdfs:label "tipjar" .

foaf:plan rdfs:label "plan" .

foaf:made rdfs:label "made" .

foaf:maker rdfs:label "maker" .

foaf:img rdfs:label "image" .

foaf:depiction rdfs:label "depiction" .

foaf:depicts rdfs:label "depicts" .

foaf:thumbnail rdfs:label "thumbnail" .

foaf:myersBriggs rdfs:label "myersBriggs" .

foaf:workplaceHomepage rdfs:label "workplace homepage" .

foaf:workInfoHomepage rdfs:label "work info homepage" .

foaf:schoolHomepage rdfs:label "schoolHomepage" .

foaf:knows rdfs:label "knows" .

foaf:interest rdfs:label "interest" .

foaf:topic_interest rdfs:label "topic_interest" .

foaf:publications rdfs:label "publications" .

foaf:currentProject rdfs:label "current project" .

foaf:pastProject rdfs:label "past project" .

foaf:fundedBy rdfs:label "funded by" .

foaf:logo rdfs:label "logo" .

foaf:focus rdfs:label "focus" .

<http://www.w3.org/2004/02/skos/core#Concept> rdfs:label "Concept" .

foaf:theme rdfs:label "theme" .

foaf:account rdfs:label "account" .

foaf:holdsAccount rdfs:label "account" .

foaf:accountServiceHomepage rdfs:label "account service homepage" .

foaf:accountName rdfs:label "account name" .

foaf:member rdfs:label "member" .

foaf:membershipClass rdfs:label "membershipClass" .

foaf:birthday rdfs:label "birthday" .

foaf:age rdfs:label "age" .

foaf:status rdfs:label "status" .

<http://purl.org/NET/dc_owl2dl/terms> rdfs:label "DCMI metadata terms"@en .

dct:license rdfs:label "License"@en-us .

dct:abstract rdfs:label "Abstract"@en-us .

dct:accessRights rdfs:label "Access Rights"@en-us .

dct:RightsStatement rdfs:label "Rights Statement"@en-us .

dct:rights rdfs:label "Rights"@en-us .

dct:accrualMethod rdfs:label "Accrual Method"@en-us .

dct:MethodOfAccrual rdfs:label "Method of Accrual"@en-us .

dct:accrualPeriodicity rdfs:label "Accrual Periodicity"@en-us .

dct:Frequency rdfs:label "Frequency"@en-us .

dct:accrualPolicy rdfs:label "Accrual Policy"@en-us .

dct:Policy rdfs:label "Policy"@en-us .

dct:alternative rdfs:label "Alternative Title"@en-us .

dct:audience rdfs:label "Audience"@en-us .

dct:AgentClass rdfs:label "Agent Class"@en-us .

dct:available rdfs:label "Date Available"@en-us .

dct:date rdfs:label "Date"@en-us .

dct:bibliographicCitation rdfs:label "Bibliographic Citation"@en-us .

dct:BibliographicResource rdfs:label "Bibliographic Resource"@en-us .

dct:identifier rdfs:label "Identifier"@en-us .

dct:conformsTo rdfs:label "Conforms To"@en-us .

dct:Standard rdfs:label "Standard"@en-us .

dct:relation rdfs:label "Relation"@en-us .

dct:contributor rdfs:label "Contributor"@en-us .

dct:coverage rdfs:label "Coverage"@en-us .

dct:LocationPeriodOrJurisdiction rdfs:label "Location, Period, or Jurisdiction"@en-us .

dct:created rdfs:label "Date Created"@en-us .

dct:dateAccepted rdfs:label "Date Accepted"@en-us .

dct:dateCopyrighted rdfs:label "Date Copyrighted"@en-us .

dct:dateSubmitted rdfs:label "Date Submitted"@en-us .

dct:educationLevel rdfs:label "Audience Education Level"@en-us .

dct:extent rdfs:label "Extent"@en-us .

dct:SizeOrDuration rdfs:label "Size or Duration"@en-us .

dct:format rdfs:label "Format"@en-us .

dct:MediaTypeOrExtent rdfs:label "Media Type or Extent"@en-us .

dct:instructionalMethod rdfs:label "Instructional Method"@en-us .

dct:MethodOfInstruction rdfs:label "Method of Instruction"@en-us .

dct:isReferencedBy rdfs:label "Is Referenced By"@en-us .

dct:isRequiredBy rdfs:label "Is Required By"@en-us .

dct:language rdfs:label "Language"@en-us .

dct:LinguisticSystem rdfs:label "Linguistic System"@en-us .

dct:LicenseDocument rdfs:label "License Document"@en-us .

dct:mediator rdfs:label "Mediator"@en-us .

dct:medium rdfs:label "Medium"@en-us .

dct:PhysicalResource rdfs:label "Physical Resource"@en-us .

dct:PhysicalMedium rdfs:label "Physical Medium"@en-us .

dct:ProvenanceStatement rdfs:label "Provenance Statement"@en-us .

dct:references rdfs:label "References"@en-us .

dct:requires rdfs:label "Requires"@en-us .

dct:rightsHolder rdfs:label "Rights Holder"@en-us .

dct:source rdfs:label "Source"@en-us .

dct:Location rdfs:label "Location"@en-us .

dct:subject rdfs:label "Subject"@en-us .

dct:type rdfs:label "Type"@en-us .

dct:valid rdfs:label "Date Valid"@en-us .

dct:DCMIType rdfs:label "DCMI Type Vocabulary"@en-us .

dct:DDC rdfs:label "DDC"@en-us .

dct:LCC rdfs:label "LCC"@en-us .

dct:LCSH rdfs:label "LCSH"@en-us .

dct:MESH rdfs:label "MeSH"@en-us .

dct:NLM rdfs:label "NLM"@en-us .

dct:TGN rdfs:label "TGN"@en-us .

dct:UDC rdfs:label "UDC"@en-us .

dct:Box rdfs:label "DCMI Box"@en-us .

dct:ISO3166 rdfs:label "ISO 3166"@en-us .

dct:ISO639-2 rdfs:label "ISO 639-2"@en-us .

dct:ISO639-3 rdfs:label "ISO 639-3"@en-us .

dct:Period rdfs:label "DCMI Period"@en-us .

dct:Point rdfs:label "DCMI Point"@en-us .

dct:RFC1766 rdfs:label "RFC 1766"@en-us .

dct:RFC3066 rdfs:label "RFC 3066"@en-us .

dct:RFC4646 rdfs:label "RFC 4646"@en-us .

dct:URI rdfs:label "URI"@en-us .

dct:W3CDTF rdfs:label "W3C-DTF"@en-us .

dct:FileFormat rdfs:label "File Format"@en-us .

dct:MediaType rdfs:label "Media Type"@en-us .

dct:Jurisdiction rdfs:label "Jurisdiction"@en-us .

rdfs:member rdfs:label "member" .

rdf:PlainLiteral rdfs:label "PlainLiteral" .

rdf:type rdfs:isDefinedBy <http://www.w3.org/1999/02/22-rdf-syntax-ns#> .

rdf:Property rdfs:isDefinedBy <http://www.w3.org/1999/02/22-rdf-syntax-ns#> .

rdfs:Class rdfs:isDefinedBy <http://www.w3.org/2000/01/rdf-schema#> .

rdfs:Resource rdfs:isDefinedBy <http://www.w3.org/2000/01/rdf-schema#> .

rdfs:subPropertyOf rdfs:isDefinedBy <http://www.w3.org/2000/01/rdf-schema#> .

rdfs:subClassOf rdfs:isDefinedBy <http://www.w3.org/2000/01/rdf-schema#> .

rdfs:domain rdfs:isDefinedBy <http://www.w3.org/2000/01/rdf-schema#> .

rdfs:range rdfs:isDefinedBy <http://www.w3.org/2000/01/rdf-schema#> .

rdf:subject rdfs:isDefinedBy <http://www.w3.org/1999/02/22-rdf-syntax-ns#> .

rdf:predicate rdfs:isDefinedBy <http://www.w3.org/1999/02/22-rdf-syntax-ns#> .

rdf:object rdfs:isDefinedBy <http://www.w3.org/1999/02/22-rdf-syntax-ns#> .

rdf:first rdfs:isDefinedBy <http://www.w3.org/1999/02/22-rdf-syntax-ns#> .

rdf:rest rdfs:isDefinedBy <http://www.w3.org/1999/02/22-rdf-syntax-ns#> .

rdf:value rdfs:isDefinedBy <http://www.w3.org/1999/02/22-rdf-syntax-ns#> .

rdf:nil rdfs:isDefinedBy <http://www.w3.org/1999/02/22-rdf-syntax-ns#> .

rdf:List rdfs:isDefinedBy <http://www.w3.org/1999/02/22-rdf-syntax-ns#> .

rdf:Statement rdfs:isDefinedBy <http://www.w3.org/1999/02/22-rdf-syntax-ns#> .

rdfs:comment rdfs:isDefinedBy <http://www.w3.org/2000/01/rdf-schema#> .

rdfs:Literal rdfs:isDefinedBy <http://www.w3.org/2000/01/rdf-schema#> .

rdfs:label rdfs:isDefinedBy <http://www.w3.org/2000/01/rdf-schema#> .

rdf:Alt rdfs:isDefinedBy <http://www.w3.org/1999/02/22-rdf-syntax-ns#> .

rdfs:Container rdfs:isDefinedBy <http://www.w3.org/2000/01/rdf-schema#> .

rdf:Bag rdfs:isDefinedBy <http://www.w3.org/1999/02/22-rdf-syntax-ns#> .

rdf:Seq rdfs:isDefinedBy <http://www.w3.org/1999/02/22-rdf-syntax-ns#> .

rdfs:ContainerMembershipProperty rdfs:isDefinedBy <http://www.w3.org/2000/01/rdf-schema#> .

rdfs:isDefinedBy rdfs:isDefinedBy <http://www.w3.org/2000/01/rdf-schema#> .

rdfs:seeAlso rdfs:isDefinedBy <http://www.w3.org/2000/01/rdf-schema#> .

rdf:XMLLiteral rdfs:isDefinedBy <http://www.w3.org/1999/02/22-rdf-syntax-ns#> .

rdfs:Datatype rdfs:isDefinedBy <http://www.w3.org/2000/01/rdf-schema#> .

ElementsGr2:placeOfBirth rdfs:isDefinedBy <http://rdvocab.info/ElementsGr2> .

ElementsGr2:placeOfDeath rdfs:isDefinedBy <http://rdvocab.info/ElementsGr2> .

skos:Concept rdfs:isDefinedBy <http://www.w3.org/2008/05/skos> .

foaf:Person rdfs:isDefinedBy <http://xmlns.com/foaf/0.1/> .

skos:altLabel rdfs:isDefinedBy <http://www.w3.org/2008/05/skos> .

skos:definition rdfs:isDefinedBy <http://www.w3.org/2008/05/skos> .

skos:hiddenLabel rdfs:isDefinedBy <http://www.w3.org/2008/05/skos> .

skos:prefLabel rdfs:isDefinedBy <http://www.w3.org/2008/05/skos> .

skos:broadMatch rdfs:isDefinedBy <http://www.w3.org/2008/05/skos> .

skos:broader rdfs:isDefinedBy <http://www.w3.org/2008/05/skos> .

skos:mappingRelation rdfs:isDefinedBy <http://www.w3.org/2008/05/skos> .

skos:broaderTransitive rdfs:isDefinedBy <http://www.w3.org/2008/05/skos> .

skos:narrower rdfs:isDefinedBy <http://www.w3.org/2008/05/skos> .

skos:narrowerTransitive rdfs:isDefinedBy <http://www.w3.org/2008/05/skos> .

skos:semanticRelation rdfs:isDefinedBy <http://www.w3.org/2008/05/skos> .

skos:changeNote rdfs:isDefinedBy <http://www.w3.org/2008/05/skos> .

skos:note rdfs:isDefinedBy <http://www.w3.org/2008/05/skos> .

skos:closeMatch rdfs:isDefinedBy <http://www.w3.org/2008/05/skos> .

skos:editorialNote rdfs:isDefinedBy <http://www.w3.org/2008/05/skos> .

skos:exactMatch rdfs:isDefinedBy <http://www.w3.org/2008/05/skos> .

skos:example rdfs:isDefinedBy <http://www.w3.org/2008/05/skos> .

skos:hasTopConcept rdfs:isDefinedBy <http://www.w3.org/2008/05/skos> .

skos:ConceptScheme rdfs:isDefinedBy <http://www.w3.org/2008/05/skos> .

skos:historyNote rdfs:isDefinedBy <http://www.w3.org/2008/05/skos> .

skos:inScheme rdfs:isDefinedBy <http://www.w3.org/2008/05/skos> .

skos:member rdfs:isDefinedBy <http://www.w3.org/2008/05/skos> .

skos:Collection rdfs:isDefinedBy <http://www.w3.org/2008/05/skos> .

skos:memberList rdfs:isDefinedBy <http://www.w3.org/2008/05/skos> .

skos:OrderedCollection rdfs:isDefinedBy <http://www.w3.org/2008/05/skos> .

skos:narrowMatch rdfs:isDefinedBy <http://www.w3.org/2008/05/skos> .

skos:related rdfs:isDefinedBy <http://www.w3.org/2008/05/skos> .

skos:relatedMatch rdfs:isDefinedBy <http://www.w3.org/2008/05/skos> .

skos:scopeNote rdfs:isDefinedBy <http://www.w3.org/2008/05/skos> .

skos:topConceptOf rdfs:isDefinedBy <http://www.w3.org/2008/05/skos> .

skos:notation rdfs:isDefinedBy <http://www.w3.org/2008/05/skos> .

ore:Aggregation rdfs:isDefinedBy <http://www.openarchives.org/ore/terms/> .

ore:aggregates rdfs:isDefinedBy <http://www.openarchives.org/ore/terms/> .

ore:Proxy rdfs:isDefinedBy <http://www.openarchives.org/ore/terms/> .

ore:proxyFor rdfs:isDefinedBy <http://www.openarchives.org/ore/terms/> .

frbr_core:Event rdfs:isDefinedBy <http://purl.org/vocab/frbr/core> .

frbr_core:Expression rdfs:isDefinedBy <http://purl.org/vocab/frbr/core> .

frbr_core:Manifestation rdfs:isDefinedBy <http://purl.org/vocab/frbr/core> .

frbr_core:Place rdfs:isDefinedBy <http://purl.org/vocab/frbr/core> .

frbr_core:Work rdfs:isDefinedBy <http://purl.org/vocab/frbr/core> .

ore:AggregatedResource rdfs:isDefinedBy <http://www.openarchives.org/ore/terms/> .

ore:ResourceMap rdfs:isDefinedBy <http://www.openarchives.org/ore/terms/> .

ore:isAggregatedBy rdfs:isDefinedBy <http://www.openarchives.org/ore/terms/> .

ore:describes rdfs:isDefinedBy <http://www.openarchives.org/ore/terms/> .

ore:isDescribedBy rdfs:isDefinedBy <http://www.openarchives.org/ore/terms/> .

ore:lineage rdfs:isDefinedBy <http://www.openarchives.org/ore/terms/> .

ore:proxyIn rdfs:isDefinedBy <http://www.openarchives.org/ore/terms/> .

ore:similarTo rdfs:isDefinedBy <http://www.openarchives.org/ore/terms/> .

ElementsGr2:addressOfTheCorporateBody rdfs:isDefinedBy <http://rdvocab.info/ElementsGr2> .

ElementsGr2:addressOfThePerson rdfs:isDefinedBy <http://rdvocab.info/ElementsGr2> .

ElementsGr2:affiliation rdfs:isDefinedBy <http://rdvocab.info/ElementsGr2> .

ElementsGr2:associatedInstitution rdfs:isDefinedBy <http://rdvocab.info/ElementsGr2> .

ElementsGr2:biographicalInformation rdfs:isDefinedBy <http://rdvocab.info/ElementsGr2> .

ElementsGr2:corporateHistory rdfs:isDefinedBy <http://rdvocab.info/ElementsGr2> .

ElementsGr2:countryAssociatedWithThePerson rdfs:isDefinedBy <http://rdvocab.info/ElementsGr2> .

ElementsGr2:dateAssociatedWithTheCorporateBody rdfs:isDefinedBy <http://rdvocab.info/ElementsGr2> .

ElementsGr2:dateOfEstablishment rdfs:isDefinedBy <http://rdvocab.info/ElementsGr2> .

ElementsGr2:dateOfConferenceEtc rdfs:isDefinedBy <http://rdvocab.info/ElementsGr2> .

ElementsGr2:dateOfTermination rdfs:isDefinedBy <http://rdvocab.info/ElementsGr2> .

ElementsGr2:dateAssociatedWithTheFamily rdfs:isDefinedBy <http://rdvocab.info/ElementsGr2> .

ElementsGr2:dateAssociatedWithThePerson rdfs:isDefinedBy <http://rdvocab.info/ElementsGr2> .

ElementsGr2:dateOfBirth rdfs:isDefinedBy <http://rdvocab.info/ElementsGr2> .

ElementsGr2:dateOfDeath rdfs:isDefinedBy <http://rdvocab.info/ElementsGr2> .

ElementsGr2:periodOfActivityOfThePerson rdfs:isDefinedBy <http://rdvocab.info/ElementsGr2> .

ElementsGr2:dateOfUsage rdfs:isDefinedBy <http://rdvocab.info/ElementsGr2> .

ElementsGr2:familyHistory rdfs:isDefinedBy <http://rdvocab.info/ElementsGr2> .

ElementsGr2:fieldOfActivityOfTheCorporateBody rdfs:isDefinedBy <http://rdvocab.info/ElementsGr2> .

ElementsGr2:fieldOfActivityOfThePerson rdfs:isDefinedBy <http://rdvocab.info/ElementsGr2> .

ElementsGr2:fullerFormOfName rdfs:isDefinedBy <http://rdvocab.info/ElementsGr2> .

ElementsGr2:fullerFormOfNamePerson rdfs:isDefinedBy <http://rdvocab.info/ElementsGr2> .

ElementsGr2:gender rdfs:isDefinedBy <http://rdvocab.info/ElementsGr2> .

ElementsGr2:hereditaryTitle rdfs:isDefinedBy <http://rdvocab.info/ElementsGr2> .

ElementsGr2:identifierForTheCorporateBody rdfs:isDefinedBy <http://rdvocab.info/ElementsGr2> .

ElementsGr2:identifierForTheFamily rdfs:isDefinedBy <http://rdvocab.info/ElementsGr2> .

ElementsGr2:identifierForThePerson rdfs:isDefinedBy <http://rdvocab.info/ElementsGr2> .

ElementsGr2:languageOfTheCorporateBody rdfs:isDefinedBy <http://rdvocab.info/ElementsGr2> .

ElementsGr2:languageOfThePerson rdfs:isDefinedBy <http://rdvocab.info/ElementsGr2> .

ElementsGr2:locationOfConferenceEtc rdfs:isDefinedBy <http://rdvocab.info/ElementsGr2> .

ElementsGr2:placeAssociatedWithTheCorporateBody rdfs:isDefinedBy <http://rdvocab.info/ElementsGr2> .

ElementsGr2:locationOfHeadquarters rdfs:isDefinedBy <http://rdvocab.info/ElementsGr2> .

ElementsGr2:name rdfs:isDefinedBy <http://rdvocab.info/ElementsGr2> .

ElementsGr2:nameOfTheCorporateBody rdfs:isDefinedBy <http://rdvocab.info/ElementsGr2> .

ElementsGr2:preferredNameForTheCorporateBody rdfs:isDefinedBy <http://rdvocab.info/ElementsGr2> .

ElementsGr2:variantNameForTheCorporateBody rdfs:isDefinedBy <http://rdvocab.info/ElementsGr2> .

ElementsGr2:nameOfTheFamily rdfs:isDefinedBy <http://rdvocab.info/ElementsGr2> .

ElementsGr2:preferredNameForTheFamily rdfs:isDefinedBy <http://rdvocab.info/ElementsGr2> .

ElementsGr2:variantNameForTheFamily rdfs:isDefinedBy <http://rdvocab.info/ElementsGr2> .

ElementsGr2:nameOfThePerson rdfs:isDefinedBy <http://rdvocab.info/ElementsGr2> .

ElementsGr2:preferredNameForThePerson rdfs:isDefinedBy <http://rdvocab.info/ElementsGr2> .

ElementsGr2:variantNameForThePerson rdfs:isDefinedBy <http://rdvocab.info/ElementsGr2> .

ElementsGr2:note rdfs:isDefinedBy <http://rdvocab.info/ElementsGr2> .

ElementsGr2:numberOfAConferenceEtc rdfs:isDefinedBy <http://rdvocab.info/ElementsGr2> .

ElementsGr2:otherDesignationAssociatedWithTheCorporateBody rdfs:isDefinedBy <http://rdvocab.info/ElementsGr2> .

ElementsGr2:otherDesignationAssociatedWithThePerson rdfs:isDefinedBy <http://rdvocab.info/ElementsGr2> .

ElementsGr2:placeAssociatedWithTheFamily rdfs:isDefinedBy <http://rdvocab.info/ElementsGr2> .

ElementsGr2:placeOfResidence rdfs:isDefinedBy <http://rdvocab.info/ElementsGr2> .

ElementsGr2:professionOrOccupation rdfs:isDefinedBy <http://rdvocab.info/ElementsGr2> .

ElementsGr2:prominentMemberOfTheFamily rdfs:isDefinedBy <http://rdvocab.info/ElementsGr2> .

ElementsGr2:scopeOfUsage rdfs:isDefinedBy <http://rdvocab.info/ElementsGr2> .

ElementsGr2:titleOfThePerson rdfs:isDefinedBy <http://rdvocab.info/ElementsGr2> .

ElementsGr2:typeOfFamily rdfs:isDefinedBy <http://rdvocab.info/ElementsGr2> .

ElementsGr2:undifferentiatedNameIndicator rdfs:isDefinedBy <http://rdvocab.info/ElementsGr2> .

ElementsGr2:undifferentiatedNameIndicatorPerson rdfs:isDefinedBy <http://rdvocab.info/ElementsGr2> .

ElementsGr2:undifferentiatedNameIndicatorCorporateBody rdfs:isDefinedBy <http://rdvocab.info/ElementsGr2> .

ElementsGr2:undifferentiatedNameIndicatorFamily rdfs:isDefinedBy <http://rdvocab.info/ElementsGr2> .

foaf:Document rdfs:isDefinedBy <http://xmlns.com/foaf/0.1/> .

foaf:primaryTopic rdfs:isDefinedBy <http://xmlns.com/foaf/0.1/> .

foaf:topic rdfs:isDefinedBy <http://xmlns.com/foaf/0.1/> .

foaf:name rdfs:isDefinedBy <http://xmlns.com/foaf/0.1/> .

dct:IMT rdfs:isDefinedBy <http://www.iana.org/assignments/media-types/> .

frbr_core:Endeavour rdfs:isDefinedBy <http://purl.org/vocab/frbr/core> .

frbr_core:ResponsibleEntity rdfs:isDefinedBy <http://purl.org/vocab/frbr/core> .

frbr_core:Subject rdfs:isDefinedBy <http://purl.org/vocab/frbr/core> .

frbr_core:Item rdfs:isDefinedBy <http://purl.org/vocab/frbr/core> .

frbr_core:CorporateBody rdfs:isDefinedBy <http://purl.org/vocab/frbr/core> .

frbr_core:Person rdfs:isDefinedBy <http://purl.org/vocab/frbr/core> .

foaf:Organization rdfs:isDefinedBy <http://xmlns.com/foaf/0.1/> .

frbr_core:Object rdfs:isDefinedBy <http://purl.org/vocab/frbr/core> .

frbr_core:Concept rdfs:isDefinedBy <http://purl.org/vocab/frbr/core> .

frbr_core:ClassicalWork rdfs:isDefinedBy <http://purl.org/vocab/frbr/core> .

frbr_core:LegalWork rdfs:isDefinedBy <http://purl.org/vocab/frbr/core> .

frbr_core:LiteraryWork rdfs:isDefinedBy <http://purl.org/vocab/frbr/core> .

frbr_core:ScholarlyWork rdfs:isDefinedBy <http://purl.org/vocab/frbr/core> .

frbr_core:Text rdfs:isDefinedBy <http://purl.org/vocab/frbr/core> .

frbr_core:Image rdfs:isDefinedBy <http://purl.org/vocab/frbr/core> .

frbr_core:Sound rdfs:isDefinedBy <http://purl.org/vocab/frbr/core> .

frbr_core:MovingImage rdfs:isDefinedBy <http://purl.org/vocab/frbr/core> .

frbr_core:Data rdfs:isDefinedBy <http://purl.org/vocab/frbr/core> .

frbr_core:Performance rdfs:isDefinedBy <http://purl.org/vocab/frbr/core> .

frbr_core:relatedEndeavour rdfs:isDefinedBy <http://purl.org/vocab/frbr/core> .

frbr_core:realization rdfs:isDefinedBy <http://purl.org/vocab/frbr/core> .

frbr_core:realizationOf rdfs:isDefinedBy <http://purl.org/vocab/frbr/core> .

frbr_core:embodiment rdfs:isDefinedBy <http://purl.org/vocab/frbr/core> .

frbr_core:embodimentOf rdfs:isDefinedBy <http://purl.org/vocab/frbr/core> .

frbr_core:exemplar rdfs:isDefinedBy <http://purl.org/vocab/frbr/core> .

frbr_core:exemplarOf rdfs:isDefinedBy <http://purl.org/vocab/frbr/core> .

frbr_core:reproduction rdfs:isDefinedBy <http://purl.org/vocab/frbr/core> .

frbr_core:reproductionOf rdfs:isDefinedBy <http://purl.org/vocab/frbr/core> .

frbr_core:successor rdfs:isDefinedBy <http://purl.org/vocab/frbr/core> .

frbr_core:successorOf rdfs:isDefinedBy <http://purl.org/vocab/frbr/core> .

frbr_core:supplement rdfs:isDefinedBy <http://purl.org/vocab/frbr/core> .

frbr_core:supplementOf rdfs:isDefinedBy <http://purl.org/vocab/frbr/core> .

frbr_core:complement rdfs:isDefinedBy <http://purl.org/vocab/frbr/core> .

frbr_core:complementOf rdfs:isDefinedBy <http://purl.org/vocab/frbr/core> .

frbr_core:summarization rdfs:isDefinedBy <http://purl.org/vocab/frbr/core> .

frbr_core:summarizationOf rdfs:isDefinedBy <http://purl.org/vocab/frbr/core> .

frbr_core:adaption rdfs:isDefinedBy <http://purl.org/vocab/frbr/core> .

frbr_core:adaptionOf rdfs:isDefinedBy <http://purl.org/vocab/frbr/core> .

frbr_core:transformation rdfs:isDefinedBy <http://purl.org/vocab/frbr/core> .

frbr_core:transformationOf rdfs:isDefinedBy <http://purl.org/vocab/frbr/core> .

frbr_core:imitation rdfs:isDefinedBy <http://purl.org/vocab/frbr/core> .

frbr_core:imitationOf rdfs:isDefinedBy <http://purl.org/vocab/frbr/core> .

frbr_core:abridgement rdfs:isDefinedBy <http://purl.org/vocab/frbr/core> .

frbr_core:abridgementOf rdfs:isDefinedBy <http://purl.org/vocab/frbr/core> .

frbr_core:revision rdfs:isDefinedBy <http://purl.org/vocab/frbr/core> .

frbr_core:revisionOf rdfs:isDefinedBy <http://purl.org/vocab/frbr/core> .

frbr_core:translation rdfs:isDefinedBy <http://purl.org/vocab/frbr/core> .

frbr_core:translationOf rdfs:isDefinedBy <http://purl.org/vocab/frbr/core> .

frbr_core:arrangement rdfs:isDefinedBy <http://purl.org/vocab/frbr/core> .

frbr_core:arrangementOf rdfs:isDefinedBy <http://purl.org/vocab/frbr/core> .

frbr_core:alternate rdfs:isDefinedBy <http://purl.org/vocab/frbr/core> .

frbr_core:alternateOf rdfs:isDefinedBy <http://purl.org/vocab/frbr/core> .

frbr_core:reconfiguration rdfs:isDefinedBy <http://purl.org/vocab/frbr/core> .

frbr_core:reconfigurationOf rdfs:isDefinedBy <http://purl.org/vocab/frbr/core> .

frbr_core:part rdfs:isDefinedBy <http://purl.org/vocab/frbr/core> .

frbr_core:partOf rdfs:isDefinedBy <http://purl.org/vocab/frbr/core> .

frbr_core:responsibleEntity rdfs:isDefinedBy <http://purl.org/vocab/frbr/core> .

frbr_core:responsibleEntityOf rdfs:isDefinedBy <http://purl.org/vocab/frbr/core> .

frbr_core:creator rdfs:isDefinedBy <http://purl.org/vocab/frbr/core> .

frbr_core:creatorOf rdfs:isDefinedBy <http://purl.org/vocab/frbr/core> .

frbr_core:realizer rdfs:isDefinedBy <http://purl.org/vocab/frbr/core> .

frbr_core:realizerOf rdfs:isDefinedBy <http://purl.org/vocab/frbr/core> .

frbr_core:producer rdfs:isDefinedBy <http://purl.org/vocab/frbr/core> .

frbr_core:producerOf rdfs:isDefinedBy <http://purl.org/vocab/frbr/core> .

frbr_core:owner rdfs:isDefinedBy <http://purl.org/vocab/frbr/core> .

frbr_core:ownerOf rdfs:isDefinedBy <http://purl.org/vocab/frbr/core> .

frbr_core:subject rdfs:isDefinedBy <http://purl.org/vocab/frbr/core> .

foaf:LabelProperty rdfs:isDefinedBy <http://xmlns.com/foaf/0.1/> .

foaf:Project rdfs:isDefinedBy <http://xmlns.com/foaf/0.1/> .

foaf:Image rdfs:isDefinedBy <http://xmlns.com/foaf/0.1/> .

foaf:OnlineAccount rdfs:isDefinedBy <http://xmlns.com/foaf/0.1/> .

foaf:OnlineGamingAccount rdfs:isDefinedBy <http://xmlns.com/foaf/0.1/> .

foaf:OnlineEcommerceAccount rdfs:isDefinedBy <http://xmlns.com/foaf/0.1/> .

foaf:OnlineChatAccount rdfs:isDefinedBy <http://xmlns.com/foaf/0.1/> .

foaf:mbox rdfs:isDefinedBy <http://xmlns.com/foaf/0.1/> .

foaf:mbox_sha1sum rdfs:isDefinedBy <http://xmlns.com/foaf/0.1/> .

foaf:gender rdfs:isDefinedBy <http://xmlns.com/foaf/0.1/> .

foaf:geekcode rdfs:isDefinedBy <http://xmlns.com/foaf/0.1/> .

foaf:dnaChecksum rdfs:isDefinedBy <http://xmlns.com/foaf/0.1/> .

foaf:sha1 rdfs:isDefinedBy <http://xmlns.com/foaf/0.1/> .

foaf:based_near rdfs:isDefinedBy <http://xmlns.com/foaf/0.1/> .

foaf:title rdfs:isDefinedBy <http://xmlns.com/foaf/0.1/> .

foaf:nick rdfs:isDefinedBy <http://xmlns.com/foaf/0.1/> .

foaf:jabberID rdfs:isDefinedBy <http://xmlns.com/foaf/0.1/> .

foaf:aimChatID rdfs:isDefinedBy <http://xmlns.com/foaf/0.1/> .

foaf:skypeID rdfs:isDefinedBy <http://xmlns.com/foaf/0.1/> .

foaf:icqChatID rdfs:isDefinedBy <http://xmlns.com/foaf/0.1/> .

foaf:yahooChatID rdfs:isDefinedBy <http://xmlns.com/foaf/0.1/> .

foaf:msnChatID rdfs:isDefinedBy <http://xmlns.com/foaf/0.1/> .

foaf:firstName rdfs:isDefinedBy <http://xmlns.com/foaf/0.1/> .

foaf:lastName rdfs:isDefinedBy <http://xmlns.com/foaf/0.1/> .

foaf:givenName rdfs:isDefinedBy <http://xmlns.com/foaf/0.1/> .

foaf:givenname rdfs:isDefinedBy <http://xmlns.com/foaf/0.1/> .

foaf:surname rdfs:isDefinedBy <http://xmlns.com/foaf/0.1/> .

foaf:family_name rdfs:isDefinedBy <http://xmlns.com/foaf/0.1/> .

foaf:familyName rdfs:isDefinedBy <http://xmlns.com/foaf/0.1/> .

foaf:phone rdfs:isDefinedBy <http://xmlns.com/foaf/0.1/> .

foaf:homepage rdfs:isDefinedBy <http://xmlns.com/foaf/0.1/> .

foaf:page rdfs:isDefinedBy <http://xmlns.com/foaf/0.1/> .

foaf:isPrimaryTopicOf rdfs:isDefinedBy <http://xmlns.com/foaf/0.1/> .

foaf:weblog rdfs:isDefinedBy <http://xmlns.com/foaf/0.1/> .

foaf:openid rdfs:isDefinedBy <http://xmlns.com/foaf/0.1/> .

foaf:tipjar rdfs:isDefinedBy <http://xmlns.com/foaf/0.1/> .

foaf:plan rdfs:isDefinedBy <http://xmlns.com/foaf/0.1/> .

foaf:made rdfs:isDefinedBy <http://xmlns.com/foaf/0.1/> .

foaf:maker rdfs:isDefinedBy <http://xmlns.com/foaf/0.1/> .

foaf:img rdfs:isDefinedBy <http://xmlns.com/foaf/0.1/> .

foaf:depiction rdfs:isDefinedBy <http://xmlns.com/foaf/0.1/> .

foaf:depicts rdfs:isDefinedBy <http://xmlns.com/foaf/0.1/> .

foaf:thumbnail rdfs:isDefinedBy <http://xmlns.com/foaf/0.1/> .

foaf:myersBriggs rdfs:isDefinedBy <http://xmlns.com/foaf/0.1/> .

foaf:workplaceHomepage rdfs:isDefinedBy <http://xmlns.com/foaf/0.1/> .

foaf:workInfoHomepage rdfs:isDefinedBy <http://xmlns.com/foaf/0.1/> .

foaf:schoolHomepage rdfs:isDefinedBy <http://xmlns.com/foaf/0.1/> .

foaf:knows rdfs:isDefinedBy <http://xmlns.com/foaf/0.1/> .

foaf:interest rdfs:isDefinedBy <http://xmlns.com/foaf/0.1/> .

foaf:topic_interest rdfs:isDefinedBy <http://xmlns.com/foaf/0.1/> .

foaf:publications rdfs:isDefinedBy <http://xmlns.com/foaf/0.1/> .

foaf:currentProject rdfs:isDefinedBy <http://xmlns.com/foaf/0.1/> .

foaf:pastProject rdfs:isDefinedBy <http://xmlns.com/foaf/0.1/> .

foaf:fundedBy rdfs:isDefinedBy <http://xmlns.com/foaf/0.1/> .

foaf:logo rdfs:isDefinedBy <http://xmlns.com/foaf/0.1/> .

foaf:focus rdfs:isDefinedBy <http://xmlns.com/foaf/0.1/> .

foaf:theme rdfs:isDefinedBy <http://xmlns.com/foaf/0.1/> .

foaf:account rdfs:isDefinedBy <http://xmlns.com/foaf/0.1/> .

foaf:holdsAccount rdfs:isDefinedBy <http://xmlns.com/foaf/0.1/> .

foaf:accountServiceHomepage rdfs:isDefinedBy <http://xmlns.com/foaf/0.1/> .

foaf:accountName rdfs:isDefinedBy <http://xmlns.com/foaf/0.1/> .

foaf:member rdfs:isDefinedBy <http://xmlns.com/foaf/0.1/> .

foaf:membershipClass rdfs:isDefinedBy <http://xmlns.com/foaf/0.1/> .

foaf:birthday rdfs:isDefinedBy <http://xmlns.com/foaf/0.1/> .

foaf:age rdfs:isDefinedBy <http://xmlns.com/foaf/0.1/> .

foaf:status rdfs:isDefinedBy <http://xmlns.com/foaf/0.1/> .

dct:DCMIType rdfs:isDefinedBy <http://dublincore.org/documents/dcmi-type-vocabulary/> .

dct:DDC rdfs:isDefinedBy <http://www.oclc.org/dewey/> .

dct:LCC rdfs:isDefinedBy <http://lcweb.loc.gov/catdir/cpso/lcco/lcco.html> .

dct:MESH rdfs:isDefinedBy <http://www.nlm.nih.gov/mesh/meshhome.html> .

dct:NLM rdfs:isDefinedBy <http://wwwcf.nlm.nih.gov/class/> .

dct:TGN rdfs:isDefinedBy <http://www.getty.edu/research/tools/vocabulary/tgn/index.html> .

dct:UDC rdfs:isDefinedBy <http://www.udcc.org/> .

dct:Box rdfs:isDefinedBy <http://dublincore.org/documents/dcmi-box/> .

dct:ISO3166 rdfs:isDefinedBy <http://www.iso.org/iso/en/prods-services/iso3166ma/02iso-3166-code-lists/list-en1.html> .

dct:ISO639-2 rdfs:isDefinedBy <http://lcweb.loc.gov/standards/iso639-2/langhome.html> .

dct:ISO639-3 rdfs:isDefinedBy <http://www.sil.org/iso639-3/> .

dct:Period rdfs:isDefinedBy <http://dublincore.org/documents/dcmi-period/> .

dct:Point rdfs:isDefinedBy <http://dublincore.org/documents/dcmi-point/> .

dct:RFC1766 rdfs:isDefinedBy <http://www.ietf.org/rfc/rfc1766.txt> .

dct:RFC3066 rdfs:isDefinedBy <http://www.ietf.org/rfc/rfc3066.txt> .

dct:RFC4646 rdfs:isDefinedBy <http://www.ietf.org/rfc/rfc4646.txt> .

dct:URI rdfs:isDefinedBy <http://www.ietf.org/rfc/rfc3986.txt> .

dct:W3CDTF rdfs:isDefinedBy <http://www.w3.org/TR/NOTE-datetime> .

rdfs:member rdfs:isDefinedBy <http://www.w3.org/2000/01/rdf-schema#> .

rdf:PlainLiteral rdfs:isDefinedBy <http://www.w3.org/TR/rdf-plain-literal/> .

<http://www.europeana.eu/schemas/edm/> rdfs:seeAlso <http://europeanalabs.eu/wiki/EDMPrototypingTask11>,
    <http://pro.europeana.eu/edm-documentation> .

<http://www.openarchives.org/ore/terms/> rdfs:seeAlso <http://www.openarchives.org/ore/toc> .

dct:date rdfs:seeAlso <http://www.w3.org/TR/NOTE-datetime> .

dct:coverage rdfs:seeAlso <http://www.getty.edu/research/tools/vocabulary/tgn/index.html> .

dct:format rdfs:seeAlso <http://www.iana.org/assignments/media-types/> .

dct:language rdfs:seeAlso <http://www.ietf.org/rfc/rfc4646.txt> .

dct:type rdfs:seeAlso <http://dublincore.org/documents/dcmi-type-vocabulary/> .

<http://www.w3.org/2000/01/rdf-schema#> rdfs:seeAlso <http://www.w3.org/2000/01/rdf-schema-more> .

<http://www.w3.org/1999/02/22-rdf-syntax-ns#> rdfs:seeAlso <http://www.w3.org/2000/01/rdf-schema-more> .

<http://americanart.si.edu/ontology/> dct:creator "Pedro Szekely", "Fengyu Yang",
    "Xuming Zhu" .

<http://purl.org/NET/dc_owl2dl/terms> dct:creator <http://simon-reinhardt.de/#me> .

<http://www.w3.org/2008/05/skos> dc:creator "Sean Bechhofer", "Alistair Miles" .

<http://www.europeana.eu/schemas/edm/> dc:creator "Antoine Isaac" .

<http://purl.org/vocab/frbr/core> dc:creator <http://iandavis.com/id/me>, _:genid-38640ccbd5eb49418600e8d7df2cf451-mor50bd147e3df08 .

_:genid-38640ccbd5eb49418600e8d7df2cf451-mor50bd147e4041a rdf:value "Added isDefinedBy property referring to FRBR core namespace" .

_:genid-38640ccbd5eb49418600e8d7df2cf451-mor50bd147e40467 rdf:value "Added definition" .

_:genid-38640ccbd5eb49418600e8d7df2cf451-mor50bd147e404b3 rdf:value "Added domain and range of Work or Expression" .

_:genid-38640ccbd5eb49418600e8d7df2cf451-mor50bd147e406be rdf:value "Added isDefinedBy property referring to FRBR core namespace" .

_:genid-38640ccbd5eb49418600e8d7df2cf451-mor50bd147e4070b rdf:value "Added definition" .

_:genid-38640ccbd5eb49418600e8d7df2cf451-mor50bd147e40757 rdf:value "Added domain and range of Work or Expression" .

_:genid-38640ccbd5eb49418600e8d7df2cf451-mor50bd147e40962 rdf:value "Added isDefinedBy property referring to FRBR core namespace" .

_:genid-38640ccbd5eb49418600e8d7df2cf451-mor50bd147e409ad rdf:value "Added definition" .

_:genid-38640ccbd5eb49418600e8d7df2cf451-mor50bd147e409fa rdf:value "Added domain and range of Work or Expression" .

_:genid-38640ccbd5eb49418600e8d7df2cf451-mor50bd147e40c00 rdf:value "Added isDefinedBy property referring to FRBR core namespace" .

_:genid-38640ccbd5eb49418600e8d7df2cf451-mor50bd147e40c4b rdf:value "Added definition" .

_:genid-38640ccbd5eb49418600e8d7df2cf451-mor50bd147e40c97 rdf:value "Added domain and range of Work or Expression" .

_:genid-38640ccbd5eb49418600e8d7df2cf451-mor50bd147e40ea3 rdf:value "Added isDefinedBy property referring to FRBR core namespace" .

_:genid-38640ccbd5eb49418600e8d7df2cf451-mor50bd147e40eee rdf:value "Added definition" .

_:genid-38640ccbd5eb49418600e8d7df2cf451-mor50bd147e40f3a rdf:value "Added domain and range of Work or Expression" .

_:genid-38640ccbd5eb49418600e8d7df2cf451-mor50bd147e41141 rdf:value "Added isDefinedBy property referring to FRBR core namespace" .

_:genid-38640ccbd5eb49418600e8d7df2cf451-mor50bd147e4118e rdf:value "Added definition" .

_:genid-38640ccbd5eb49418600e8d7df2cf451-mor50bd147e411e1 rdf:value "Added domain and range of Work or Expression" .

_:genid-38640ccbd5eb49418600e8d7df2cf451-mor50bd147e413f6 rdf:value "Added isDefinedBy property referring to FRBR core namespace" .

_:genid-38640ccbd5eb49418600e8d7df2cf451-mor50bd147e41442 rdf:value "Added definition" .

_:genid-38640ccbd5eb49418600e8d7df2cf451-mor50bd147e4148d rdf:value "Added domain and range of Work or Expression" .

_:genid-38640ccbd5eb49418600e8d7df2cf451-mor50bd147e416a1 rdf:value "Added isDefinedBy property referring to FRBR core namespace" .

_:genid-38640ccbd5eb49418600e8d7df2cf451-mor50bd147e416ec rdf:value "Added definition" .

_:genid-38640ccbd5eb49418600e8d7df2cf451-mor50bd147e41738 rdf:value "Added domain and range of Work or Expression" .

_:genid-38640ccbd5eb49418600e8d7df2cf451-mor50bd147e4193f rdf:value "Added isDefinedBy property referring to FRBR core namespace" .

_:genid-38640ccbd5eb49418600e8d7df2cf451-mor50bd147e4198a rdf:value "Added definition" .

_:genid-38640ccbd5eb49418600e8d7df2cf451-mor50bd147e419d9 rdf:value "Added domain and range of Work or Expression" .

_:genid-38640ccbd5eb49418600e8d7df2cf451-mor50bd147e41bde rdf:value "Added isDefinedBy property referring to FRBR core namespace" .

_:genid-38640ccbd5eb49418600e8d7df2cf451-mor50bd147e41c2a rdf:value "Added definition" .

_:genid-38640ccbd5eb49418600e8d7df2cf451-mor50bd147e41c76 rdf:value "Added domain and range of Work or Expression" .

_:genid-38640ccbd5eb49418600e8d7df2cf451-mor50bd147e41e80 rdf:value "Added isDefinedBy property referring to FRBR core namespace" .

_:genid-38640ccbd5eb49418600e8d7df2cf451-mor50bd147e41ecb rdf:value "Added definition" .

_:genid-38640ccbd5eb49418600e8d7df2cf451-mor50bd147e41f16 rdf:value "Added domain and range of Work or Expression" .

_:genid-38640ccbd5eb49418600e8d7df2cf451-mor50bd147e42120 rdf:value "Added isDefinedBy property referring to FRBR core namespace" .

_:genid-38640ccbd5eb49418600e8d7df2cf451-mor50bd147e42174 rdf:value "Added definition" .

_:genid-38640ccbd5eb49418600e8d7df2cf451-mor50bd147e421c2 rdf:value "Added domain and range of Work or Expression" .

_:genid-38640ccbd5eb49418600e8d7df2cf451-mor50bd147e423cc rdf:value "Added isDefinedBy property referring to FRBR core namespace" .

_:genid-38640ccbd5eb49418600e8d7df2cf451-mor50bd147e42417 rdf:value "Added definition" .

_:genid-38640ccbd5eb49418600e8d7df2cf451-mor50bd147e42464 rdf:value "Added domain and range of Work or Expression" .

_:genid-38640ccbd5eb49418600e8d7df2cf451-mor50bd147e424d0 rdf:value "Added isDefinedBy property referring to FRBR core namespace" .

_:genid-38640ccbd5eb49418600e8d7df2cf451-mor50bd147e4251f rdf:value "Added definition" .

_:genid-38640ccbd5eb49418600e8d7df2cf451-mor50bd147e4257a rdf:value "Added domain and range of Expression" .

_:genid-38640ccbd5eb49418600e8d7df2cf451-mor50bd147e425e9 rdf:value "Added isDefinedBy property referring to FRBR core namespace" .

_:genid-38640ccbd5eb49418600e8d7df2cf451-mor50bd147e42635 rdf:value "Added definition" .

_:genid-38640ccbd5eb49418600e8d7df2cf451-mor50bd147e42681 rdf:value "Added domain and range of Expression" .

_:genid-38640ccbd5eb49418600e8d7df2cf451-mor50bd147e426f2 rdf:value "Added isDefinedBy property referring to FRBR core namespace" .

_:genid-38640ccbd5eb49418600e8d7df2cf451-mor50bd147e4273d rdf:value "Added definition" .

_:genid-38640ccbd5eb49418600e8d7df2cf451-mor50bd147e4278a rdf:value "Added domain and range of Expression" .

_:genid-38640ccbd5eb49418600e8d7df2cf451-mor50bd147e427f6 rdf:value "Added isDefinedBy property referring to FRBR core namespace" .

_:genid-38640ccbd5eb49418600e8d7df2cf451-mor50bd147e42842 rdf:value "Added definition" .

_:genid-38640ccbd5eb49418600e8d7df2cf451-mor50bd147e4288e rdf:value "Added domain and range of Expression" .

_:genid-38640ccbd5eb49418600e8d7df2cf451-mor50bd147e428fb rdf:value "Added isDefinedBy property referring to FRBR core namespace" .

_:genid-38640ccbd5eb49418600e8d7df2cf451-mor50bd147e42948 rdf:value "Added definition" .

_:genid-38640ccbd5eb49418600e8d7df2cf451-mor50bd147e42994 rdf:value "Added domain and range of Expression" .

_:genid-38640ccbd5eb49418600e8d7df2cf451-mor50bd147e42a01 rdf:value "Added isDefinedBy property referring to FRBR core namespace" .

_:genid-38640ccbd5eb49418600e8d7df2cf451-mor50bd147e42a4f rdf:value "Added definition" .

_:genid-38640ccbd5eb49418600e8d7df2cf451-mor50bd147e42a9b rdf:value "Added domain and range of Expression" .

_:genid-38640ccbd5eb49418600e8d7df2cf451-mor50bd147e42b08 rdf:value "Added isDefinedBy property referring to FRBR core namespace" .

_:genid-38640ccbd5eb49418600e8d7df2cf451-mor50bd147e42b58 rdf:value "Added definition" .

_:genid-38640ccbd5eb49418600e8d7df2cf451-mor50bd147e42ba4 rdf:value "Added domain and range of Expression" .

_:genid-38640ccbd5eb49418600e8d7df2cf451-mor50bd147e42c11 rdf:value "Added isDefinedBy property referring to FRBR core namespace" .

_:genid-38640ccbd5eb49418600e8d7df2cf451-mor50bd147e42c5d rdf:value "Added definition" .

_:genid-38640ccbd5eb49418600e8d7df2cf451-mor50bd147e42cac rdf:value "Added domain and range of Expression" .

_:genid-38640ccbd5eb49418600e8d7df2cf451-mor50bd147e42d99 rdf:value "Added isDefinedBy property referring to FRBR core namespace" .

_:genid-38640ccbd5eb49418600e8d7df2cf451-mor50bd147e42de7 rdf:value "Added definition" .

_:genid-38640ccbd5eb49418600e8d7df2cf451-mor50bd147e42e52 rdf:value "Added isDefinedBy property referring to FRBR core namespace" .

_:genid-38640ccbd5eb49418600e8d7df2cf451-mor50bd147e42e9d rdf:value "Added definition" .

_:genid-38640ccbd5eb49418600e8d7df2cf451-mor50bd147e42f0c rdf:value "Added isDefinedBy property referring to FRBR core namespace" .

_:genid-38640ccbd5eb49418600e8d7df2cf451-mor50bd147e42f58 rdf:value "Added definition" .

_:genid-38640ccbd5eb49418600e8d7df2cf451-mor50bd147e42fc3 rdf:value "Added isDefinedBy property referring to FRBR core namespace" .

_:genid-38640ccbd5eb49418600e8d7df2cf451-mor50bd147e4300e rdf:value "Added definition" .

_:genid-38640ccbd5eb49418600e8d7df2cf451-mor50bd147e4307c rdf:value "Added isDefinedBy property referring to FRBR core namespace" .

_:genid-38640ccbd5eb49418600e8d7df2cf451-mor50bd147e430ca rdf:value "Added definition" .

_:genid-38640ccbd5eb49418600e8d7df2cf451-mor50bd147e43138 rdf:value "Added isDefinedBy property referring to FRBR core namespace" .

_:genid-38640ccbd5eb49418600e8d7df2cf451-mor50bd147e4318b rdf:value "Added definition" .

_:genid-38640ccbd5eb49418600e8d7df2cf451-mor50bd147e43202 rdf:value "Added isDefinedBy property referring to FRBR core namespace" .

_:genid-38640ccbd5eb49418600e8d7df2cf451-mor50bd147e4324e rdf:value "Added definition" .

_:genid-38640ccbd5eb49418600e8d7df2cf451-mor50bd147e432be rdf:value "Added isDefinedBy property referring to FRBR core namespace" .

_:genid-38640ccbd5eb49418600e8d7df2cf451-mor50bd147e4330c rdf:value "Added definition" .

_:genid-38640ccbd5eb49418600e8d7df2cf451-mor50bd147e4337b rdf:value "Added isDefinedBy property referring to FRBR core namespace" .

_:genid-38640ccbd5eb49418600e8d7df2cf451-mor50bd147e433c7 rdf:value "Added definition" .

_:genid-38640ccbd5eb49418600e8d7df2cf451-mor50bd147e43436 rdf:value "Added isDefinedBy property referring to FRBR core namespace" .

_:genid-38640ccbd5eb49418600e8d7df2cf451-mor50bd147e43481 rdf:value "Added definition" .

_:genid-38640ccbd5eb49418600e8d7df2cf451-mor50bd147e434fa rdf:value "Added isDefinedBy property referring to FRBR core namespace" .

_:genid-38640ccbd5eb49418600e8d7df2cf451-mor50bd147e43545 rdf:value "Added definition" .

_:genid-38640ccbd5eb49418600e8d7df2cf451-mor50bd147e435b5 rdf:value "Added isDefinedBy property referring to FRBR core namespace" .

_:genid-38640ccbd5eb49418600e8d7df2cf451-mor50bd147e43600 rdf:value "Added definition" .

_:genid-38640ccbd5eb49418600e8d7df2cf451-mor50bd147e4377b rdf:value "Added isDefinedBy property referring to FRBR core namespace" .

_:genid-38640ccbd5eb49418600e8d7df2cf451-mor50bd147e437c6 rdf:value "Added definition" .

_:node92 rdfs:label "The Open Archives Initiative ORE Project" .

_:genid-38640ccbd5eb49418600e8d7df2cf451-mor50bd147e3df74 dc:creator <http://iandavis.com/id/me>;
  rdfs:label "Added type hierarchy"@en .

_:genid-38640ccbd5eb49418600e8d7df2cf451-mor50bd147e3dfc0 dc:creator <http://iandavis.com/id/me>;
  rdfs:label "Various minor tidying tasks"@en .

_:genid-38640ccbd5eb49418600e8d7df2cf451-mor50bd147e3e0bd rdfs:label "the union of all expressions, items, manifestations and works"@en .

_:genid-38640ccbd5eb49418600e8d7df2cf451-mor50bd147e3e84b rdfs:label "the union of all people and corporate bodies"@en .

_:genid-38640ccbd5eb49418600e8d7df2cf451-mor50bd147e3eb2e rdfs:label "the union of all organizations and groups"@en .

_:genid-38640ccbd5eb49418600e8d7df2cf451-mor50bd147e3ed08 rdfs:label "the union of all events, objects, places and concepts"@en .

_:genid-38640ccbd5eb49418600e8d7df2cf451-mor50bd147e3fa74 rdfs:label "a manifestation or an item"@en .

_:genid-38640ccbd5eb49418600e8d7df2cf451-mor50bd147e3fb4c rdfs:label "a manifestation or an item"@en .

_:genid-38640ccbd5eb49418600e8d7df2cf451-mor50bd147e3fd1d rdfs:label "a manifestation or an item"@en .

_:genid-38640ccbd5eb49418600e8d7df2cf451-mor50bd147e3fdf6 rdfs:label "a manifestation or an item"@en .

_:genid-38640ccbd5eb49418600e8d7df2cf451-mor50bd147e3e223 dc:creator "Ian Davis" .

_:genid-38640ccbd5eb49418600e8d7df2cf451-mor50bd147e3e26f dc:creator "Ian Davis" .

_:genid-38640ccbd5eb49418600e8d7df2cf451-mor50bd147e3e2bf dc:creator "Ian Davis" .

_:genid-38640ccbd5eb49418600e8d7df2cf451-mor50bd147e3e496 dc:creator "Ian Davis" .

_:genid-38640ccbd5eb49418600e8d7df2cf451-mor50bd147e3e4e2 dc:creator "Ian Davis" .

_:genid-38640ccbd5eb49418600e8d7df2cf451-mor50bd147e3e52e dc:creator "Ian Davis" .

_:genid-38640ccbd5eb49418600e8d7df2cf451-mor50bd147e3e6b4 dc:creator "Ian Davis" .

_:genid-38640ccbd5eb49418600e8d7df2cf451-mor50bd147e3e74b dc:creator "Ian Davis" .

_:genid-38640ccbd5eb49418600e8d7df2cf451-mor50bd147e3e798 dc:creator "Ian Davis" .

_:genid-38640ccbd5eb49418600e8d7df2cf451-mor50bd147e3e700 dc:creator "Ian Davis" .

_:genid-38640ccbd5eb49418600e8d7df2cf451-mor50bd147e3e7e4 dc:creator "Ian Davis" .

_:genid-38640ccbd5eb49418600e8d7df2cf451-mor50bd147e3e5a5 dc:creator "Ian Davis" .

_:genid-38640ccbd5eb49418600e8d7df2cf451-mor50bd147e3e5f3 dc:creator "Ian Davis" .

_:genid-38640ccbd5eb49418600e8d7df2cf451-mor50bd147e3e641 dc:creator "Ian Davis" .

_:genid-38640ccbd5eb49418600e8d7df2cf451-mor50bd147e3e336 dc:creator "Ian Davis" .

_:genid-38640ccbd5eb49418600e8d7df2cf451-mor50bd147e3e383 dc:creator "Ian Davis" .

_:genid-38640ccbd5eb49418600e8d7df2cf451-mor50bd147e3e424 dc:creator "Ian Davis" .

_:genid-38640ccbd5eb49418600e8d7df2cf451-mor50bd147e3e3d8 dc:creator "Ian Davis" .

_:genid-38640ccbd5eb49418600e8d7df2cf451-mor50bd147e3e925 dc:creator "Ian Davis" .

_:genid-38640ccbd5eb49418600e8d7df2cf451-mor50bd147e3e971 dc:creator "Ian Davis" .

_:genid-38640ccbd5eb49418600e8d7df2cf451-mor50bd147e3e9bd dc:creator "Ian Davis" .

_:genid-38640ccbd5eb49418600e8d7df2cf451-mor50bd147e3ec08 dc:creator "Ian Davis" .

_:genid-38640ccbd5eb49418600e8d7df2cf451-mor50bd147e3ec53 dc:creator "Ian Davis" .

_:genid-38640ccbd5eb49418600e8d7df2cf451-mor50bd147e3ec9f dc:creator "Ian Davis" .

_:genid-38640ccbd5eb49418600e8d7df2cf451-mor50bd147e3ea2b dc:creator "Ian Davis" .

_:genid-38640ccbd5eb49418600e8d7df2cf451-mor50bd147e3ea78 dc:creator "Ian Davis" .

_:genid-38640ccbd5eb49418600e8d7df2cf451-mor50bd147e3eac9 dc:creator "Ian Davis" .

_:genid-38640ccbd5eb49418600e8d7df2cf451-mor50bd147e3ee70 dc:creator "Ian Davis" .

_:genid-38640ccbd5eb49418600e8d7df2cf451-mor50bd147e3eebb dc:creator "Ian Davis" .

_:genid-38640ccbd5eb49418600e8d7df2cf451-mor50bd147e3ef08 dc:creator "Ian Davis" .

_:genid-38640ccbd5eb49418600e8d7df2cf451-mor50bd147e3f23c dc:creator "Ian Davis" .

_:genid-38640ccbd5eb49418600e8d7df2cf451-mor50bd147e3f2de dc:creator "Ian Davis" .

_:genid-38640ccbd5eb49418600e8d7df2cf451-mor50bd147e3f292 dc:creator "Ian Davis" .

_:genid-38640ccbd5eb49418600e8d7df2cf451-mor50bd147e3f0e2 dc:creator "Ian Davis" .

_:genid-38640ccbd5eb49418600e8d7df2cf451-mor50bd147e3f12e dc:creator "Ian Davis" .

_:genid-38640ccbd5eb49418600e8d7df2cf451-mor50bd147e3f1c4 dc:creator "Ian Davis" .

_:genid-38640ccbd5eb49418600e8d7df2cf451-mor50bd147e3f17a dc:creator "Ian Davis" .

_:genid-38640ccbd5eb49418600e8d7df2cf451-mor50bd147e3f354 dc:creator "Ian Davis" .

_:genid-38640ccbd5eb49418600e8d7df2cf451-mor50bd147e3f3a9 dc:creator "Ian Davis" .

_:genid-38640ccbd5eb49418600e8d7df2cf451-mor50bd147e3f43f dc:creator "Ian Davis" .

_:genid-38640ccbd5eb49418600e8d7df2cf451-mor50bd147e3f3f4 dc:creator "Ian Davis" .

_:genid-38640ccbd5eb49418600e8d7df2cf451-mor50bd147e3ef7f dc:creator "Ian Davis" .

_:genid-38640ccbd5eb49418600e8d7df2cf451-mor50bd147e3efcc dc:creator "Ian Davis" .

_:genid-38640ccbd5eb49418600e8d7df2cf451-mor50bd147e3f065 dc:creator "Ian Davis" .

_:genid-38640ccbd5eb49418600e8d7df2cf451-mor50bd147e3f019 dc:creator "Ian Davis" .

_:genid-38640ccbd5eb49418600e8d7df2cf451-mor50bd147e3f566 dc:creator "Ian Davis" .

_:genid-38640ccbd5eb49418600e8d7df2cf451-mor50bd147e3f5b4 dc:creator "Ian Davis" .

_:genid-38640ccbd5eb49418600e8d7df2cf451-mor50bd147e3f622 dc:creator "Ian Davis" .

_:genid-38640ccbd5eb49418600e8d7df2cf451-mor50bd147e3f66c dc:creator "Ian Davis" .

_:genid-38640ccbd5eb49418600e8d7df2cf451-mor50bd147e3f6da dc:creator "Ian Davis" .

_:genid-38640ccbd5eb49418600e8d7df2cf451-mor50bd147e3f729 dc:creator "Ian Davis" .

_:genid-38640ccbd5eb49418600e8d7df2cf451-mor50bd147e3f797 dc:creator "Ian Davis" .

_:genid-38640ccbd5eb49418600e8d7df2cf451-mor50bd147e3f7e2 dc:creator "Ian Davis" .

_:genid-38640ccbd5eb49418600e8d7df2cf451-mor50bd147e3f852 dc:creator "Ian Davis" .

_:genid-38640ccbd5eb49418600e8d7df2cf451-mor50bd147e3f89d dc:creator "Ian Davis" .

_:genid-38640ccbd5eb49418600e8d7df2cf451-mor50bd147e3f90e dc:creator "Ian Davis" .

_:genid-38640ccbd5eb49418600e8d7df2cf451-mor50bd147e3f95a dc:creator "Ian Davis" .

<http://www.w3.org/2008/05/skos> dc:description "An RDF vocabulary for describing the basic structure and content of concept schemes such as thesauri, classification schemes, subject heading lists, taxonomies, 'folksonomies', other types of controlled vocabulary, and also concept schemes embedded in glossaries and terminologies."@en .

<http://www.europeana.eu/schemas/edm/> dc:description "The Europeana Data Model (EDM) is aimed at being an integration medium for collecting, connecting and enriching the descriptions provided by Europeana data providers. The RDF vocabulary for http://www.europeana.eu/schemas/edm/ defines the elements introduced by EDM (as opposed to the ones EDM re-uses from other namespaces)."@en .

<http://xmlns.com/foaf/0.1/> dc:description "The Friend of a Friend (FOAF) RDF vocabulary, described using W3C RDF Schema and the Web Ontology Language." .

<http://www.w3.org/1999/02/22-rdf-syntax-ns#> dc:description "This is the RDF Schema for the RDF vocabulary defined in the RDF namespace." .

<http://www.w3.org/2008/05/skos> dc:contributor "Participants in W3C's Semantic Web Deployment Working Group.",
    "Dave Beckett", "Nikki Rogers" .

<http://americanart.si.edu/ontology/> dc:contributor "Participants in Smithsonian Project Group of Information Science Institute, USC." .

<http://www.europeana.eu/schemas/edm/> dc:contributor "Participants of Europeana Version 1.0 Work Package on Further Specification of Functionality and Interoperability aspects of Europeana (WP3)",
    "Nasos Drosopoulos", "Hugo Borbinhas", "Julia Iwanowa", "Vassilis Tzouvaras", "Martin Doerr" .

<http://purl.org/vocab/frbr/core> dc:contributor <http://bruce.darcus.name/about#me> .

<http://www.w3.org/2008/05/skos> dc:title "SKOS Core Vocabulary"@en .

<http://www.europeana.eu/schemas/edm/> dc:title "Europeana Data Model (EDM) vocabulary"@en .

<http://rdvocab.info/ElementsGr2> dc:title "RDA Group 2 Elements"@en .

<http://purl.org/vocab/frbr/core> dc:title "Expression of Core FRBR Concepts in RDF"@en .

<http://xmlns.com/foaf/0.1/> dc:title "Friend of a Friend (FOAF) vocabulary" .

<http://www.w3.org/2000/01/rdf-schema#> dc:title "The RDF Schema vocabulary (RDFS)" .

<http://www.w3.org/1999/02/22-rdf-syntax-ns#> dc:title "The RDF Vocabulary (RDF)" .

skos:Concept dct:issued "2008-05-xx" .

skos:altLabel dct:issued "2008-05-xx" .

skos:definition dct:issued "2008-05-xx" .

skos:hiddenLabel dct:issued "2008-05-xx" .

skos:prefLabel dct:issued "2008-05-xx" .

skos:broadMatch dct:issued "2008-05-xx" .

skos:broader dct:issued "2008-05-xx" .

skos:mappingRelation dct:issued "2008-05-xx" .

skos:broaderTransitive dct:issued "2008-05-xx" .

skos:narrower dct:issued "2008-05-xx" .

skos:narrowerTransitive dct:issued "2008-05-xx" .

skos:semanticRelation dct:issued "2008-05-xx" .

skos:changeNote dct:issued "2008-05-xx" .

skos:note dct:issued "2008-05-xx" .

skos:closeMatch dct:issued "2008-05-xx" .

skos:editorialNote dct:issued "2008-05-xx" .

skos:exactMatch dct:issued "2008-05-xx" .

skos:example dct:issued "2008-05-xx" .

skos:hasTopConcept dct:issued "2008-05-xx" .

skos:ConceptScheme dct:issued "2008-05-xx" .

skos:historyNote dct:issued "2008-05-xx" .

skos:inScheme dct:issued "2008-05-xx" .

skos:member dct:issued "2008-05-xx" .

skos:Collection dct:issued "2008-05-xx" .

skos:memberList dct:issued "2008-05-xx" .

skos:OrderedCollection dct:issued "2008-05-xx" .

skos:narrowMatch dct:issued "2008-05-xx" .

skos:related dct:issued "2008-05-xx" .

skos:relatedMatch dct:issued "2008-05-xx" .

skos:scopeNote dct:issued "2008-05-xx" .

skos:topConceptOf dct:issued "2008-05-xx" .

skos:notation dct:issued "2008-05-xx" .

<http://americanart.si.edu/ontology/> dct:issued "2012-07-30"^^xsd:date .

frbr_core:Event dct:issued "2005-07-15" .

frbr_core:Expression dct:issued "2005-07-15" .

frbr_core:Manifestation dct:issued "2005-07-15" .

frbr_core:Place dct:issued "2005-07-15" .

frbr_core:Work dct:issued "2005-07-15" .

<http://purl.org/vocab/frbr/core> dct:issued "2005-07-15" .

frbr_core:Endeavour dct:issued "2005-07-15" .

frbr_core:ResponsibleEntity dct:issued "2005-07-15" .

frbr_core:Subject dct:issued "2005-07-15" .

frbr_core:Item dct:issued "2005-07-15" .

frbr_core:CorporateBody dct:issued "2005-07-15" .

frbr_core:Person dct:issued "2005-08-08" .

frbr_core:Object dct:issued "2005-07-15" .

frbr_core:Concept dct:issued "2005-07-15" .

frbr_core:ClassicalWork dct:issued "2005-10-14" .

frbr_core:LegalWork dct:issued "2005-10-14" .

frbr_core:LiteraryWork dct:issued "2005-10-14" .

frbr_core:ScholarlyWork dct:issued "2005-10-14" .

frbr_core:Text dct:issued "2005-10-14" .

frbr_core:Image dct:issued "2005-10-14" .

frbr_core:Sound dct:issued "2005-10-14" .

frbr_core:MovingImage dct:issued "2005-10-14" .

frbr_core:Data dct:issued "2005-10-14" .

frbr_core:Performance dct:issued "2005-10-14" .

frbr_core:relatedEndeavour dct:issued "2005-07-15" .

frbr_core:realization dct:issued "2005-07-15" .

frbr_core:realizationOf dct:issued "2005-07-15" .

frbr_core:embodiment dct:issued "2005-07-15" .

frbr_core:embodimentOf dct:issued "2005-07-15" .

frbr_core:exemplar dct:issued "2005-07-15" .

frbr_core:exemplarOf dct:issued "2005-07-15" .

frbr_core:reproduction dct:issued "2005-07-15" .

frbr_core:reproductionOf dct:issued "2005-07-15" .

frbr_core:successor dct:issued "2005-07-15" .

frbr_core:successorOf dct:issued "2005-07-15" .

frbr_core:supplement dct:issued "2005-07-15" .

frbr_core:supplementOf dct:issued "2005-07-15" .

frbr_core:complement dct:issued "2005-07-15" .

frbr_core:complementOf dct:issued "2005-07-15" .

frbr_core:summarization dct:issued "2005-07-15" .

frbr_core:summarizationOf dct:issued "2005-07-15" .

frbr_core:adaption dct:issued "2005-07-15" .

frbr_core:adaptionOf dct:issued "2005-07-15" .

frbr_core:transformation dct:issued "2005-07-15" .

frbr_core:transformationOf dct:issued "2005-07-15" .

frbr_core:imitation dct:issued "2005-07-15" .

frbr_core:imitationOf dct:issued "2005-07-15" .

frbr_core:abridgement dct:issued "2005-07-15" .

frbr_core:abridgementOf dct:issued "2005-07-15" .

frbr_core:revision dct:issued "2005-07-15" .

frbr_core:revisionOf dct:issued "2005-07-15" .

frbr_core:translation dct:issued "2005-07-15" .

frbr_core:translationOf dct:issued "2005-07-15" .

frbr_core:arrangement dct:issued "2005-07-15" .

frbr_core:arrangementOf dct:issued "2005-07-15" .

frbr_core:alternate dct:issued "2005-08-10" .

frbr_core:alternateOf dct:issued "2005-08-10" .

frbr_core:reconfiguration dct:issued "2005-08-10" .

frbr_core:reconfigurationOf dct:issued "2005-08-10" .

frbr_core:part dct:issued "2005-07-15" .

frbr_core:partOf dct:issued "2005-07-15" .

frbr_core:responsibleEntity dct:issued "2005-07-15" .

frbr_core:responsibleEntityOf dct:issued "2005-07-15" .

frbr_core:creator dct:issued "2005-07-15" .

frbr_core:creatorOf dct:issued "2005-07-15" .

frbr_core:realizer dct:issued "2005-07-15" .

frbr_core:realizerOf dct:issued "2005-07-15" .

frbr_core:producer dct:issued "2005-07-15" .

frbr_core:producerOf dct:issued "2005-07-15" .

frbr_core:owner dct:issued "2005-07-15" .

frbr_core:ownerOf dct:issued "2005-07-15" .

frbr_core:subject dct:issued "2005-07-15" .

ElementsGr2:placeOfBirth skos:definition "The town, city, province, state, and/or country in which a person was born."@en .

ElementsGr2:placeOfDeath skos:definition "The town, city, province, state, and/or country in which a person died."@en .

skos:Concept skos:definition "An abstract idea or notion; a unit of thought."@en .

skos:altLabel skos:definition "An alternative lexical label for a resource."@en .

skos:definition skos:definition "A statement or formal explanation of the meaning of a concept."@en .

skos:hiddenLabel skos:definition "A lexical label for a resource that should be hidden when generating visual displays of the resource, but should still be accessible to free text search operations."@en .

skos:prefLabel skos:definition "The preferred lexical label for a resource, in a given language."@en .

skos:broadMatch skos:definition "skos:broadMatch is used to state a hierarchical mapping link between two conceptual resources in different concept schemes."@en .

skos:broader skos:definition "A concept that is more general in meaning."@en .

skos:mappingRelation skos:definition "Definition"@en .

skos:broaderTransitive skos:definition "skos:broaderTransitive is a transitive superproperty of skos:broader." .

skos:narrower skos:definition "A concept that is more specific in meaning."@en .

skos:narrowerTransitive skos:definition "skos:narrowerTransitive is a transitive superproperty of skos:broader. By convention, skos:narrowerTransitive is not intended to be used in assertions, but provides a mechanism whereby the transitive closure of skos:narrower can be queried." .

skos:semanticRelation skos:definition "A concept related by meaning."@en .

skos:changeNote skos:definition "A note about a modification to a concept."@en .

skos:note skos:definition "A general note, for any purpose."@en .

skos:closeMatch skos:definition "skos:closeMatch is used to link two concepts that are sufficiently similar that they can be used interchangeably in some information retrieval applications. In order to avoid the possibility of \"compound errors\" when combining mappings across more than two concept schemes, skos:closeMatch is not declared to be a transitive property."@en .

skos:editorialNote skos:definition "A note for an editor, translator or maintainer of the vocabulary."@en .

skos:exactMatch skos:definition "skos:exactMatch is used to link two concepts, indicating a high degree of confidence that the concepts can be used interchangeably across a wide range of information retrieval applications. skos:exactMatch is a transitive property, and is a sub-property of skos:closeMatch."@en .

skos:example skos:definition "An example of the use of a concept."@en .

skos:hasTopConcept skos:definition "A top level concept in the concept scheme."@en .

skos:ConceptScheme skos:definition "A set of concepts, optionally including statements about semantic relationships between those concepts."@en .

skos:historyNote skos:definition "A note about the past state/use/meaning of a concept."@en .

skos:inScheme skos:definition "A concept scheme in which the concept is included."@en .

skos:member skos:definition "A member of a collection."@en .

skos:Collection skos:definition "A meaningful collection of concepts."@en .

skos:memberList skos:definition "An RDF list containing the members of an ordered collection."@en .

skos:OrderedCollection skos:definition "An ordered collection of concepts, where both the grouping and the ordering are meaningful."@en .

skos:narrowMatch skos:definition "skos:narrowMatch is used to state a hierarchical mapping link between two conceptual resources in different concept schemes."@en .

skos:related skos:definition "A concept with which there is an associative semantic relationship."@en .

skos:relatedMatch skos:definition "skos:relatedMatch is used to state an associative mapping link between two conceptual resources in different concept schemes."@en .

skos:scopeNote skos:definition "A note that helps to clarify the meaning of a concept."@en .

skos:topConceptOf skos:definition "Relates a concept to the concept scheme that it is a top level concept of."@en .

skos:notation skos:definition "A notation, also known as classification code, is a string of characters such as \"T58.5\" or \"303.4833\" used to uniquely identify a concept within the scope of a given concept scheme."@en .

frbr_core:Event skos:definition "An action or occurrence."@en .

frbr_core:Expression skos:definition "A realization of a single work usually in a physical form."@en .

frbr_core:Manifestation skos:definition "The physical embodiment of one or more expressions."@en .

frbr_core:Place skos:definition "A location."@en .

frbr_core:Work skos:definition "An abstract notion of an artistic or intellectual creation."@en .

ElementsGr2:addressOfTheCorporateBody skos:definition "The address of a corporate bodys headquarters or offices, or an e-mail or Internet address for the body."@en .

ElementsGr2:addressOfThePerson skos:definition "The address of a persons place of residence, business, or employer, and/or an e-mail or Internet address."@en .

ElementsGr2:affiliation skos:definition "A group with which a person is affiliated or has been affiliated through employment, membership, cultural identity, etc."@en .

ElementsGr2:associatedInstitution skos:definition "An institution commonly associated with a corporate body."@en .

ElementsGr2:biographicalInformation skos:definition "Information pertaining to the life or history of a person."@en .

ElementsGr2:corporateHistory skos:definition "Information pertaining to the history of a corporate body."@en .

ElementsGr2:countryAssociatedWithThePerson skos:definition "A country with which a person is identified."@en .

ElementsGr2:dateAssociatedWithTheCorporateBody skos:definition "The date or range of dates on which a conference, etc., is held, or a date with which a corporate body is otherwise associated (e.g., date of founding)."@en .

ElementsGr2:dateOfEstablishment skos:definition "The date on which a corporate body was established or founded."@en .

ElementsGr2:dateOfConferenceEtc skos:definition "The date or range of dates on which a conference, congress, meeting, exhibition, fair, festival, etc., was held."@en .

ElementsGr2:dateOfTermination skos:definition "The date on which a corporate body was terminated or dissolved."@en .

ElementsGr2:dateAssociatedWithTheFamily skos:definition "A significant date associated with a family."@en .

ElementsGr2:dateAssociatedWithThePerson skos:definition "A significant date associated with a person (e.g., date of birth, date of death)."@en .

ElementsGr2:dateOfBirth skos:definition "The year a person was born. Date of birth may also include the month and day of the persons birth."@en .

ElementsGr2:dateOfDeath skos:definition "The year a person died. Date of death may also include the month and day of the persons death."@en .

ElementsGr2:periodOfActivityOfThePerson skos:definition "A date or range of dates indicative of the period in which a person was active in his or her primary field of endeavour."@en .

ElementsGr2:dateOfUsage skos:definition "A date or range of dates associated with the use of the name designated as the preferred name for a person."@en .

ElementsGr2:familyHistory skos:definition "Information pertaining to the history of a family."@en .

ElementsGr2:fieldOfActivityOfTheCorporateBody skos:definition "A field of business in which a corporate body is engaged, its area of competence, responsibility, jurisdiction, etc."@en .

ElementsGr2:fieldOfActivityOfThePerson skos:definition "A field of endeavour, area of expertise, etc., in which a person is engaged or was engaged."@en .

ElementsGr2:fullerFormOfName skos:definition "The full form of a part of a name represented only by an initial or abbreviation in the form chosen as the preferred name, or a part of the name not included in the form chosen as the preferred name."@en .

ElementsGr2:fullerFormOfNamePerson skos:definition "The full form of a part of a name represented only by an initial or abbreviation in the form chosen as the preferred name, or a part of the name not included in the form chosen as the preferred name."@en .

ElementsGr2:gender skos:definition "The gender with which a person identifies."@en .

ElementsGr2:hereditaryTitle skos:definition "A title of nobility, etc., associated with a family."@en .

ElementsGr2:identifierForTheCorporateBody skos:definition """A character string uniquely associated with a corporate body, or with a surrogate for a corporate body (e.g., an authority record), that

serves to differentiate that corporate body from other corporate bodies."""@en .

ElementsGr2:identifierForTheFamily skos:definition "A character string uniquely associated with a family, or with a surrogate for a family (e.g., an authority record), that serves to differentiate that family from other families."@en .

ElementsGr2:identifierForThePerson skos:definition "A character string uniquely associated with a person, or with a surrogate for a person (e.g., an authority record), that serves to differentiate that person from other persons."@en .

ElementsGr2:languageOfTheCorporateBody skos:definition "A language a corporate body uses in its communications."@en .

ElementsGr2:languageOfThePerson skos:definition "A language a person uses when writing for publication, broadcasting, etc."@en .

ElementsGr2:locationOfConferenceEtc skos:definition "A local place in which a conference, congress, meeting, exhibition, fair, festival, etc., was held."@en .

ElementsGr2:placeAssociatedWithTheCorporateBody skos:definition """A significant location associated with a corporate body (e.g., location of a conference, etc., location of the headquarters of an

organization)."""@en .

ElementsGr2:locationOfHeadquarters skos:definition "A country, state, province, etc., or local place in which an organization has its headquarters."@en .

ElementsGr2:nameOfTheCorporateBody skos:definition "A word, character, or group of words and/or characters by which a corporate body is known."@en .

ElementsGr2:preferredNameForTheCorporateBody skos:definition "The name or form of name chosen as the basis for the authorized access point representing that body."@en .

ElementsGr2:variantNameForTheCorporateBody skos:definition """A name or form of name by which a corporate body is known that differs from the name or form of name chosen as the preferred

name."""@en .

ElementsGr2:nameOfTheFamily skos:definition "A word, character, or group of words and/or characters by which a family is known."@en .

ElementsGr2:preferredNameForTheFamily skos:definition "The name or form of name chosen as the basis for the authorized access point representing that family."@en .

ElementsGr2:variantNameForTheFamily skos:definition "A name or form of name by which a family is known that differs from the name or form of name chosen as the preferred name."@en .

ElementsGr2:nameOfThePerson skos:definition "A word, character, or group of words and/or characters by which a person is known."@en .

ElementsGr2:preferredNameForThePerson skos:definition "The name or form of name chosen as the basis for the authorized access point representing that person."@en .

ElementsGr2:variantNameForThePerson skos:definition "A name or form of name by which a person is known that differs from the name or form of name chosen as the preferred name."@en .

ElementsGr2:note skos:definition "An annotation providing additional information relating to data recorded in another element."@en .

ElementsGr2:numberOfAConferenceEtc skos:definition "A designation of the sequencing of a conference, etc., within a series of conferences, etc."@en .

ElementsGr2:otherDesignationAssociatedWithTheCorporateBody skos:definition "A word, phrase, or abbreviation indicating incorporation or legal status of a corporate body, or any term serving to differentiate the body from other corporate bodies, persons, etc."@en .

ElementsGr2:otherDesignationAssociatedWithThePerson skos:definition "A term other than a title that is associated with a persons name."@en .

ElementsGr2:placeAssociatedWithTheFamily skos:definition "A place where a family resides or has resided or has some connection."@en .

ElementsGr2:placeOfResidence skos:definition "A town, city, province, state, and/or country in which a person resides or has resided."@en .

ElementsGr2:professionOrOccupation skos:definition "A profession or occupation in which a person works or has worked."@en .

ElementsGr2:prominentMemberOfTheFamily skos:definition "A well-known individual who is a member of a family."@en .

ElementsGr2:scopeOfUsage skos:definition "The type or form of work associated with the name designated as the preferred name for a person, family, or corporate body."@en .

ElementsGr2:titleOfThePerson skos:definition "A word or phrase indicative of royalty, nobility, or ecclesiastical rank or office, or a term of address for a person of religious vocation."@en .

ElementsGr2:typeOfFamily skos:definition "A categorization or generic descriptor for the type of family."@en .

ElementsGr2:undifferentiatedNameIndicator skos:definition "A categorization indicating that the core elements recorded are insufficient to differentiate between two or more entities with the same name."@en .

ElementsGr2:undifferentiatedNameIndicatorPerson skos:definition "A categorization indicating that the core elements recorded are insufficient to differentiate between two or more persons with the same name."@en .

ElementsGr2:undifferentiatedNameIndicatorCorporateBody skos:definition "A categorization indicating that the core elements recorded are insufficient to differentiate between two or more corporate bodies with the same name."@en .

ElementsGr2:undifferentiatedNameIndicatorFamily skos:definition "A categorization indicating that the core elements recorded are insufficient to differentiate between two or more families with the same name."@en .

frbr_core:Endeavour skos:definition "Any of the products of artistic or creative endeavour."@en .

frbr_core:ResponsibleEntity skos:definition "One responsible for the creation, production, distribution or maintenance of artistic or creative content."@en .

frbr_core:Subject skos:definition "Something that may serve as the subject of a work."@en .

frbr_core:Item skos:definition "An exemplar of a single manifestation."@en .

frbr_core:CorporateBody skos:definition "An organization or group of individuals and/or other organizations."@en .

frbr_core:Person skos:definition "A living or dead individual."@en .

frbr_core:Object skos:definition "A tangible or material thing."@en .

frbr_core:Concept skos:definition "An abstract idea or notion."@en .

frbr_core:relatedEndeavour skos:definition "Another endeavour that is related in some way to an endeavour."@en .

frbr_core:realization skos:definition "An expression that is an intellectual or artistic realization of a work."@en .

frbr_core:realizationOf skos:definition "The work that has been realized by an expression."@en .

frbr_core:embodiment skos:definition "A manifestation that embodies an expression."@en .

frbr_core:embodimentOf skos:definition "An expression that is embodied by a manifestation."@en .

frbr_core:exemplar skos:definition "An item that is an exemplar of a manifestation."@en .

frbr_core:exemplarOf skos:definition "The manifestation that is exemplified by a item."@en .

frbr_core:reproduction skos:definition "A reproduction of a manifestation or item."@en .

frbr_core:reproductionOf skos:definition "A manifestation or item that is reproduced."@en .

frbr_core:successor skos:definition "A successor to a work or expression."@en .

frbr_core:successorOf skos:definition "A work or expression that is succeeded."@en .

frbr_core:supplement skos:definition "A supplement to a work or expression."@en .

frbr_core:supplementOf skos:definition "A work or expression that is supplemented."@en .

frbr_core:complement skos:definition "A complement to a work or expression."@en .

frbr_core:complementOf skos:definition "A work or expression that is complemented."@en .

frbr_core:summarization skos:definition "A summarization of a work or expression."@en .

frbr_core:summarizationOf skos:definition "A work or expression that is summarized."@en .

frbr_core:adaption skos:definition "An adaption of a work or expression."@en .

frbr_core:adaptionOf skos:definition "A work or expression that is adapted."@en .

frbr_core:transformation skos:definition "A transformation of a work or expression."@en .

frbr_core:transformationOf skos:definition "A work or expression that is transformed."@en .

frbr_core:imitation skos:definition "An imitation of a work or expression."@en .

frbr_core:imitationOf skos:definition "A work or expression that is imitated."@en .

frbr_core:abridgement skos:definition "An abridgment of an expression."@en .

frbr_core:abridgementOf skos:definition "An expression that is abridged."@en .

frbr_core:revision skos:definition "A revision of an expression."@en .

frbr_core:revisionOf skos:definition "An expression that is revised."@en .

frbr_core:translation skos:definition "A translation of an expression."@en .

frbr_core:translationOf skos:definition "An expression that is translated."@en .

frbr_core:arrangement skos:definition "An arrangement of an expression."@en .

frbr_core:arrangementOf skos:definition "An expression that is arranged."@en .

frbr_core:alternate skos:definition "An alternative to a manifestation."@en .

frbr_core:alternateOf skos:definition "A manifestation that is alternated."@en .

frbr_core:reconfiguration skos:definition "A recongifuration of an item."@en .

frbr_core:reconfigurationOf skos:definition "An item that is reconfigured."@en .

frbr_core:part skos:definition "A part of an endeavour."@en .

frbr_core:partOf skos:definition "An endeavour incorporating an endeavour."@en .

frbr_core:responsibleEntity skos:definition "An entity in some way responsible for an endeavour."@en .

frbr_core:responsibleEntityOf skos:definition "An endeavour that is the responsibility of an entity."@en .

frbr_core:creator skos:definition "An entity in some way responsible for the creation of a work."@en .

frbr_core:creatorOf skos:definition "A work that was in some way created by of an entity."@en .

frbr_core:realizer skos:definition "An entity in some way responsible for realizing an expression."@en .

frbr_core:realizerOf skos:definition "An expression that was in some way realized by an entity."@en .

frbr_core:producer skos:definition "An entity in some way responsible for producing a manifestation."@en .

frbr_core:producerOf skos:definition "A manifestation that was in some way produced an entity."@en .

frbr_core:owner skos:definition "An entity that owns an item."@en .

frbr_core:ownerOf skos:definition "An item that is in some way owned an entity."@en .

frbr_core:subject skos:definition "The subject of a work."@en .

status:1002 skos:prefLabel "New-Proposed"@en .

skos:Concept skos:changeNote _:node2 .

skos:altLabel skos:changeNote _:node5 .

skos:definition skos:changeNote _:node11 .

skos:hiddenLabel skos:changeNote _:node16 .

skos:prefLabel skos:changeNote _:node27 .

skos:broadMatch skos:changeNote _:node6 .

skos:broader skos:changeNote _:node7 .

skos:mappingRelation skos:changeNote _:node19 .

skos:broaderTransitive skos:changeNote _:node8 .

skos:narrower skos:changeNote _:node23 .

skos:narrowerTransitive skos:changeNote _:node24 .

skos:semanticRelation skos:changeNote _:node31 .

skos:changeNote skos:changeNote _:node9 .

skos:note skos:changeNote _:node26 .

skos:closeMatch skos:changeNote _:node10 .

skos:editorialNote skos:changeNote _:node12 .

skos:exactMatch skos:changeNote _:node13 .

skos:example skos:changeNote _:node14 .

skos:hasTopConcept skos:changeNote _:node15 .

skos:ConceptScheme skos:changeNote _:node3 .

skos:historyNote skos:changeNote _:node17 .

skos:inScheme skos:changeNote _:node18 .

skos:member skos:changeNote _:node20 .

skos:Collection skos:changeNote _:node1 .

skos:memberList skos:changeNote _:node21 .

skos:OrderedCollection skos:changeNote _:node4 .

skos:narrowMatch skos:changeNote _:node22 .

skos:related skos:changeNote _:node28 .

skos:relatedMatch skos:changeNote _:node29 .

skos:scopeNote skos:changeNote _:node30 .

skos:topConceptOf skos:changeNote _:node32 .

skos:notation skos:changeNote _:node25 .

frbr_core:Event skos:changeNote _:genid-38640ccbd5eb49418600e8d7df2cf451-mor50bd147e3f23c,
    _:genid-38640ccbd5eb49418600e8d7df2cf451-mor50bd147e3f2de .

frbr_core:Expression skos:changeNote _:genid-38640ccbd5eb49418600e8d7df2cf451-mor50bd147e3e496,
    _:genid-38640ccbd5eb49418600e8d7df2cf451-mor50bd147e3e4e2, _:genid-38640ccbd5eb49418600e8d7df2cf451-mor50bd147e3e52e .

frbr_core:Manifestation skos:changeNote _:genid-38640ccbd5eb49418600e8d7df2cf451-mor50bd147e3e5a5,
    _:genid-38640ccbd5eb49418600e8d7df2cf451-mor50bd147e3e5f3, _:genid-38640ccbd5eb49418600e8d7df2cf451-mor50bd147e3e641 .

frbr_core:Place skos:changeNote _:genid-38640ccbd5eb49418600e8d7df2cf451-mor50bd147e3f354,
    _:genid-38640ccbd5eb49418600e8d7df2cf451-mor50bd147e3f3a9, _:genid-38640ccbd5eb49418600e8d7df2cf451-mor50bd147e3f43f .

frbr_core:Work skos:changeNote _:genid-38640ccbd5eb49418600e8d7df2cf451-mor50bd147e3e336,
    _:genid-38640ccbd5eb49418600e8d7df2cf451-mor50bd147e3e383, _:genid-38640ccbd5eb49418600e8d7df2cf451-mor50bd147e3e424 .

<http://purl.org/vocab/frbr/core> skos:changeNote _:genid-38640ccbd5eb49418600e8d7df2cf451-mor50bd147e3dfc0 .

frbr_core:Endeavour skos:changeNote _:genid-38640ccbd5eb49418600e8d7df2cf451-mor50bd147e3e223,
    _:genid-38640ccbd5eb49418600e8d7df2cf451-mor50bd147e3e26f, _:genid-38640ccbd5eb49418600e8d7df2cf451-mor50bd147e3e2bf .

frbr_core:ResponsibleEntity skos:changeNote _:genid-38640ccbd5eb49418600e8d7df2cf451-mor50bd147e3e925,
    _:genid-38640ccbd5eb49418600e8d7df2cf451-mor50bd147e3e971, _:genid-38640ccbd5eb49418600e8d7df2cf451-mor50bd147e3e9bd .

frbr_core:Subject skos:changeNote _:genid-38640ccbd5eb49418600e8d7df2cf451-mor50bd147e3ee70,
    _:genid-38640ccbd5eb49418600e8d7df2cf451-mor50bd147e3eebb, _:genid-38640ccbd5eb49418600e8d7df2cf451-mor50bd147e3ef08 .

frbr_core:Item skos:changeNote _:genid-38640ccbd5eb49418600e8d7df2cf451-mor50bd147e3e6b4,
    _:genid-38640ccbd5eb49418600e8d7df2cf451-mor50bd147e3e74b, _:genid-38640ccbd5eb49418600e8d7df2cf451-mor50bd147e3e798 .

frbr_core:CorporateBody skos:changeNote _:genid-38640ccbd5eb49418600e8d7df2cf451-mor50bd147e3ec08,
    _:genid-38640ccbd5eb49418600e8d7df2cf451-mor50bd147e3ec53, _:genid-38640ccbd5eb49418600e8d7df2cf451-mor50bd147e3ec9f .

frbr_core:Person skos:changeNote _:genid-38640ccbd5eb49418600e8d7df2cf451-mor50bd147e3ea2b,
    _:genid-38640ccbd5eb49418600e8d7df2cf451-mor50bd147e3ea78, _:genid-38640ccbd5eb49418600e8d7df2cf451-mor50bd147e3eac9 .

frbr_core:Object skos:changeNote _:genid-38640ccbd5eb49418600e8d7df2cf451-mor50bd147e3f0e2,
    _:genid-38640ccbd5eb49418600e8d7df2cf451-mor50bd147e3f12e, _:genid-38640ccbd5eb49418600e8d7df2cf451-mor50bd147e3f1c4 .

frbr_core:Concept skos:changeNote _:genid-38640ccbd5eb49418600e8d7df2cf451-mor50bd147e3ef7f,
    _:genid-38640ccbd5eb49418600e8d7df2cf451-mor50bd147e3efcc, _:genid-38640ccbd5eb49418600e8d7df2cf451-mor50bd147e3f065 .

frbr_core:relatedEndeavour skos:changeNote _:genid-38640ccbd5eb49418600e8d7df2cf451-mor50bd147e3f566,
    _:genid-38640ccbd5eb49418600e8d7df2cf451-mor50bd147e3f5b4 .

frbr_core:realization skos:changeNote _:genid-38640ccbd5eb49418600e8d7df2cf451-mor50bd147e3f622,
    _:genid-38640ccbd5eb49418600e8d7df2cf451-mor50bd147e3f66c .

frbr_core:realizationOf skos:changeNote _:genid-38640ccbd5eb49418600e8d7df2cf451-mor50bd147e3f6da,
    _:genid-38640ccbd5eb49418600e8d7df2cf451-mor50bd147e3f729 .

frbr_core:embodiment skos:changeNote _:genid-38640ccbd5eb49418600e8d7df2cf451-mor50bd147e3f797,
    _:genid-38640ccbd5eb49418600e8d7df2cf451-mor50bd147e3f7e2 .

frbr_core:embodimentOf skos:changeNote _:genid-38640ccbd5eb49418600e8d7df2cf451-mor50bd147e3f852,
    _:genid-38640ccbd5eb49418600e8d7df2cf451-mor50bd147e3f89d .

frbr_core:exemplar skos:changeNote _:genid-38640ccbd5eb49418600e8d7df2cf451-mor50bd147e3f90e,
    _:genid-38640ccbd5eb49418600e8d7df2cf451-mor50bd147e3f95a .

frbr_core:exemplarOf skos:changeNote _:genid-38640ccbd5eb49418600e8d7df2cf451-mor50bd147e3f9c6 .

_:genid-38640ccbd5eb49418600e8d7df2cf451-mor50bd147e3f9c6 dc:creator "Ian Davis" .

frbr_core:exemplarOf skos:changeNote _:genid-38640ccbd5eb49418600e8d7df2cf451-mor50bd147e3fa11 .

_:genid-38640ccbd5eb49418600e8d7df2cf451-mor50bd147e3fa11 dc:creator "Ian Davis" .

frbr_core:reproduction skos:changeNote _:genid-38640ccbd5eb49418600e8d7df2cf451-mor50bd147e3fc25 .

_:genid-38640ccbd5eb49418600e8d7df2cf451-mor50bd147e3fc25 dc:creator "Ian Davis" .

frbr_core:reproduction skos:changeNote _:genid-38640ccbd5eb49418600e8d7df2cf451-mor50bd147e3fc70 .

_:genid-38640ccbd5eb49418600e8d7df2cf451-mor50bd147e3fc70 dc:creator "Ian Davis" .

frbr_core:reproductionOf skos:changeNote _:genid-38640ccbd5eb49418600e8d7df2cf451-mor50bd147e3fed1 .

_:genid-38640ccbd5eb49418600e8d7df2cf451-mor50bd147e3fed1 dc:creator "Ian Davis" .

frbr_core:reproductionOf skos:changeNote _:genid-38640ccbd5eb49418600e8d7df2cf451-mor50bd147e3ff1d .

_:genid-38640ccbd5eb49418600e8d7df2cf451-mor50bd147e3ff1d dc:creator "Ian Davis" .

frbr_core:successor skos:changeNote _:genid-38640ccbd5eb49418600e8d7df2cf451-mor50bd147e40171 .

_:genid-38640ccbd5eb49418600e8d7df2cf451-mor50bd147e40171 dc:creator "Ian Davis" .

frbr_core:successor skos:changeNote _:genid-38640ccbd5eb49418600e8d7df2cf451-mor50bd147e401bd .

_:genid-38640ccbd5eb49418600e8d7df2cf451-mor50bd147e401bd dc:creator "Ian Davis" .

frbr_core:successorOf skos:changeNote _:genid-38640ccbd5eb49418600e8d7df2cf451-mor50bd147e4041a .

_:genid-38640ccbd5eb49418600e8d7df2cf451-mor50bd147e4041a dc:creator "Ian Davis" .

frbr_core:successorOf skos:changeNote _:genid-38640ccbd5eb49418600e8d7df2cf451-mor50bd147e40467 .

_:genid-38640ccbd5eb49418600e8d7df2cf451-mor50bd147e40467 dc:creator "Ian Davis" .

frbr_core:supplement skos:changeNote _:genid-38640ccbd5eb49418600e8d7df2cf451-mor50bd147e406be .

_:genid-38640ccbd5eb49418600e8d7df2cf451-mor50bd147e406be dc:creator "Ian Davis" .

frbr_core:supplement skos:changeNote _:genid-38640ccbd5eb49418600e8d7df2cf451-mor50bd147e4070b .

_:genid-38640ccbd5eb49418600e8d7df2cf451-mor50bd147e4070b dc:creator "Ian Davis" .

frbr_core:supplementOf skos:changeNote _:genid-38640ccbd5eb49418600e8d7df2cf451-mor50bd147e40962 .

_:genid-38640ccbd5eb49418600e8d7df2cf451-mor50bd147e40962 dc:creator "Ian Davis" .

frbr_core:supplementOf skos:changeNote _:genid-38640ccbd5eb49418600e8d7df2cf451-mor50bd147e409ad .

_:genid-38640ccbd5eb49418600e8d7df2cf451-mor50bd147e409ad dc:creator "Ian Davis" .

frbr_core:complement skos:changeNote _:genid-38640ccbd5eb49418600e8d7df2cf451-mor50bd147e40c00 .

_:genid-38640ccbd5eb49418600e8d7df2cf451-mor50bd147e40c00 dc:creator "Ian Davis" .

frbr_core:complement skos:changeNote _:genid-38640ccbd5eb49418600e8d7df2cf451-mor50bd147e40c4b .

_:genid-38640ccbd5eb49418600e8d7df2cf451-mor50bd147e40c4b dc:creator "Ian Davis" .

frbr_core:complementOf skos:changeNote _:genid-38640ccbd5eb49418600e8d7df2cf451-mor50bd147e40ea3 .

_:genid-38640ccbd5eb49418600e8d7df2cf451-mor50bd147e40ea3 dc:creator "Ian Davis" .

frbr_core:complementOf skos:changeNote _:genid-38640ccbd5eb49418600e8d7df2cf451-mor50bd147e40eee .

_:genid-38640ccbd5eb49418600e8d7df2cf451-mor50bd147e40eee dc:creator "Ian Davis" .

frbr_core:summarization skos:changeNote _:genid-38640ccbd5eb49418600e8d7df2cf451-mor50bd147e41141 .

_:genid-38640ccbd5eb49418600e8d7df2cf451-mor50bd147e41141 dc:creator "Ian Davis" .

frbr_core:summarization skos:changeNote _:genid-38640ccbd5eb49418600e8d7df2cf451-mor50bd147e4118e .

_:genid-38640ccbd5eb49418600e8d7df2cf451-mor50bd147e4118e dc:creator "Ian Davis" .

frbr_core:summarizationOf skos:changeNote _:genid-38640ccbd5eb49418600e8d7df2cf451-mor50bd147e413f6 .

_:genid-38640ccbd5eb49418600e8d7df2cf451-mor50bd147e413f6 dc:creator "Ian Davis" .

frbr_core:summarizationOf skos:changeNote _:genid-38640ccbd5eb49418600e8d7df2cf451-mor50bd147e41442 .

_:genid-38640ccbd5eb49418600e8d7df2cf451-mor50bd147e41442 dc:creator "Ian Davis" .

frbr_core:adaption skos:changeNote _:genid-38640ccbd5eb49418600e8d7df2cf451-mor50bd147e416a1 .

_:genid-38640ccbd5eb49418600e8d7df2cf451-mor50bd147e416a1 dc:creator "Ian Davis" .

frbr_core:adaption skos:changeNote _:genid-38640ccbd5eb49418600e8d7df2cf451-mor50bd147e416ec .

_:genid-38640ccbd5eb49418600e8d7df2cf451-mor50bd147e416ec dc:creator "Ian Davis" .

frbr_core:adaptionOf skos:changeNote _:genid-38640ccbd5eb49418600e8d7df2cf451-mor50bd147e4193f .

_:genid-38640ccbd5eb49418600e8d7df2cf451-mor50bd147e4193f dc:creator "Ian Davis" .

frbr_core:adaptionOf skos:changeNote _:genid-38640ccbd5eb49418600e8d7df2cf451-mor50bd147e4198a .

_:genid-38640ccbd5eb49418600e8d7df2cf451-mor50bd147e4198a dc:creator "Ian Davis" .

frbr_core:transformation skos:changeNote _:genid-38640ccbd5eb49418600e8d7df2cf451-mor50bd147e41bde .

_:genid-38640ccbd5eb49418600e8d7df2cf451-mor50bd147e41bde dc:creator "Ian Davis" .

frbr_core:transformation skos:changeNote _:genid-38640ccbd5eb49418600e8d7df2cf451-mor50bd147e41c2a .

_:genid-38640ccbd5eb49418600e8d7df2cf451-mor50bd147e41c2a dc:creator "Ian Davis" .

frbr_core:transformationOf skos:changeNote _:genid-38640ccbd5eb49418600e8d7df2cf451-mor50bd147e41e80 .

_:genid-38640ccbd5eb49418600e8d7df2cf451-mor50bd147e41e80 dc:creator "Ian Davis" .

frbr_core:transformationOf skos:changeNote _:genid-38640ccbd5eb49418600e8d7df2cf451-mor50bd147e41ecb .

_:genid-38640ccbd5eb49418600e8d7df2cf451-mor50bd147e41ecb dc:creator "Ian Davis" .

frbr_core:imitation skos:changeNote _:genid-38640ccbd5eb49418600e8d7df2cf451-mor50bd147e42120 .

_:genid-38640ccbd5eb49418600e8d7df2cf451-mor50bd147e42120 dc:creator "Ian Davis" .

frbr_core:imitation skos:changeNote _:genid-38640ccbd5eb49418600e8d7df2cf451-mor50bd147e42174 .

_:genid-38640ccbd5eb49418600e8d7df2cf451-mor50bd147e42174 dc:creator "Ian Davis" .

frbr_core:imitationOf skos:changeNote _:genid-38640ccbd5eb49418600e8d7df2cf451-mor50bd147e423cc .

_:genid-38640ccbd5eb49418600e8d7df2cf451-mor50bd147e423cc dc:creator "Ian Davis" .

frbr_core:imitationOf skos:changeNote _:genid-38640ccbd5eb49418600e8d7df2cf451-mor50bd147e42417 .

_:genid-38640ccbd5eb49418600e8d7df2cf451-mor50bd147e42417 dc:creator "Ian Davis" .

frbr_core:abridgement skos:changeNote _:genid-38640ccbd5eb49418600e8d7df2cf451-mor50bd147e424d0 .

_:genid-38640ccbd5eb49418600e8d7df2cf451-mor50bd147e424d0 dc:creator "Ian Davis" .

frbr_core:abridgement skos:changeNote _:genid-38640ccbd5eb49418600e8d7df2cf451-mor50bd147e4251f .

_:genid-38640ccbd5eb49418600e8d7df2cf451-mor50bd147e4251f dc:creator "Ian Davis" .

frbr_core:abridgementOf skos:changeNote _:genid-38640ccbd5eb49418600e8d7df2cf451-mor50bd147e425e9 .

_:genid-38640ccbd5eb49418600e8d7df2cf451-mor50bd147e425e9 dc:creator "Ian Davis" .

frbr_core:abridgementOf skos:changeNote _:genid-38640ccbd5eb49418600e8d7df2cf451-mor50bd147e42635 .

_:genid-38640ccbd5eb49418600e8d7df2cf451-mor50bd147e42635 dc:creator "Ian Davis" .

frbr_core:revision skos:changeNote _:genid-38640ccbd5eb49418600e8d7df2cf451-mor50bd147e426f2 .

_:genid-38640ccbd5eb49418600e8d7df2cf451-mor50bd147e426f2 dc:creator "Ian Davis" .

frbr_core:revision skos:changeNote _:genid-38640ccbd5eb49418600e8d7df2cf451-mor50bd147e4273d .

_:genid-38640ccbd5eb49418600e8d7df2cf451-mor50bd147e4273d dc:creator "Ian Davis" .

frbr_core:revisionOf skos:changeNote _:genid-38640ccbd5eb49418600e8d7df2cf451-mor50bd147e427f6 .

_:genid-38640ccbd5eb49418600e8d7df2cf451-mor50bd147e427f6 dc:creator "Ian Davis" .

frbr_core:revisionOf skos:changeNote _:genid-38640ccbd5eb49418600e8d7df2cf451-mor50bd147e42842 .

_:genid-38640ccbd5eb49418600e8d7df2cf451-mor50bd147e42842 dc:creator "Ian Davis" .

frbr_core:translation skos:changeNote _:genid-38640ccbd5eb49418600e8d7df2cf451-mor50bd147e428fb .

_:genid-38640ccbd5eb49418600e8d7df2cf451-mor50bd147e428fb dc:creator "Ian Davis" .

frbr_core:translation skos:changeNote _:genid-38640ccbd5eb49418600e8d7df2cf451-mor50bd147e42948 .

_:genid-38640ccbd5eb49418600e8d7df2cf451-mor50bd147e42948 dc:creator "Ian Davis" .

frbr_core:translationOf skos:changeNote _:genid-38640ccbd5eb49418600e8d7df2cf451-mor50bd147e42a01 .

_:genid-38640ccbd5eb49418600e8d7df2cf451-mor50bd147e42a01 dc:creator "Ian Davis" .

frbr_core:translationOf skos:changeNote _:genid-38640ccbd5eb49418600e8d7df2cf451-mor50bd147e42a4f .

_:genid-38640ccbd5eb49418600e8d7df2cf451-mor50bd147e42a4f dc:creator "Ian Davis" .

frbr_core:arrangement skos:changeNote _:genid-38640ccbd5eb49418600e8d7df2cf451-mor50bd147e42b08 .

_:genid-38640ccbd5eb49418600e8d7df2cf451-mor50bd147e42b08 dc:creator "Ian Davis" .

frbr_core:arrangement skos:changeNote _:genid-38640ccbd5eb49418600e8d7df2cf451-mor50bd147e42b58 .

_:genid-38640ccbd5eb49418600e8d7df2cf451-mor50bd147e42b58 dc:creator "Ian Davis" .

frbr_core:arrangementOf skos:changeNote _:genid-38640ccbd5eb49418600e8d7df2cf451-mor50bd147e42c11 .

_:genid-38640ccbd5eb49418600e8d7df2cf451-mor50bd147e42c11 dc:creator "Ian Davis" .

frbr_core:arrangementOf skos:changeNote _:genid-38640ccbd5eb49418600e8d7df2cf451-mor50bd147e42c5d .

_:genid-38640ccbd5eb49418600e8d7df2cf451-mor50bd147e42c5d dc:creator "Ian Davis" .

frbr_core:part skos:changeNote _:genid-38640ccbd5eb49418600e8d7df2cf451-mor50bd147e42d99 .

_:genid-38640ccbd5eb49418600e8d7df2cf451-mor50bd147e42d99 dc:creator "Ian Davis" .

frbr_core:part skos:changeNote _:genid-38640ccbd5eb49418600e8d7df2cf451-mor50bd147e42de7 .

_:genid-38640ccbd5eb49418600e8d7df2cf451-mor50bd147e42de7 dc:creator "Ian Davis" .

frbr_core:partOf skos:changeNote _:genid-38640ccbd5eb49418600e8d7df2cf451-mor50bd147e42e52 .

_:genid-38640ccbd5eb49418600e8d7df2cf451-mor50bd147e42e52 dc:creator "Ian Davis" .

frbr_core:partOf skos:changeNote _:genid-38640ccbd5eb49418600e8d7df2cf451-mor50bd147e42e9d .

_:genid-38640ccbd5eb49418600e8d7df2cf451-mor50bd147e42e9d dc:creator "Ian Davis" .

frbr_core:responsibleEntity skos:changeNote _:genid-38640ccbd5eb49418600e8d7df2cf451-mor50bd147e42f0c .

_:genid-38640ccbd5eb49418600e8d7df2cf451-mor50bd147e42f0c dc:creator "Ian Davis" .

frbr_core:responsibleEntity skos:changeNote _:genid-38640ccbd5eb49418600e8d7df2cf451-mor50bd147e42f58 .

_:genid-38640ccbd5eb49418600e8d7df2cf451-mor50bd147e42f58 dc:creator "Ian Davis" .

frbr_core:responsibleEntityOf skos:changeNote _:genid-38640ccbd5eb49418600e8d7df2cf451-mor50bd147e42fc3 .

_:genid-38640ccbd5eb49418600e8d7df2cf451-mor50bd147e42fc3 dc:creator "Ian Davis" .

frbr_core:responsibleEntityOf skos:changeNote _:genid-38640ccbd5eb49418600e8d7df2cf451-mor50bd147e4300e .

_:genid-38640ccbd5eb49418600e8d7df2cf451-mor50bd147e4300e dc:creator "Ian Davis" .

frbr_core:creator skos:changeNote _:genid-38640ccbd5eb49418600e8d7df2cf451-mor50bd147e4307c .

_:genid-38640ccbd5eb49418600e8d7df2cf451-mor50bd147e4307c dc:creator "Ian Davis" .

frbr_core:creator skos:changeNote _:genid-38640ccbd5eb49418600e8d7df2cf451-mor50bd147e430ca .

_:genid-38640ccbd5eb49418600e8d7df2cf451-mor50bd147e430ca dc:creator "Ian Davis" .

frbr_core:creatorOf skos:changeNote _:genid-38640ccbd5eb49418600e8d7df2cf451-mor50bd147e43138 .

_:genid-38640ccbd5eb49418600e8d7df2cf451-mor50bd147e43138 dc:creator "Ian Davis" .

frbr_core:creatorOf skos:changeNote _:genid-38640ccbd5eb49418600e8d7df2cf451-mor50bd147e4318b .

_:genid-38640ccbd5eb49418600e8d7df2cf451-mor50bd147e4318b dc:creator "Ian Davis" .

frbr_core:realizer skos:changeNote _:genid-38640ccbd5eb49418600e8d7df2cf451-mor50bd147e43202 .

_:genid-38640ccbd5eb49418600e8d7df2cf451-mor50bd147e43202 dc:creator "Ian Davis" .

frbr_core:realizer skos:changeNote _:genid-38640ccbd5eb49418600e8d7df2cf451-mor50bd147e4324e .

_:genid-38640ccbd5eb49418600e8d7df2cf451-mor50bd147e4324e dc:creator "Ian Davis" .

frbr_core:realizerOf skos:changeNote _:genid-38640ccbd5eb49418600e8d7df2cf451-mor50bd147e432be .

_:genid-38640ccbd5eb49418600e8d7df2cf451-mor50bd147e432be dc:creator "Ian Davis" .

frbr_core:realizerOf skos:changeNote _:genid-38640ccbd5eb49418600e8d7df2cf451-mor50bd147e4330c .

_:genid-38640ccbd5eb49418600e8d7df2cf451-mor50bd147e4330c dc:creator "Ian Davis" .

frbr_core:producer skos:changeNote _:genid-38640ccbd5eb49418600e8d7df2cf451-mor50bd147e4337b .

_:genid-38640ccbd5eb49418600e8d7df2cf451-mor50bd147e4337b dc:creator "Ian Davis" .

frbr_core:producer skos:changeNote _:genid-38640ccbd5eb49418600e8d7df2cf451-mor50bd147e433c7 .

_:genid-38640ccbd5eb49418600e8d7df2cf451-mor50bd147e433c7 dc:creator "Ian Davis" .

frbr_core:producerOf skos:changeNote _:genid-38640ccbd5eb49418600e8d7df2cf451-mor50bd147e43436 .

_:genid-38640ccbd5eb49418600e8d7df2cf451-mor50bd147e43436 dc:creator "Ian Davis" .

frbr_core:producerOf skos:changeNote _:genid-38640ccbd5eb49418600e8d7df2cf451-mor50bd147e43481 .

_:genid-38640ccbd5eb49418600e8d7df2cf451-mor50bd147e43481 dc:creator "Ian Davis" .

frbr_core:owner skos:changeNote _:genid-38640ccbd5eb49418600e8d7df2cf451-mor50bd147e434fa .

_:genid-38640ccbd5eb49418600e8d7df2cf451-mor50bd147e434fa dc:creator "Ian Davis" .

frbr_core:owner skos:changeNote _:genid-38640ccbd5eb49418600e8d7df2cf451-mor50bd147e43545 .

_:genid-38640ccbd5eb49418600e8d7df2cf451-mor50bd147e43545 dc:creator "Ian Davis" .

frbr_core:ownerOf skos:changeNote _:genid-38640ccbd5eb49418600e8d7df2cf451-mor50bd147e435b5 .

_:genid-38640ccbd5eb49418600e8d7df2cf451-mor50bd147e435b5 dc:creator "Ian Davis" .

frbr_core:ownerOf skos:changeNote _:genid-38640ccbd5eb49418600e8d7df2cf451-mor50bd147e43600 .

_:genid-38640ccbd5eb49418600e8d7df2cf451-mor50bd147e43600 dc:creator "Ian Davis" .

frbr_core:subject skos:changeNote _:genid-38640ccbd5eb49418600e8d7df2cf451-mor50bd147e4377b .

_:genid-38640ccbd5eb49418600e8d7df2cf451-mor50bd147e4377b dc:creator "Ian Davis" .

frbr_core:subject skos:changeNote _:genid-38640ccbd5eb49418600e8d7df2cf451-mor50bd147e437c6 .

_:genid-38640ccbd5eb49418600e8d7df2cf451-mor50bd147e437c6 dc:creator "Ian Davis" .

<http://rdvocab.info/ElementsGr2> skos:note "This is the provisional registration of the RDA Group 2 Element Vocabulary, managed by the DCMI/RDA Task Group. "@en .

<http://purl.org/vocab/frbr/core> skos:example <file:///var/www/vocab.org/www/htdocs/frbr/frbr-example-film-20050809.html>;
  skos:historyNote _:genid-38640ccbd5eb49418600e8d7df2cf451-mor50bd147e3df74 .

frbr_core:Event skos:historyNote _:genid-38640ccbd5eb49418600e8d7df2cf451-mor50bd147e3f292;
  owl:disjointWith frbr_core:Place, frbr_core:Object, frbr_core:Concept .

frbr_core:Place skos:historyNote _:genid-38640ccbd5eb49418600e8d7df2cf451-mor50bd147e3f3f4 .

frbr_core:Work skos:historyNote _:genid-38640ccbd5eb49418600e8d7df2cf451-mor50bd147e3e3d8 .

frbr_core:Item skos:historyNote _:genid-38640ccbd5eb49418600e8d7df2cf451-mor50bd147e3e700,
    _:genid-38640ccbd5eb49418600e8d7df2cf451-mor50bd147e3e7e4 .

frbr_core:Object skos:historyNote _:genid-38640ccbd5eb49418600e8d7df2cf451-mor50bd147e3f17a .

frbr_core:Concept skos:historyNote _:genid-38640ccbd5eb49418600e8d7df2cf451-mor50bd147e3f019 .

frbr_core:reproduction skos:historyNote _:genid-38640ccbd5eb49418600e8d7df2cf451-mor50bd147e3fcbc .

_:genid-38640ccbd5eb49418600e8d7df2cf451-mor50bd147e3fcbc dc:creator "Ian Davis" .

frbr_core:reproductionOf skos:historyNote _:genid-38640ccbd5eb49418600e8d7df2cf451-mor50bd147e3ff6a .

_:genid-38640ccbd5eb49418600e8d7df2cf451-mor50bd147e3ff6a dc:creator "Ian Davis" .

frbr_core:successor skos:historyNote _:genid-38640ccbd5eb49418600e8d7df2cf451-mor50bd147e40209 .

_:genid-38640ccbd5eb49418600e8d7df2cf451-mor50bd147e40209 dc:creator "Ian Davis" .

frbr_core:successorOf skos:historyNote _:genid-38640ccbd5eb49418600e8d7df2cf451-mor50bd147e404b3 .

_:genid-38640ccbd5eb49418600e8d7df2cf451-mor50bd147e404b3 dc:creator "Ian Davis" .

frbr_core:supplement skos:historyNote _:genid-38640ccbd5eb49418600e8d7df2cf451-mor50bd147e40757 .

_:genid-38640ccbd5eb49418600e8d7df2cf451-mor50bd147e40757 dc:creator "Ian Davis" .

frbr_core:supplementOf skos:historyNote _:genid-38640ccbd5eb49418600e8d7df2cf451-mor50bd147e409fa .

_:genid-38640ccbd5eb49418600e8d7df2cf451-mor50bd147e409fa dc:creator "Ian Davis" .

frbr_core:complement skos:historyNote _:genid-38640ccbd5eb49418600e8d7df2cf451-mor50bd147e40c97 .

_:genid-38640ccbd5eb49418600e8d7df2cf451-mor50bd147e40c97 dc:creator "Ian Davis" .

frbr_core:complementOf skos:historyNote _:genid-38640ccbd5eb49418600e8d7df2cf451-mor50bd147e40f3a .

_:genid-38640ccbd5eb49418600e8d7df2cf451-mor50bd147e40f3a dc:creator "Ian Davis" .

frbr_core:summarization skos:historyNote _:genid-38640ccbd5eb49418600e8d7df2cf451-mor50bd147e411e1 .

_:genid-38640ccbd5eb49418600e8d7df2cf451-mor50bd147e411e1 dc:creator "Ian Davis" .

frbr_core:summarizationOf skos:historyNote _:genid-38640ccbd5eb49418600e8d7df2cf451-mor50bd147e4148d .

_:genid-38640ccbd5eb49418600e8d7df2cf451-mor50bd147e4148d dc:creator "Ian Davis" .

frbr_core:adaption skos:historyNote _:genid-38640ccbd5eb49418600e8d7df2cf451-mor50bd147e41738 .

_:genid-38640ccbd5eb49418600e8d7df2cf451-mor50bd147e41738 dc:creator "Ian Davis" .

frbr_core:adaptionOf skos:historyNote _:genid-38640ccbd5eb49418600e8d7df2cf451-mor50bd147e419d9 .

_:genid-38640ccbd5eb49418600e8d7df2cf451-mor50bd147e419d9 dc:creator "Ian Davis" .

frbr_core:transformation skos:historyNote _:genid-38640ccbd5eb49418600e8d7df2cf451-mor50bd147e41c76 .

_:genid-38640ccbd5eb49418600e8d7df2cf451-mor50bd147e41c76 dc:creator "Ian Davis" .

frbr_core:transformationOf skos:historyNote _:genid-38640ccbd5eb49418600e8d7df2cf451-mor50bd147e41f16 .

_:genid-38640ccbd5eb49418600e8d7df2cf451-mor50bd147e41f16 dc:creator "Ian Davis" .

frbr_core:imitation skos:historyNote _:genid-38640ccbd5eb49418600e8d7df2cf451-mor50bd147e421c2 .

_:genid-38640ccbd5eb49418600e8d7df2cf451-mor50bd147e421c2 dc:creator "Ian Davis" .

frbr_core:imitationOf skos:historyNote _:genid-38640ccbd5eb49418600e8d7df2cf451-mor50bd147e42464 .

_:genid-38640ccbd5eb49418600e8d7df2cf451-mor50bd147e42464 dc:creator "Ian Davis" .

frbr_core:abridgement skos:historyNote _:genid-38640ccbd5eb49418600e8d7df2cf451-mor50bd147e4257a .

_:genid-38640ccbd5eb49418600e8d7df2cf451-mor50bd147e4257a dc:creator "Ian Davis" .

frbr_core:abridgementOf skos:historyNote _:genid-38640ccbd5eb49418600e8d7df2cf451-mor50bd147e42681 .

_:genid-38640ccbd5eb49418600e8d7df2cf451-mor50bd147e42681 dc:creator "Ian Davis" .

frbr_core:revision skos:historyNote _:genid-38640ccbd5eb49418600e8d7df2cf451-mor50bd147e4278a .

_:genid-38640ccbd5eb49418600e8d7df2cf451-mor50bd147e4278a dc:creator "Ian Davis" .

frbr_core:revisionOf skos:historyNote _:genid-38640ccbd5eb49418600e8d7df2cf451-mor50bd147e4288e .

_:genid-38640ccbd5eb49418600e8d7df2cf451-mor50bd147e4288e dc:creator "Ian Davis" .

frbr_core:translation skos:historyNote _:genid-38640ccbd5eb49418600e8d7df2cf451-mor50bd147e42994 .

_:genid-38640ccbd5eb49418600e8d7df2cf451-mor50bd147e42994 dc:creator "Ian Davis" .

frbr_core:translationOf skos:historyNote _:genid-38640ccbd5eb49418600e8d7df2cf451-mor50bd147e42a9b .

_:genid-38640ccbd5eb49418600e8d7df2cf451-mor50bd147e42a9b dc:creator "Ian Davis" .

frbr_core:arrangement skos:historyNote _:genid-38640ccbd5eb49418600e8d7df2cf451-mor50bd147e42ba4 .

_:genid-38640ccbd5eb49418600e8d7df2cf451-mor50bd147e42ba4 dc:creator "Ian Davis" .

frbr_core:arrangementOf skos:historyNote _:genid-38640ccbd5eb49418600e8d7df2cf451-mor50bd147e42cac .

_:genid-38640ccbd5eb49418600e8d7df2cf451-mor50bd147e42cac dc:creator "Ian Davis" .

ElementsGr2:placeOfBirth skos:scopeNote "FRAD 4.1."@en .

ElementsGr2:placeOfDeath skos:scopeNote "FRAD 4.1."@en .

ElementsGr2:addressOfTheCorporateBody skos:scopeNote "FRAD 4.3."@en .

ElementsGr2:addressOfThePerson skos:scopeNote "FRAD 4.1."@en .

ElementsGr2:affiliation skos:scopeNote "FRAD 4.1."@en .

ElementsGr2:biographicalInformation skos:scopeNote "FRAD 4.1."@en .

ElementsGr2:corporateHistory skos:scopeNote "FRAD 4.3."@en .

ElementsGr2:countryAssociatedWithThePerson skos:scopeNote "FRAD 4.1."@en .

ElementsGr2:dateAssociatedWithTheCorporateBody skos:scopeNote "FRBR 4.7.4 and FRAD 4.3."@en .

ElementsGr2:dateOfEstablishment skos:scopeNote "FRBR 4.7.4 and FRAD 4.3."@en .

ElementsGr2:dateOfConferenceEtc skos:scopeNote "FRBR 4.7.4 and FRAD 4.3."@en .

ElementsGr2:dateOfTermination skos:scopeNote "FRBR 4.7.4 and FRAD 4.3."@en .

ElementsGr2:dateAssociatedWithTheFamily skos:scopeNote "FRAD 4.2."@en .

ElementsGr2:dateAssociatedWithThePerson skos:scopeNote "FRBR 4.6.2 and FRAD 4.1."@en .

ElementsGr2:dateOfDeath skos:scopeNote "FRBR 4.6.2 and FRAD 4.1."@en .

ElementsGr2:periodOfActivityOfThePerson skos:scopeNote "FRBR 4.6.2 and FRAD 4.1."@en .

ElementsGr2:familyHistory skos:scopeNote "FRAD 4.2."@en .

ElementsGr2:fieldOfActivityOfTheCorporateBody skos:scopeNote "FRAD 4.3."@en .

ElementsGr2:fieldOfActivityOfThePerson skos:scopeNote "FRBR 4.6.4 and FRAD 4.1."@en .

ElementsGr2:fullerFormOfName skos:scopeNote "FRBR 4.6.1 and FRAD 4.1."@en .

ElementsGr2:gender skos:scopeNote "FRAD 4.1."@en .

ElementsGr2:hereditaryTitle skos:scopeNote "FRAD 4.2."@en .

ElementsGr2:identifierForTheCorporateBody skos:scopeNote "FRAD 5.2."@en .

ElementsGr2:identifierForTheFamily skos:scopeNote "FRAD 5.2."@en .

ElementsGr2:languageOfTheCorporateBody skos:scopeNote "FRAD 4.3."@en .

ElementsGr2:languageOfThePerson skos:scopeNote "FRAD 4.1."@en .

ElementsGr2:placeAssociatedWithTheCorporateBody skos:scopeNote "FRBR 4.7.3 and FRAD 4.3."@en .

ElementsGr2:locationOfHeadquarters skos:scopeNote "FRBR 4.7.3 and FRAD 4.3."@en .

ElementsGr2:nameOfTheCorporateBody skos:scopeNote "FRBR 4.7.1 and FRAD 5.2."@en .

ElementsGr2:preferredNameForTheCorporateBody skos:scopeNote "FRBR 4.6.1 and FRAD 5.2."@en .

ElementsGr2:nameOfTheFamily skos:scopeNote "FRAD 5.2."@en .

ElementsGr2:preferredNameForTheFamily skos:scopeNote "FRAD 5.2."@en .

ElementsGr2:nameOfThePerson skos:scopeNote "FRBR 4.6.1 and FRAD 5.2."@en .

ElementsGr2:preferredNameForThePerson skos:scopeNote "FRBR 4.6.1 and FRAD 5.2."@en .

ElementsGr2:otherDesignationAssociatedWithTheCorporateBody skos:scopeNote "FRBR 4.7.2, 4.7.5 and FRAD 4.3."@en .

ElementsGr2:otherDesignationAssociatedWithThePerson skos:scopeNote "FRBR 4.6.4 and FRAD 4.1."@en .

ElementsGr2:placeAssociatedWithTheFamily skos:scopeNote "FRAD 4.2."@en .

ElementsGr2:placeOfResidence skos:scopeNote "FRAD 4.1."@en .

ElementsGr2:professionOrOccupation skos:scopeNote "FRAD 4.1."@en .

ElementsGr2:prominentMemberOfTheFamily skos:scopeNote "FRAD 4.2."@en .

ElementsGr2:titleOfThePerson skos:scopeNote "FRBR 4.6.3 and FRAD 4.1."@en .

skos:Concept owl:disjointWith skos:ConceptScheme .

foaf:Person owl:disjointWith foaf:Organization, foaf:Project .

skos:Collection owl:disjointWith skos:Concept, skos:ConceptScheme .

frbr_core:Expression owl:disjointWith frbr_core:Item, frbr_core:Manifestation, frbr_core:Work .

frbr_core:Manifestation owl:disjointWith frbr_core:Expression, frbr_core:Item, frbr_core:Work .

frbr_core:Place owl:disjointWith frbr_core:Concept, frbr_core:Event, frbr_core:Object .

frbr_core:Work owl:disjointWith frbr_core:Expression, frbr_core:Item, frbr_core:Manifestation .

foaf:Document owl:disjointWith foaf:Organization, foaf:Project .

frbr_core:Endeavour owl:disjointWith frbr_core:ResponsibleEntity, frbr_core:Subject .

frbr_core:ResponsibleEntity owl:disjointWith frbr_core:Endeavour, frbr_core:Subject .

frbr_core:Subject owl:disjointWith frbr_core:Endeavour, frbr_core:ResponsibleEntity .

frbr_core:Item owl:disjointWith frbr_core:Expression, frbr_core:Manifestation, frbr_core:Work .

frbr_core:Person owl:disjointWith frbr_core:Endeavour, frbr_core:Subject .

foaf:Organization owl:disjointWith foaf:Document, foaf:Person .

frbr_core:Object owl:disjointWith frbr_core:Concept, frbr_core:Event, frbr_core:Place .

frbr_core:Concept owl:disjointWith frbr_core:Event, frbr_core:Object, frbr_core:Place .

foaf:Project owl:disjointWith foaf:Document, foaf:Person .

<http://americanart.si.edu/ontology/> dct:description "The Smithsonian American Art Museum is a museum in Washington, D.C. with an extensive collection of American art."@en;
  dct:modified "2013-04-16";
  dct:title "Smithsonian American Art Museum(SAAM)"@en;
  owl:versionInfo "5.0" .

<http://purl.org/NET/dc_owl2dl/terms> dct:modified "2009-09-07" .

<http://www.europeana.eu/schemas/edm/> owl:versionInfo "5.2.3" .

<http://www.openarchives.org/ore/terms/> dct:title "The OAI ORE terms vocabulary" .

<http://purl.org/vocab/frbr/core> dc:identifier "http://purl.org/vocab/frbr/frbr-core-20051014" .

dct:creator <http://www.w3.org/2004/02/skos/core#definition> "An entity primarily responsible for making the resource."@en-us .

edm:Agent <http://www.w3.org/2004/02/skos/core#definition> """This class comprises people, either individually or in groups, who have the
potential to perform intentional actions for which they can be held responsible.""" .

edm:ProvidedCHO <http://www.w3.org/2004/02/skos/core#definition> "This class comprises the Cultural Heritage objects that Europeana collects descriptions about."@en .

edm:Place <http://www.w3.org/2004/02/skos/core#definition> "An \"extent in space, in particular on the surface of the earth, in the pure sense of physics: independent from temporal phenomena and matter\" (CIDOC CRM)"@en .

dct:issued <http://www.w3.org/2004/02/skos/core#definition> "Date of formal issuance (e.g., publication) of the resource."@en-us .

dct:modified <http://www.w3.org/2004/02/skos/core#definition> "Date on which the resource was changed."@en-us .

dct:title <http://www.w3.org/2004/02/skos/core#definition> "A name given to the resource."@en-us .

dct:description <http://www.w3.org/2004/02/skos/core#definition> "An account of the resource."@en-us .

edm:year <http://www.w3.org/2004/02/skos/core#definition> """A point of time associated with an event in the life of the original analog or
born digital object."""@en .

dct:temporal <http://www.w3.org/2004/02/skos/core#definition> "Temporal characteristics of the resource."@en-us .

edm:dataProvider <http://www.w3.org/2004/02/skos/core#definition> "This element is specifically included to allow the name of the organisation who supplies data to Europeana indirectly via an aggregator to be recorded and displayed in the portal. Aggregator names are recorded in edm:provider. If an organisation provides data directly to Europeana (i.e. not via an aggregator) the values in edm:dataProvider and edm:provider will be the same. Organisation names should be provided as an ordinary text string until the Europeana Authority File for Organisations has been established. At that point providers will be able to send an identifier from the file instead of a text string. The name provided should be the preferred form of the name in the language the provider chooses as the default language for display in the portal. Countries with multiple languages may prefer to concatenate the name in more than one language (See the example below.) Note: Europeana Data Provider is not necessarily the institution where the physical object is located."@en .

dct:provenance <http://www.w3.org/2004/02/skos/core#definition> "A statement of any changes in ownership and custody of the resource since its creation that are significant for its authenticity, integrity, and interpretation."@en-us .

edm:userTag <http://www.w3.org/2004/02/skos/core#definition> "This is a tag created by a user through the Europeana interface."@en .

edm:hasMet <http://www.w3.org/2004/02/skos/core#definition> "edm:hasMet relates a resource with the objects or phenomena that have happened to or have happened together with the resource under consideration. We can abstractly think of history and the present as a series of meetings between people and other things in space-time. Therefore we name this relationship as the things the object has met in the course of its existence. These meetings are events in the proper sense, in which other people and things participate in any role."@en .

edm:hasType <http://www.w3.org/2004/02/skos/core#definition> """This property relates a resource with the concepts it belongs to in a suitable
type system such as MIME or any thesaurus that captures categories of objects in a given field (e.g., the Objects facet in Gettys Art and Architecture Thesaurus). It does not capture aboutness."""@en .

edm:isRelatedTo <http://www.w3.org/2004/02/skos/core#definition> """edm:isRelatedTo is the most general contextual property in EDM. Contextual
properties have typically to do either with the things that have happened to or together with the object under consideration, or what the object refers to by its shape, form or features in a figural or encoded form. For sake of simplicity, we include in the contextual relationships also the scholarly classification, which may have either to do with the role and cultural connections of the object in the past, or its kind of structure, substance or contents as it can be verified at present."""@en .

edm:isDerivativeOf <http://www.w3.org/2004/02/skos/core#definition> "This property captures a narrower notion of derivation than edm:isSimilarTo, in the sense that it relates a resource to another one, obtained by reworking, reducing, expanding, parts or the whole contents of the former, and possibly adding some minor parts. Versions have an even narrower meaning, in that it requires common identity between the related resources. Translations, summaries, abstractions etc. do not qualify as versions, but do qualify as derivatives."@en .

dct:hasFormat <http://www.w3.org/2004/02/skos/core#definition> "A related resource that is substantially the same as the pre-existing described resource, but in another format."@en-us .

dct:hasVersion <http://www.w3.org/2004/02/skos/core#definition> "A related resource that is a version, edition, or adaptation of the described resource."@en-us .

dct:isFormatOf <http://www.w3.org/2004/02/skos/core#definition> "A related resource that is substantially the same as the described resource, but in another format."@en-us .

dct:isReplacedBy <http://www.w3.org/2004/02/skos/core#definition> "A related resource that supplants, displaces, or supersedes the described resource."@en-us .

dct:isVersionOf <http://www.w3.org/2004/02/skos/core#definition> "A related resource of which the described resource is a version, edition, or adaptation."@en-us .

dct:replaces <http://www.w3.org/2004/02/skos/core#definition> "A related resource that is supplanted, displaced, or superseded by the described resource."@en-us .

dct:spatial <http://www.w3.org/2004/02/skos/core#definition> "Spatial characteristics of the resource."@en-us .

dct:tableOfContents <http://www.w3.org/2004/02/skos/core#definition> "A list of subunits of the resource."@en-us .

edm:hasView <http://www.w3.org/2004/02/skos/core#definition> """This property relates a ORE aggregation about a CHO with a web resource
providing a view of that CHO. Examples of view are: a thumbnail, a textual
abstract and a table of contents. The ORE aggregation may be a Europeana
Aggregation, in which case the view is an object owned by Europeana (i.e., an instance of edm:EuropeanaObject) or an aggregation contributed by a content provider. In order to capture both these cases, the domain of edm:hasView is ore:Aggregation and its range is edm:WebResource"""@en .

edm:aggregatedCHO <http://www.w3.org/2004/02/skos/core#definition> """This property associates an ORE aggregation with the Cultural Heritage
Object(s) (CHO for short) it is about."""@en .

edm:currentLocation <http://www.w3.org/2004/02/skos/core#definition> "The geographic location and/or name of the repository, building, site, or other entity whose boundaries presently include the resource."@en .

edm:happenedAt <http://www.w3.org/2004/02/skos/core#definition> """This property associates an event with the place at which the event
happened."""@en .

edm:Event <http://www.w3.org/2004/02/skos/core#definition> """An event is a change \"of states in cultural, social or physical systems,
 regardless of scale, brought about by a series or group of coherent physical,
cultural, technological or legal phenomena\" (E5 Event in CIDOC CRM) or a \"set of coherent phenomena or cultural manifestations bounded in time and  space\" (E4 Period in CIDOC CRM)
"""@en .

edm:NonInformationResource <http://www.w3.org/2004/02/skos/core#definition> "All resources that are not information resources."@en .

edm:WebResource <http://www.w3.org/2004/02/skos/core#definition> """Information Resources that have at least one Web Representation and at least
a URI."""@en .

edm:incorporates <http://www.w3.org/2004/02/skos/core#definition> """This property captures the use of some resource to add value to another
resource. Such resources may be nested, such as performing a theater play text, and then recording the performance, or creating an artful edition of a collection of poems or just aggregating various poems in an anthology. There may be no single part that contains ultimately the incorporated object, which may be dispersed in the presentation. Therefore, incorporated resources do in general not form proper parts. Incorporated resources are not part of the same resource, but are taken from other resources, and have an independent history. Therefore edm:incorporates is not a sub-property of dcterm:hasPart."""@en .

edm:isSimilarTo <http://www.w3.org/2004/02/skos/core#definition> "The most generic derivation property, covering also the case of questionable derivation. Is Similar To asserts that parts of the contents of one resource exhibit common features with respect to ideas, shapes, structures, colors, words, plots, topics with the contents of the related resource. Those common features may be attributed to a common origin or influence (in particular for derivation), but also to more generic cultural or psychological factors."@en .

edm:isAnnotationOf <http://www.w3.org/2004/02/skos/core#definition> """This property relates an annotation (a Europeana object) with the resource
that it annotates."""@en .

edm:EuropeanaObject <http://www.w3.org/2004/02/skos/core#definition> "Any object that is the result of Europeanas activities"@en .

edm:isNextInSequence <http://www.w3.org/2004/02/skos/core#definition> "edm:isNextInSequence relates two resources S and R that are ordered parts of the same resource A, and such that R comes immediately after R in the order created by their being parts of S."@en .

edm:isRepresentationOf <http://www.w3.org/2004/02/skos/core#definition> "This property associates an information resource to the resource (if any) that it represents"@en .

edm:InformationResource <http://www.w3.org/2004/02/skos/core#definition> "An information resource is a resource whose essential characteristics can be conveyed in a single message. It can be associated with a URI, it can have a representation, for example: a text is an InformationResource."@en .

edm:isShownAt <http://www.w3.org/2004/02/skos/core#definition> "An unambiguous URL reference to the digital object on the providers web site in its full information context."@en .

edm:landingPage <http://www.w3.org/2004/02/skos/core#definition> """This property captures the relation between an aggregation representing a
Cultural Heritage Object and the Web Resource representing that Object on
the providers web site."""@en .

edm:isShownBy <http://www.w3.org/2004/02/skos/core#definition> "An unambiguous URL reference to the digital object on the providers web site in the best available resolution/quality."@en .

edm:isSuccessorOf <http://www.w3.org/2004/02/skos/core#definition> "This property captures the relation between the continuation of a resource and that resource. This applies to a story, a serial, a journal etc. No content of the successor resource is identical or has a similar form with that of the precursor. The similarity is only in the context, subjects and figures of a plot. Successors typically form part of a common whole  such as a trilogy, a journal, etc."@en .

edm:object <http://www.w3.org/2004/02/skos/core#definition> """The URL of a thumbnail representing the digital object or, if there is no such
thumbnail, the URL of the digital object in the best resolution available on the
web site of the data provider from which a thumbnail could be generated. This will often be the same URL as given in edm:isShownBy."""@en .

edm:occurredAt <http://www.w3.org/2004/02/skos/core#definition> """This property associates an event to the smallest known time span that
overlaps with the occurrence of that event"""@en .

edm:TimeSpan <http://www.w3.org/2004/02/skos/core#definition> """The class of \"abstract temporal extents, in the sense of Galilean physics,
 having a beginning, an end and a duration\" (CIDOC CRM)"""@en .

edm:provider <http://www.w3.org/2004/02/skos/core#definition> "Name of the organization that delivers data to Europeana"@en .

edm:realizes <http://www.w3.org/2004/02/skos/core#definition> "This property describes a relation between a physical thing and the information resource that is contained in it, visible at it or otherwise carried by it, if applicable."@en .

edm:PhysicalThing <http://www.w3.org/2004/02/skos/core#definition> """A persistent physical item such as a painting, a building, a book or a stone.
Persons are not items. This class represents Cultural Heritage Objects known to Europeana to be physical things (such as Mona Lisa) as well as all physical things Europeana refers to in the descriptions of Cultural Heritage Objects (such as the Rosetta Stone)."""@en .

edm:rights <http://www.w3.org/2004/02/skos/core#definition> """Information about copyright of the digital object as specified by isShownBy
and isShownAt"""@en .

edm:uri <http://www.w3.org/2004/02/skos/core#definition> "This is a tag created by a user through the Europeana interface."@en .

edm:wasPresentAt <http://www.w3.org/2004/02/skos/core#definition> "This property associates the people, things or information resources with an event at which they were present"@en .

edm:type <http://www.w3.org/2004/02/skos/core#definition> "The Europeana material type of the resource"@en .

edm:ugc <http://www.w3.org/2004/02/skos/core#definition> "This element is used to identify user generated content (also called user created content).  It should be applied to all digitised or born digital content contributed by the general public and collected by Europeana through a crowdsourcing initiative or project."@en .

dct:PeriodOfTime <http://www.w3.org/2004/02/skos/core#definition> "An interval of time that is named or defined by its start and end dates."@en-us .

edm:EuropeanaAggregation <http://www.w3.org/2004/02/skos/core#definition> """The set of resources related to a single Cultural Heritage Object that
collectively represent that object in Europeana. Such set consists of: all
descriptions about the object that Europeana collects from (possibly different) content providers, including thumbnails and other forms of abstractions, as well as of the description of the object Europeana builds.""" .

edm:unstored <http://www.w3.org/2004/02/skos/core#definition> """This is a container element which includes all relevant information that
otherwise cannot be mapped to another element in the ESE."""@en .

edm:language <http://www.w3.org/2004/02/skos/core#definition> "A language assigned to the resource with reference to the Provider."@en .

dct:publisher <http://www.w3.org/2004/02/skos/core#definition> "An entity responsible for making the resource available."@en-us .

dct:hasPart <http://www.w3.org/2004/02/skos/core#definition> "A related resource that is included either physically or logically in the described resource."@en-us .

dct:isPartOf <http://www.w3.org/2004/02/skos/core#definition> "A related resource in which the described resource is physically or logically included."@en-us .

dct:IMT <http://www.w3.org/2004/02/skos/core#definition> "The set of media types specified by the Internet Assigned Numbers Authority."@en-us .

dct:Agent <http://www.w3.org/2004/02/skos/core#definition> "A resource that acts or has the power to act."@en-us .

dct:license <http://www.w3.org/2004/02/skos/core#definition> "A legal document giving official permission to do something with the resource."@en-us .

dct:abstract <http://www.w3.org/2004/02/skos/core#definition> "A summary of the resource."@en-us .

dct:accessRights <http://www.w3.org/2004/02/skos/core#definition> "Information about who can access the resource or an indication of its security status."@en-us .

dct:RightsStatement <http://www.w3.org/2004/02/skos/core#definition> "A statement about the intellectual property rights (IPR) held in or over a Resource, a legal document giving official permission to do something with a resource, or a statement about access rights."@en-us .

dct:rights <http://www.w3.org/2004/02/skos/core#definition> "Information about rights held in and over the resource."@en-us .

dct:accrualMethod <http://www.w3.org/2004/02/skos/core#definition> "The method by which items are added to a collection."@en-us .

dct:MethodOfAccrual <http://www.w3.org/2004/02/skos/core#definition> "A method by which resources are added to a collection."@en-us .

dct:accrualPeriodicity <http://www.w3.org/2004/02/skos/core#definition> "The frequency with which items are added to a collection."@en-us .

dct:Frequency <http://www.w3.org/2004/02/skos/core#definition> "A rate at which something recurs."@en-us .

dct:accrualPolicy <http://www.w3.org/2004/02/skos/core#definition> "The policy governing the addition of items to a collection."@en-us .

dct:Policy <http://www.w3.org/2004/02/skos/core#definition> "A plan or course of action by an authority, intended to influence and determine decisions, actions, and other matters."@en-us .

dct:alternative <http://www.w3.org/2004/02/skos/core#definition> "An alternative name for the resource."@en-us .

dct:audience <http://www.w3.org/2004/02/skos/core#definition> "A class of entity for whom the resource is intended or useful."@en-us .

dct:AgentClass <http://www.w3.org/2004/02/skos/core#definition> "A group of agents."@en-us .

dct:available <http://www.w3.org/2004/02/skos/core#definition> "Date (often a range) that the resource became or will become available."@en-us .

dct:date <http://www.w3.org/2004/02/skos/core#definition> "A point or period of time associated with an event in the lifecycle of the resource."@en-us .

dct:bibliographicCitation <http://www.w3.org/2004/02/skos/core#definition> "A bibliographic reference for the resource."@en-us .

dct:BibliographicResource <http://www.w3.org/2004/02/skos/core#definition> "A book, article, or other documentary resource."@en-us .

dct:identifier <http://www.w3.org/2004/02/skos/core#definition> "An unambiguous reference to the resource within a given context."@en-us .

dct:conformsTo <http://www.w3.org/2004/02/skos/core#definition> "An established standard to which the described resource conforms."@en-us .

dct:Standard <http://www.w3.org/2004/02/skos/core#definition> "A basis for comparison; a reference point against which other things can be evaluated."@en-us .

dct:relation <http://www.w3.org/2004/02/skos/core#definition> "A related resource."@en-us .

dct:contributor <http://www.w3.org/2004/02/skos/core#definition> "An entity responsible for making contributions to the resource."@en-us .

dct:coverage <http://www.w3.org/2004/02/skos/core#definition> "The spatial or temporal topic of the resource, the spatial applicability of the resource, or the jurisdiction under which the resource is relevant."@en-us .

dct:LocationPeriodOrJurisdiction <http://www.w3.org/2004/02/skos/core#definition>
    "A location, period of time, or jurisdiction."@en-us .

dct:created <http://www.w3.org/2004/02/skos/core#definition> "Date of creation of the resource."@en-us .

dct:dateAccepted <http://www.w3.org/2004/02/skos/core#definition> "Date of acceptance of the resource."@en-us .

dct:dateCopyrighted <http://www.w3.org/2004/02/skos/core#definition> "Date of copyright."@en-us .

dct:dateSubmitted <http://www.w3.org/2004/02/skos/core#definition> "Date of submission of the resource."@en-us .

dct:educationLevel <http://www.w3.org/2004/02/skos/core#definition> "A class of entity, defined in terms of progression through an educational or training context, for which the described resource is intended."@en-us .

dct:extent <http://www.w3.org/2004/02/skos/core#definition> "The size or duration of the resource."@en-us .

dct:SizeOrDuration <http://www.w3.org/2004/02/skos/core#definition> "A dimension or extent, or a time taken to play or execute."@en-us .

dct:format <http://www.w3.org/2004/02/skos/core#definition> "The file format, physical medium, or dimensions of the resource."@en-us .

dct:MediaTypeOrExtent <http://www.w3.org/2004/02/skos/core#definition> "A media type or extent."@en-us .

dct:instructionalMethod <http://www.w3.org/2004/02/skos/core#definition> "A process, used to engender knowledge, attitudes and skills, that the described resource is designed to support."@en-us .

dct:MethodOfInstruction <http://www.w3.org/2004/02/skos/core#definition> "A process that is used to engender knowledge, attitudes, and skills."@en-us .

dct:isReferencedBy <http://www.w3.org/2004/02/skos/core#definition> "A related resource that references, cites, or otherwise points to the described resource."@en-us .

dct:isRequiredBy <http://www.w3.org/2004/02/skos/core#definition> "A related resource that requires the described resource to support its function, delivery, or coherence."@en-us .

dct:language <http://www.w3.org/2004/02/skos/core#definition> "A language of the resource."@en-us .

dct:LinguisticSystem <http://www.w3.org/2004/02/skos/core#definition> "A system of signs, symbols, sounds, gestures, or rules used in communication."@en-us .

dct:LicenseDocument <http://www.w3.org/2004/02/skos/core#definition> "A legal document giving official permission to do something with a Resource."@en-us .

dct:mediator <http://www.w3.org/2004/02/skos/core#definition> "An entity that mediates access to the resource and for whom the resource is intended or useful."@en-us .

dct:medium <http://www.w3.org/2004/02/skos/core#definition> "The material or physical carrier of the resource."@en-us .

dct:PhysicalResource <http://www.w3.org/2004/02/skos/core#definition> "A material thing."@en-us .

dct:PhysicalMedium <http://www.w3.org/2004/02/skos/core#definition> "A physical material or carrier."@en-us .

dct:ProvenanceStatement <http://www.w3.org/2004/02/skos/core#definition> "A statement of any changes in ownership and custody of a resource since its creation that are significant for its authenticity, integrity, and interpretation."@en-us .

dct:references <http://www.w3.org/2004/02/skos/core#definition> "A related resource that is referenced, cited, or otherwise pointed to by the described resource."@en-us .

dct:requires <http://www.w3.org/2004/02/skos/core#definition> "A related resource that is required by the described resource to support its function, delivery, or coherence."@en-us .

dct:rightsHolder <http://www.w3.org/2004/02/skos/core#definition> "A person or organization owning or managing rights over the resource."@en-us .

dct:source <http://www.w3.org/2004/02/skos/core#definition> "A related resource from which the described resource is derived."@en-us .

dct:Location <http://www.w3.org/2004/02/skos/core#definition> "A spatial region or named place."@en-us .

dct:subject <http://www.w3.org/2004/02/skos/core#definition> "The topic of the resource."@en-us .

dct:type <http://www.w3.org/2004/02/skos/core#definition> "The nature or genre of the resource."@en-us .

dct:valid <http://www.w3.org/2004/02/skos/core#definition> "Date (often a range) of validity of a resource."@en-us .

dct:DCMIType <http://www.w3.org/2004/02/skos/core#definition> "The set of classes specified by the DCMI Type Vocabulary, used to categorize the nature or genre of the resource."@en-us .

dct:DDC <http://www.w3.org/2004/02/skos/core#definition> "The set of conceptual resources specified by the Dewey Decimal Classification."@en-us .

dct:LCC <http://www.w3.org/2004/02/skos/core#definition> "The set of conceptual resources specified by the Library of Congress Classification."@en-us .

dct:LCSH <http://www.w3.org/2004/02/skos/core#definition> "The set of labeled concepts specified by the Library of Congress Subject Headings."@en-us .

dct:MESH <http://www.w3.org/2004/02/skos/core#definition> "The set of labeled concepts specified by the Medical Subject Headings."@en-us .

dct:NLM <http://www.w3.org/2004/02/skos/core#definition> "The set of conceptual resources specified by the National Library of Medicine Classification."@en-us .

dct:TGN <http://www.w3.org/2004/02/skos/core#definition> "The set of places specified by the Getty Thesaurus of Geographic Names."@en-us .

dct:UDC <http://www.w3.org/2004/02/skos/core#definition> "The set of conceptual resources specified by the Universal Decimal Classification."@en-us .

dct:Box <http://www.w3.org/2004/02/skos/core#definition> "The set of regions in space defined by their geographic coordinates according to the DCMI Box Encoding Scheme."@en-us .

dct:ISO3166 <http://www.w3.org/2004/02/skos/core#definition> "The set of codes listed in ISO 3166-1 for the representation of names of countries."@en-us .

dct:ISO639-2 <http://www.w3.org/2004/02/skos/core#definition> "The three-letter alphabetic codes listed in ISO639-2 for the representation of names of languages."@en-us .

dct:ISO639-3 <http://www.w3.org/2004/02/skos/core#definition> "The set of three-letter codes listed in ISO 639-3 for the representation of names of languages."@en-us .

dct:Period <http://www.w3.org/2004/02/skos/core#definition> "The set of time intervals defined by their limits according to the DCMI Period Encoding Scheme."@en-us .

dct:Point <http://www.w3.org/2004/02/skos/core#definition> "The set of points in space defined by their geographic coordinates according to the DCMI Point Encoding Scheme."@en-us .

dct:RFC1766 <http://www.w3.org/2004/02/skos/core#definition> "The set of tags, constructed according to RFC 1766, for the identification of languages."@en-us .

dct:RFC3066 <http://www.w3.org/2004/02/skos/core#definition> "The set of tags constructed according to RFC 3066 for the identification of languages."@en-us .

dct:RFC4646 <http://www.w3.org/2004/02/skos/core#definition> "The set of tags constructed according to RFC 4646 for the identification of languages."@en-us .

dct:URI <http://www.w3.org/2004/02/skos/core#definition> "The set of identifiers constructed according to the generic syntax for Uniform Resource Identifiers as specified by the Internet Engineering Task Force."@en-us .

dct:W3CDTF <http://www.w3.org/2004/02/skos/core#definition> "The set of dates and times constructed according to the W3C Date and Time Formats Specification."@en-us .

dct:FileFormat <http://www.w3.org/2004/02/skos/core#definition> "A digital resource format."@en-us .

dct:MediaType <http://www.w3.org/2004/02/skos/core#definition> "A file format or physical medium."@en-us .

dct:Jurisdiction <http://www.w3.org/2004/02/skos/core#definition> "The extent or range of judicial, law enforcement, or other authority."@en-us .

<http://purl.org/vocab/frbr/core> dc:date "2009-05-16" .

_:genid-38640ccbd5eb49418600e8d7df2cf451-mor50bd147e3df74 dc:date "2005-10-14" .

_:genid-38640ccbd5eb49418600e8d7df2cf451-mor50bd147e3dfc0 dc:date "2009-05-16" .

_:genid-38640ccbd5eb49418600e8d7df2cf451-mor50bd147e3e223 dc:date "2005-08-08" .

_:genid-38640ccbd5eb49418600e8d7df2cf451-mor50bd147e3e26f dc:date "2005-08-08" .

_:genid-38640ccbd5eb49418600e8d7df2cf451-mor50bd147e3e2bf dc:date "2005-08-09" .

_:genid-38640ccbd5eb49418600e8d7df2cf451-mor50bd147e3e496 dc:date "2005-08-08" .

_:genid-38640ccbd5eb49418600e8d7df2cf451-mor50bd147e3e4e2 dc:date "2005-08-08" .

_:genid-38640ccbd5eb49418600e8d7df2cf451-mor50bd147e3e52e dc:date "2005-08-09" .

_:genid-38640ccbd5eb49418600e8d7df2cf451-mor50bd147e3e6b4 dc:date "2005-08-08" .

_:genid-38640ccbd5eb49418600e8d7df2cf451-mor50bd147e3e74b dc:date "2005-08-08" .

_:genid-38640ccbd5eb49418600e8d7df2cf451-mor50bd147e3e798 dc:date "2005-08-09" .

_:genid-38640ccbd5eb49418600e8d7df2cf451-mor50bd147e3e700 dc:date "2005-08-08" .

_:genid-38640ccbd5eb49418600e8d7df2cf451-mor50bd147e3e7e4 dc:date "2005-08-10" .

_:genid-38640ccbd5eb49418600e8d7df2cf451-mor50bd147e3e5a5 dc:date "2005-08-08" .

_:genid-38640ccbd5eb49418600e8d7df2cf451-mor50bd147e3e5f3 dc:date "2005-08-08" .

_:genid-38640ccbd5eb49418600e8d7df2cf451-mor50bd147e3e641 dc:date "2005-08-09" .

_:genid-38640ccbd5eb49418600e8d7df2cf451-mor50bd147e3e336 dc:date "2005-08-08" .

_:genid-38640ccbd5eb49418600e8d7df2cf451-mor50bd147e3e383 dc:date "2005-08-08" .

_:genid-38640ccbd5eb49418600e8d7df2cf451-mor50bd147e3e424 dc:date "2005-08-09" .

_:genid-38640ccbd5eb49418600e8d7df2cf451-mor50bd147e3e3d8 dc:date "2005-08-08" .

_:genid-38640ccbd5eb49418600e8d7df2cf451-mor50bd147e3e925 dc:date "2005-08-08" .

_:genid-38640ccbd5eb49418600e8d7df2cf451-mor50bd147e3e971 dc:date "2005-08-08" .

_:genid-38640ccbd5eb49418600e8d7df2cf451-mor50bd147e3e9bd dc:date "2005-08-09" .

_:genid-38640ccbd5eb49418600e8d7df2cf451-mor50bd147e3ec08 dc:date "2005-08-08" .

_:genid-38640ccbd5eb49418600e8d7df2cf451-mor50bd147e3ec53 dc:date "2005-08-08" .

_:genid-38640ccbd5eb49418600e8d7df2cf451-mor50bd147e3ec9f dc:date "2005-08-09" .

_:genid-38640ccbd5eb49418600e8d7df2cf451-mor50bd147e3ea2b dc:date "2005-08-08" .

_:genid-38640ccbd5eb49418600e8d7df2cf451-mor50bd147e3ea78 dc:date "2005-08-08" .

_:genid-38640ccbd5eb49418600e8d7df2cf451-mor50bd147e3eac9 dc:date "2005-08-09" .

_:genid-38640ccbd5eb49418600e8d7df2cf451-mor50bd147e3ee70 dc:date "2005-08-08" .

_:genid-38640ccbd5eb49418600e8d7df2cf451-mor50bd147e3eebb dc:date "2005-08-08" .

_:genid-38640ccbd5eb49418600e8d7df2cf451-mor50bd147e3ef08 dc:date "2005-08-09" .

_:genid-38640ccbd5eb49418600e8d7df2cf451-mor50bd147e3f23c dc:date "2005-08-08" .

_:genid-38640ccbd5eb49418600e8d7df2cf451-mor50bd147e3f2de dc:date "2005-08-09" .

_:genid-38640ccbd5eb49418600e8d7df2cf451-mor50bd147e3f292 dc:date "2005-08-08" .

_:genid-38640ccbd5eb49418600e8d7df2cf451-mor50bd147e3f0e2 dc:date "2005-08-08" .

_:genid-38640ccbd5eb49418600e8d7df2cf451-mor50bd147e3f12e dc:date "2005-08-08" .

_:genid-38640ccbd5eb49418600e8d7df2cf451-mor50bd147e3f1c4 dc:date "2005-08-09" .

_:genid-38640ccbd5eb49418600e8d7df2cf451-mor50bd147e3f17a dc:date "2005-08-08" .

_:genid-38640ccbd5eb49418600e8d7df2cf451-mor50bd147e3f354 dc:date "2005-08-08" .

_:genid-38640ccbd5eb49418600e8d7df2cf451-mor50bd147e3f3a9 dc:date "2005-08-08" .

_:genid-38640ccbd5eb49418600e8d7df2cf451-mor50bd147e3f43f dc:date "2005-08-09" .

_:genid-38640ccbd5eb49418600e8d7df2cf451-mor50bd147e3f3f4 dc:date "2005-08-08" .

_:genid-38640ccbd5eb49418600e8d7df2cf451-mor50bd147e3ef7f dc:date "2005-08-08" .

_:genid-38640ccbd5eb49418600e8d7df2cf451-mor50bd147e3efcc dc:date "2005-08-08" .

_:genid-38640ccbd5eb49418600e8d7df2cf451-mor50bd147e3f065 dc:date "2005-08-09" .

_:genid-38640ccbd5eb49418600e8d7df2cf451-mor50bd147e3f019 dc:date "2005-08-08" .

_:genid-38640ccbd5eb49418600e8d7df2cf451-mor50bd147e3f566 dc:date "2005-08-08" .

_:genid-38640ccbd5eb49418600e8d7df2cf451-mor50bd147e3f5b4 dc:date "2005-08-09" .

_:genid-38640ccbd5eb49418600e8d7df2cf451-mor50bd147e3f622 dc:date "2005-08-08" .

_:genid-38640ccbd5eb49418600e8d7df2cf451-mor50bd147e3f66c dc:date "2005-08-09" .

_:genid-38640ccbd5eb49418600e8d7df2cf451-mor50bd147e3f6da dc:date "2005-08-08" .

_:genid-38640ccbd5eb49418600e8d7df2cf451-mor50bd147e3f729 dc:date "2005-08-09" .

_:genid-38640ccbd5eb49418600e8d7df2cf451-mor50bd147e3f797 dc:date "2005-08-08" .

_:genid-38640ccbd5eb49418600e8d7df2cf451-mor50bd147e3f7e2 dc:date "2005-08-09" .

_:genid-38640ccbd5eb49418600e8d7df2cf451-mor50bd147e3f852 dc:date "2005-08-08" .

_:genid-38640ccbd5eb49418600e8d7df2cf451-mor50bd147e3f89d dc:date "2005-08-09" .

_:genid-38640ccbd5eb49418600e8d7df2cf451-mor50bd147e3f90e dc:date "2005-08-08" .

_:genid-38640ccbd5eb49418600e8d7df2cf451-mor50bd147e3f95a dc:date "2005-08-09" .

<http://vocab.org/frbr/core.html> dc:format "text/html" .

<http://vocab.org/frbr/core.json> dc:format "application/json" .

<http://vocab.org/frbr/core.turtle> dc:format "text/plain" .

<http://vocab.org/frbr/core.rdf> dct:hasFormat <http://vocab.org/frbr/core.html>,
    <http://vocab.org/frbr/core.json>, <http://vocab.org/frbr/core.turtle> .

<http://purl.org/vocab/frbr/core> dct:isVersionOf <http://purl.org/vocab/frbr/core#>;
  dct:replaces <http://purl.org/vocab/frbr/frbr-core-20050809> .

_:genid-38640ccbd5eb49418600e8d7df2cf451-mor50bd147e3f9c6 dc:date "2005-08-08" .

_:genid-38640ccbd5eb49418600e8d7df2cf451-mor50bd147e3fa11 dc:date "2005-08-09" .

_:genid-38640ccbd5eb49418600e8d7df2cf451-mor50bd147e3fc25 dc:date "2005-08-08" .

_:genid-38640ccbd5eb49418600e8d7df2cf451-mor50bd147e3fc70 dc:date "2005-08-09" .

_:genid-38640ccbd5eb49418600e8d7df2cf451-mor50bd147e3fcbc dc:date "2005-08-10" .

_:genid-38640ccbd5eb49418600e8d7df2cf451-mor50bd147e3fed1 dc:date "2005-08-08" .

_:genid-38640ccbd5eb49418600e8d7df2cf451-mor50bd147e3ff1d dc:date "2005-08-09" .

_:genid-38640ccbd5eb49418600e8d7df2cf451-mor50bd147e3ff6a dc:date "2005-08-10" .

_:genid-38640ccbd5eb49418600e8d7df2cf451-mor50bd147e40171 dc:date "2005-08-08" .

_:genid-38640ccbd5eb49418600e8d7df2cf451-mor50bd147e401bd dc:date "2005-08-09" .

_:genid-38640ccbd5eb49418600e8d7df2cf451-mor50bd147e40209 dc:date "2005-08-10" .

_:genid-38640ccbd5eb49418600e8d7df2cf451-mor50bd147e4041a dc:date "2005-08-08" .

_:genid-38640ccbd5eb49418600e8d7df2cf451-mor50bd147e40467 dc:date "2005-08-09" .

_:genid-38640ccbd5eb49418600e8d7df2cf451-mor50bd147e404b3 dc:date "2005-08-10" .

_:genid-38640ccbd5eb49418600e8d7df2cf451-mor50bd147e406be dc:date "2005-08-08" .

_:genid-38640ccbd5eb49418600e8d7df2cf451-mor50bd147e4070b dc:date "2005-08-09" .

_:genid-38640ccbd5eb49418600e8d7df2cf451-mor50bd147e40757 dc:date "2005-08-10" .

_:genid-38640ccbd5eb49418600e8d7df2cf451-mor50bd147e40962 dc:date "2005-08-08" .

_:genid-38640ccbd5eb49418600e8d7df2cf451-mor50bd147e409ad dc:date "2005-08-09" .

_:genid-38640ccbd5eb49418600e8d7df2cf451-mor50bd147e409fa dc:date "2005-08-10" .

_:genid-38640ccbd5eb49418600e8d7df2cf451-mor50bd147e40c00 dc:date "2005-08-08" .

_:genid-38640ccbd5eb49418600e8d7df2cf451-mor50bd147e40c4b dc:date "2005-08-09" .

_:genid-38640ccbd5eb49418600e8d7df2cf451-mor50bd147e40c97 dc:date "2005-08-10" .

_:genid-38640ccbd5eb49418600e8d7df2cf451-mor50bd147e40ea3 dc:date "2005-08-08" .

_:genid-38640ccbd5eb49418600e8d7df2cf451-mor50bd147e40eee dc:date "2005-08-09" .

_:genid-38640ccbd5eb49418600e8d7df2cf451-mor50bd147e40f3a dc:date "2005-08-10" .

_:genid-38640ccbd5eb49418600e8d7df2cf451-mor50bd147e41141 dc:date "2005-08-08" .

_:genid-38640ccbd5eb49418600e8d7df2cf451-mor50bd147e4118e dc:date "2005-08-09" .

_:genid-38640ccbd5eb49418600e8d7df2cf451-mor50bd147e411e1 dc:date "2005-08-10" .

_:genid-38640ccbd5eb49418600e8d7df2cf451-mor50bd147e413f6 dc:date "2005-08-08" .

_:genid-38640ccbd5eb49418600e8d7df2cf451-mor50bd147e41442 dc:date "2005-08-09" .

_:genid-38640ccbd5eb49418600e8d7df2cf451-mor50bd147e4148d dc:date "2005-08-10" .

_:genid-38640ccbd5eb49418600e8d7df2cf451-mor50bd147e416a1 dc:date "2005-08-08" .

_:genid-38640ccbd5eb49418600e8d7df2cf451-mor50bd147e416ec dc:date "2005-08-09" .

_:genid-38640ccbd5eb49418600e8d7df2cf451-mor50bd147e41738 dc:date "2005-08-10" .

_:genid-38640ccbd5eb49418600e8d7df2cf451-mor50bd147e4193f dc:date "2005-08-08" .

_:genid-38640ccbd5eb49418600e8d7df2cf451-mor50bd147e4198a dc:date "2005-08-09" .

_:genid-38640ccbd5eb49418600e8d7df2cf451-mor50bd147e419d9 dc:date "2005-08-10" .

_:genid-38640ccbd5eb49418600e8d7df2cf451-mor50bd147e41bde dc:date "2005-08-08" .

_:genid-38640ccbd5eb49418600e8d7df2cf451-mor50bd147e41c2a dc:date "2005-08-09" .

_:genid-38640ccbd5eb49418600e8d7df2cf451-mor50bd147e41c76 dc:date "2005-08-10" .

_:genid-38640ccbd5eb49418600e8d7df2cf451-mor50bd147e41e80 dc:date "2005-08-08" .

_:genid-38640ccbd5eb49418600e8d7df2cf451-mor50bd147e41ecb dc:date "2005-08-09" .

_:genid-38640ccbd5eb49418600e8d7df2cf451-mor50bd147e41f16 dc:date "2005-08-10" .

_:genid-38640ccbd5eb49418600e8d7df2cf451-mor50bd147e42120 dc:date "2005-08-08" .

_:genid-38640ccbd5eb49418600e8d7df2cf451-mor50bd147e42174 dc:date "2005-08-09" .

_:genid-38640ccbd5eb49418600e8d7df2cf451-mor50bd147e421c2 dc:date "2005-08-10" .

_:genid-38640ccbd5eb49418600e8d7df2cf451-mor50bd147e423cc dc:date "2005-08-08" .

_:genid-38640ccbd5eb49418600e8d7df2cf451-mor50bd147e42417 dc:date "2005-08-09" .

_:genid-38640ccbd5eb49418600e8d7df2cf451-mor50bd147e42464 dc:date "2005-08-10" .

_:genid-38640ccbd5eb49418600e8d7df2cf451-mor50bd147e424d0 dc:date "2005-08-08" .

_:genid-38640ccbd5eb49418600e8d7df2cf451-mor50bd147e4251f dc:date "2005-08-09" .

_:genid-38640ccbd5eb49418600e8d7df2cf451-mor50bd147e4257a dc:date "2005-08-10" .

_:genid-38640ccbd5eb49418600e8d7df2cf451-mor50bd147e425e9 dc:date "2005-08-08" .

_:genid-38640ccbd5eb49418600e8d7df2cf451-mor50bd147e42635 dc:date "2005-08-09" .

_:genid-38640ccbd5eb49418600e8d7df2cf451-mor50bd147e42681 dc:date "2005-08-10" .

_:genid-38640ccbd5eb49418600e8d7df2cf451-mor50bd147e426f2 dc:date "2005-08-08" .

_:genid-38640ccbd5eb49418600e8d7df2cf451-mor50bd147e4273d dc:date "2005-08-09" .

_:genid-38640ccbd5eb49418600e8d7df2cf451-mor50bd147e4278a dc:date "2005-08-10" .

_:genid-38640ccbd5eb49418600e8d7df2cf451-mor50bd147e427f6 dc:date "2005-08-08" .

_:genid-38640ccbd5eb49418600e8d7df2cf451-mor50bd147e42842 dc:date "2005-08-09" .

_:genid-38640ccbd5eb49418600e8d7df2cf451-mor50bd147e4288e dc:date "2005-08-10" .

_:genid-38640ccbd5eb49418600e8d7df2cf451-mor50bd147e428fb dc:date "2005-08-08" .

_:genid-38640ccbd5eb49418600e8d7df2cf451-mor50bd147e42948 dc:date "2005-08-09" .

edm:Agent <http://www.w3.org/2004/02/skos/core#example> "Leonardo da Vinci, the British Museum, W3C" .

edm:ProvidedCHO <http://www.w3.org/2004/02/skos/core#example> "Mona Lisa, Winged Victory of Samothrace"@en .

edm:Event <http://www.w3.org/2004/02/skos/core#example> "the 2nd World War"@en, "the act of painting Mona Lisa"@en,
    "the change of custody of Mona Lisa"@en .

edm:EuropeanaObject <http://www.w3.org/2004/02/skos/core#example> "An annotation created by a user through the Europeana portal"@en,
    "Any content created by the users through the service made available by Europeana for that purpose"@en,
    "Any instance of the class EuropeanaAggregation"@en .

edm:EuropeanaAggregation <http://www.w3.org/2004/02/skos/core#example> "The 56th issue of \"Le Temps\" is a (different) Cultural Heritage Object represented in Europeana by another EuropeanaAggregation instance"@en,
    "The journal \"Le Temps\" is a Cultural Heritage Object represented in Europeana by one EuropeanaAggregation instance"@en,
    "The painting Mona Lisa is a Cultural Heritage Object represented in Europeana by one EuropeanaAggregation instance"@en .

edm:Agent <http://www.w3.org/2004/02/skos/core#scopeNote> "Rationale: This class is a domain of edm:wasPresentAt" .

edm:ProvidedCHO <http://www.w3.org/2004/02/skos/core#scopeNote> "Rationale: This class is the range of edm:aggregatedCHO. A resource of type ProvidedCHO can be the subject of statements using edm:isRelatedTo or any more specific property."@en .

edm:Event <http://www.w3.org/2004/02/skos/core#scopeNote> "Rationale:This class is a domain of edm:happenedAt and the domain of edm:occurredAt"@en .

edm:EuropeanaObject <http://www.w3.org/2004/02/skos/core#scopeNote> "Rationale: This class is used to tag objects that are the result of activity of Europeana, and, as such, objects on which Europeana holds rights"@en .

edm:EuropeanaAggregation <http://www.w3.org/2004/02/skos/core#scopeNote> "Obligation and Occurence: The relation between the Cultural Heritage Objects represented in Europeana and the instances of the class EuropeanaAggregation is one-to-one, in the data maintained by Europeana: every Cultural Heritage Object is represented by an instance of EuropeanaAggregation, and every instance of EuropeanaAggregation represent a Cultural Heritage Object."@en,
    "Rationale: This class is used in Europeana to gather in a single conceptual unit all the information about a Cultural Heritage Object, necessary for all operations on these objects."@en .

_:genid-38640ccbd5eb49418600e8d7df2cf451-mor50bd147e42994 dc:date "2005-08-10" .

_:genid-38640ccbd5eb49418600e8d7df2cf451-mor50bd147e42a01 dc:date "2005-08-08" .

_:genid-38640ccbd5eb49418600e8d7df2cf451-mor50bd147e42a4f dc:date "2005-08-09" .

edm:ProvidedCHO <http://www.w3.org/2004/02/skos/core#note> "This class has been mostly motivated by the need to assign a type to the central node in the EDM pattern, during the ingestion process, related to the XML expression of EDM at that stage. It was especially intended to fit the cases where edm:PhysicalThing  cannot be used as the type of the resource standing for the real-world object (independently of any specific data contributor perspective)."@en .

dct:title <http://www.w3.org/2004/02/skos/core#note> "In current practice, this term is used primarily with literal values; however, there are important uses with non-literal values as well. As of December 2007, the DCMI Usage Board is leaving this range unspecified pending an investigation of options."@en-us .

dct:hasFormat <http://www.w3.org/2004/02/skos/core#note> "This term is intended to be used with non-literal values as defined in the DCMI Abstract Model (http://dublincore.org/documents/abstract-model/). As of December 2007, the DCMI Usage Board is seeking a way to express this intention with a formal range declaration."@en-us .

dct:hasVersion <http://www.w3.org/2004/02/skos/core#note> "This term is intended to be used with non-literal values as defined in the DCMI Abstract Model (http://dublincore.org/documents/abstract-model/). As of December 2007, the DCMI Usage Board is seeking a way to express this intention with a formal range declaration."@en-us .

dct:isFormatOf <http://www.w3.org/2004/02/skos/core#note> "This term is intended to be used with non-literal values as defined in the DCMI Abstract Model (http://dublincore.org/documents/abstract-model/). As of December 2007, the DCMI Usage Board is seeking a way to express this intention with a formal range declaration."@en-us .

dct:isReplacedBy <http://www.w3.org/2004/02/skos/core#note> "This term is intended to be used with non-literal values as defined in the DCMI Abstract Model (http://dublincore.org/documents/abstract-model/). As of December 2007, the DCMI Usage Board is seeking a way to express this intention with a formal range declaration."@en-us .

dct:isVersionOf <http://www.w3.org/2004/02/skos/core#note> "This term is intended to be used with non-literal values as defined in the DCMI Abstract Model (http://dublincore.org/documents/abstract-model/). As of December 2007, the DCMI Usage Board is seeking a way to express this intention with a formal range declaration."@en-us .

dct:replaces <http://www.w3.org/2004/02/skos/core#note> "This term is intended to be used with non-literal values as defined in the DCMI Abstract Model (http://dublincore.org/documents/abstract-model/). As of December 2007, the DCMI Usage Board is seeking a way to express this intention with a formal range declaration."@en-us .

edm:Event <http://www.w3.org/2004/02/skos/core#note> "Events are identified either by the content provider or by Europeana enrichment at ingestion time"@en .

edm:EuropeanaAggregation <http://www.w3.org/2004/02/skos/core#note> "An instance of EuropeanaAggregation is created at ingestion time for each different Cultural Heritage Object recognized by Europeana. Such instance is associated to the Cultural Heritage Object that it is about, by the property edm:aggregatedCHO"@en .

dct:hasPart <http://www.w3.org/2004/02/skos/core#note> "This term is intended to be used with non-literal values as defined in the DCMI Abstract Model (http://dublincore.org/documents/abstract-model/). As of December 2007, the DCMI Usage Board is seeking a way to express this intention with a formal range declaration."@en-us .

dct:isPartOf <http://www.w3.org/2004/02/skos/core#note> "This term is intended to be used with non-literal values as defined in the DCMI Abstract Model (http://dublincore.org/documents/abstract-model/). As of December 2007, the DCMI Usage Board is seeking a way to express this intention with a formal range declaration."@en-us .

dct:alternative <http://www.w3.org/2004/02/skos/core#note> "In current practice, this term is used primarily with literal values; however, there are important uses with non-literal values as well. As of December 2007, the DCMI Usage Board is leaving this range unspecified pending an investigation of options."@en-us .

dct:relation <http://www.w3.org/2004/02/skos/core#note> "This term is intended to be used with non-literal values as defined in the DCMI Abstract Model (http://dublincore.org/documents/abstract-model/). As of December 2007, the DCMI Usage Board is seeking a way to express this intention with a formal range declaration."@en-us .

dct:isReferencedBy <http://www.w3.org/2004/02/skos/core#note> "This term is intended to be used with non-literal values as defined in the DCMI Abstract Model (http://dublincore.org/documents/abstract-model/). As of December 2007, the DCMI Usage Board is seeking a way to express this intention with a formal range declaration."@en-us .

dct:isRequiredBy <http://www.w3.org/2004/02/skos/core#note> "This term is intended to be used with non-literal values as defined in the DCMI Abstract Model (http://dublincore.org/documents/abstract-model/). As of December 2007, the DCMI Usage Board is seeking a way to express this intention with a formal range declaration."@en-us .

dct:references <http://www.w3.org/2004/02/skos/core#note> "This term is intended to be used with non-literal values as defined in the DCMI Abstract Model (http://dublincore.org/documents/abstract-model/). As of December 2007, the DCMI Usage Board is seeking a way to express this intention with a formal range declaration."@en-us .

dct:requires <http://www.w3.org/2004/02/skos/core#note> "This term is intended to be used with non-literal values as defined in the DCMI Abstract Model (http://dublincore.org/documents/abstract-model/). As of December 2007, the DCMI Usage Board is seeking a way to express this intention with a formal range declaration."@en-us .

dct:source <http://www.w3.org/2004/02/skos/core#note> "This term is intended to be used with non-literal values as defined in the DCMI Abstract Model (http://dublincore.org/documents/abstract-model/). As of December 2007, the DCMI Usage Board is seeking a way to express this intention with a formal range declaration."@en-us .

dct:subject <http://www.w3.org/2004/02/skos/core#note> "This term is intended to be used with non-literal values as defined in the DCMI Abstract Model (http://dublincore.org/documents/abstract-model/). As of December 2007, the DCMI Usage Board is seeking a way to express this intention with a formal range declaration."@en-us .

_:genid-38640ccbd5eb49418600e8d7df2cf451-mor50bd147e42a9b dc:date "2005-08-10" .

<http://www.openarchives.org/ore/terms/> dct:publisher _:node92 .

ElementsGr2:placeOfBirth reg:status status:1002 .

ElementsGr2:placeOfDeath reg:status status:1002 .

ElementsGr2:addressOfTheCorporateBody reg:status status:1002 .

ElementsGr2:addressOfThePerson reg:status status:1002 .

ElementsGr2:affiliation reg:status status:1002 .

ElementsGr2:associatedInstitution reg:status status:1002 .

ElementsGr2:biographicalInformation reg:status status:1002 .

ElementsGr2:corporateHistory reg:status status:1002 .

ElementsGr2:countryAssociatedWithThePerson reg:status status:1002 .

ElementsGr2:dateAssociatedWithTheCorporateBody reg:status status:1002 .

ElementsGr2:dateOfEstablishment reg:status status:1002 .

ElementsGr2:dateOfConferenceEtc reg:status status:1002 .

ElementsGr2:dateOfTermination reg:status status:1002 .

ElementsGr2:dateAssociatedWithTheFamily reg:status status:1002 .

ElementsGr2:dateAssociatedWithThePerson reg:status status:1002 .

ElementsGr2:dateOfBirth reg:status status:1002 .

ElementsGr2:dateOfDeath reg:status status:1002 .

ElementsGr2:periodOfActivityOfThePerson reg:status status:1002 .

ElementsGr2:dateOfUsage reg:status status:1002 .

ElementsGr2:familyHistory reg:status status:1002 .

ElementsGr2:fieldOfActivityOfTheCorporateBody reg:status status:1002 .

ElementsGr2:fieldOfActivityOfThePerson reg:status status:1002 .

ElementsGr2:fullerFormOfName reg:status status:1002 .

ElementsGr2:fullerFormOfNamePerson reg:status status:1002 .

ElementsGr2:gender reg:status status:1002 .

ElementsGr2:hereditaryTitle reg:status status:1002 .

ElementsGr2:identifierForTheCorporateBody reg:status status:1002 .

ElementsGr2:identifierForTheFamily reg:status status:1002 .

ElementsGr2:identifierForThePerson reg:status status:1002 .

ElementsGr2:languageOfTheCorporateBody reg:status status:1002 .

ElementsGr2:languageOfThePerson reg:status status:1002 .

ElementsGr2:locationOfConferenceEtc reg:status status:1002 .

ElementsGr2:placeAssociatedWithTheCorporateBody reg:status status:1002 .

ElementsGr2:locationOfHeadquarters reg:status status:1002 .

ElementsGr2:name reg:status status:1002 .

ElementsGr2:nameOfTheCorporateBody reg:status status:1002 .

ElementsGr2:preferredNameForTheCorporateBody reg:status status:1002 .

ElementsGr2:variantNameForTheCorporateBody reg:status status:1002 .

ElementsGr2:nameOfTheFamily reg:status status:1002 .

ElementsGr2:preferredNameForTheFamily reg:status status:1002 .

ElementsGr2:variantNameForTheFamily reg:status status:1002 .

ElementsGr2:nameOfThePerson reg:status status:1002 .

ElementsGr2:preferredNameForThePerson reg:status status:1002 .

ElementsGr2:variantNameForThePerson reg:status status:1002 .

ElementsGr2:note reg:status status:1002 .

ElementsGr2:numberOfAConferenceEtc reg:status status:1002 .

ElementsGr2:otherDesignationAssociatedWithTheCorporateBody reg:status status:1002 .

ElementsGr2:otherDesignationAssociatedWithThePerson reg:status status:1002 .

ElementsGr2:placeAssociatedWithTheFamily reg:status status:1002 .

ElementsGr2:placeOfResidence reg:status status:1002 .

ElementsGr2:professionOrOccupation reg:status status:1002 .

ElementsGr2:prominentMemberOfTheFamily reg:status status:1002 .

ElementsGr2:scopeOfUsage reg:status status:1002 .

ElementsGr2:titleOfThePerson reg:status status:1002 .

ElementsGr2:typeOfFamily reg:status status:1002 .

ElementsGr2:undifferentiatedNameIndicator reg:status status:1002 .

ElementsGr2:undifferentiatedNameIndicatorPerson reg:status status:1002 .

ElementsGr2:undifferentiatedNameIndicatorCorporateBody reg:status status:1002 .

ElementsGr2:undifferentiatedNameIndicatorFamily reg:status status:1002 .

ElementsGr2:placeOfBirth reg:name "placeOfBirth"@en .

ElementsGr2:placeOfDeath reg:name "placeOfDeath"@en .

ElementsGr2:addressOfTheCorporateBody reg:name "addressOfTheCorporateBody"@en .

ElementsGr2:addressOfThePerson reg:name "addressOfThePerson"@en .

ElementsGr2:affiliation reg:name "affiliation"@en .

ElementsGr2:associatedInstitution reg:name "associatedInstitution"@en .

ElementsGr2:biographicalInformation reg:name "biographicalInformation"@en .

ElementsGr2:corporateHistory reg:name "corporateHistory"@en .

ElementsGr2:countryAssociatedWithThePerson reg:name "countryAssociatedWithThePerson"@en .

ElementsGr2:dateAssociatedWithTheCorporateBody reg:name "dateAssociatedWithTheCorporateBody"@en .

ElementsGr2:dateOfEstablishment reg:name "dateOfEstablishment"@en .

ElementsGr2:dateOfConferenceEtc reg:name "dateOfConferenceEtc"@en .

ElementsGr2:dateOfTermination reg:name "dateOfTermination"@en .

ElementsGr2:dateAssociatedWithTheFamily reg:name "dateAssociatedWithTheFamily"@en .

ElementsGr2:dateAssociatedWithThePerson reg:name "dateAssociatedWithThePerson"@en .

ElementsGr2:dateOfBirth reg:name "dateOfBirth"@en .

ElementsGr2:dateOfDeath reg:name "dateOfDeath"@en .

ElementsGr2:periodOfActivityOfThePerson reg:name "periodOfActivityOfThePerson"@en .

ElementsGr2:dateOfUsage reg:name "dateOfUsage"@en .

ElementsGr2:familyHistory reg:name "familyHistory"@en .

ElementsGr2:fieldOfActivityOfTheCorporateBody reg:name "fieldOfActivityOfTheCorporateBody"@en .

ElementsGr2:fieldOfActivityOfThePerson reg:name "fieldOfActivityOfThePerson"@en .

ElementsGr2:fullerFormOfName reg:name "fullerFormOfName"@en .

ElementsGr2:fullerFormOfNamePerson reg:name "fullerFormOfNamePerson"@en .

ElementsGr2:gender reg:name "gender"@en .

ElementsGr2:hereditaryTitle reg:name "hereditaryTitle"@en .

ElementsGr2:identifierForTheCorporateBody reg:name "identifierForTheCorporateBody"@en .

ElementsGr2:identifierForTheFamily reg:name "identifierForTheFamily"@en .

ElementsGr2:identifierForThePerson reg:name "identifierForThePerson"@en .

ElementsGr2:languageOfTheCorporateBody reg:name "languageOfTheCorporateBody"@en .

ElementsGr2:languageOfThePerson reg:name "languageOfThePerson"@en .

ElementsGr2:locationOfConferenceEtc reg:name "locationOfConferenceEtc"@en .

ElementsGr2:placeAssociatedWithTheCorporateBody reg:name "placeAssociatedWithTheCorporateBody"@en .

ElementsGr2:locationOfHeadquarters reg:name "locationOfHeadquarters"@en .

ElementsGr2:name reg:name "name"@en .

ElementsGr2:nameOfTheCorporateBody reg:name "nameOfTheCorporateBody"@en .

ElementsGr2:preferredNameForTheCorporateBody reg:name "preferredNameForTheCorporateBody"@en .

ElementsGr2:variantNameForTheCorporateBody reg:name "variantNameForTheCorporateBody"@en .

ElementsGr2:nameOfTheFamily reg:name "nameOfTheFamily"@en .

ElementsGr2:preferredNameForTheFamily reg:name "preferredNameForTheFamily"@en .

ElementsGr2:variantNameForTheFamily reg:name "variantNameForTheFamily"@en .

ElementsGr2:nameOfThePerson reg:name "nameOfThePerson"@en .

ElementsGr2:preferredNameForThePerson reg:name "preferredNameForThePerson"@en .

ElementsGr2:variantNameForThePerson reg:name "variantNameForThePerson"@en .

ElementsGr2:note reg:name "note"@en .

ElementsGr2:numberOfAConferenceEtc reg:name "numberOfAConferenceEtc"@en .

ElementsGr2:otherDesignationAssociatedWithTheCorporateBody reg:name "otherDesignationAssociatedWithTheCorporateBody"@en .

ElementsGr2:otherDesignationAssociatedWithThePerson reg:name "otherDesignationAssociatedWithThePerson"@en .

ElementsGr2:placeAssociatedWithTheFamily reg:name "placeAssociatedWithTheFamily"@en .

ElementsGr2:placeOfResidence reg:name "placeOfResidence"@en .

ElementsGr2:professionOrOccupation reg:name "professionOrOccupation"@en .

ElementsGr2:prominentMemberOfTheFamily reg:name "prominentMemberOfTheFamily"@en .

ElementsGr2:scopeOfUsage reg:name "scopeOfUsage"@en .

ElementsGr2:titleOfThePerson reg:name "titleOfThePerson"@en .

ElementsGr2:typeOfFamily reg:name "typeOfFamily"@en .

ElementsGr2:undifferentiatedNameIndicator reg:name "undifferentiatedNameIndicator"@en .

ElementsGr2:undifferentiatedNameIndicatorPerson reg:name "undifferentiatedNameIndicatorPerson"@en .

ElementsGr2:undifferentiatedNameIndicatorCorporateBody reg:name "undifferentiatedNameIndicatorCorporateBody"@en .

ElementsGr2:undifferentiatedNameIndicatorFamily reg:name "undifferentiatedNameIndicatorFamily"@en .

ElementsGr2:dateAssociatedWithTheCorporateBody reg:hasSubproperty ElementsGr2:dateOfEstablishment,
    ElementsGr2:dateOfConferenceEtc, ElementsGr2:dateOfTermination .

ElementsGr2:dateAssociatedWithThePerson reg:hasSubproperty ElementsGr2:dateOfBirth,
    ElementsGr2:dateOfDeath, ElementsGr2:periodOfActivityOfThePerson .

ElementsGr2:fullerFormOfName reg:hasSubproperty ElementsGr2:fullerFormOfNamePerson .

ElementsGr2:placeAssociatedWithTheCorporateBody reg:hasSubproperty ElementsGr2:locationOfConferenceEtc,
    ElementsGr2:locationOfHeadquarters .

ElementsGr2:nameOfTheCorporateBody reg:hasSubproperty ElementsGr2:preferredNameForTheCorporateBody,
    ElementsGr2:variantNameForTheCorporateBody .

ElementsGr2:nameOfTheFamily reg:hasSubproperty ElementsGr2:preferredNameForTheFamily,
    ElementsGr2:variantNameForTheFamily .

ElementsGr2:nameOfThePerson reg:hasSubproperty ElementsGr2:preferredNameForThePerson,
    ElementsGr2:variantNameForThePerson .

ElementsGr2:undifferentiatedNameIndicator reg:hasSubproperty ElementsGr2:undifferentiatedNameIndicatorPerson,
    ElementsGr2:undifferentiatedNameIndicatorCorporateBody, ElementsGr2:undifferentiatedNameIndicatorFamily .

<http://vocab.org/frbr/core.rdf> foaf:primaryTopic <http://purl.org/vocab/frbr/core>;
  foaf:topic <http://purl.org/vocab/frbr/core> .

<http://purl.org/vocab/frbr/core> dc:rights "Copyright  2005 Richard Newman and Ian Davis";
  vann:preferredNamespaceUri "http://purl.org/vocab/frbr/core#";
  vann:preferredNamespacePrefix "frbr" .

<http://iandavis.com/id/me> foaf:name "Ian Davis" .

_:genid-38640ccbd5eb49418600e8d7df2cf451-mor50bd147e42b08 dc:date "2005-08-08" .

<http://bruce.darcus.name/about#me> foaf:name "Bruce D'Arcus" .

<file:///var/www/vocab.org/www/htdocs/frbr/> msg0:license <http://creativecommons.org/licenses/by/2.0/uk/> .

<http://creativecommons.org/licenses/by/2.0/uk/> msg0:permits msg0:Reproduction, msg0:Distribution,
    msg0:DerivativeWorks;
  msg0:requires msg0:Notice, msg0:Attribution .

foaf:Person vs:term_status "stable" .

foaf:Document vs:term_status "testing" .

foaf:primaryTopic vs:term_status "stable" .

foaf:topic vs:term_status "testing" .

foaf:name vs:term_status "testing" .

foaf:Organization vs:term_status "stable" .

foaf:Group vs:term_status "stable" .

foaf:LabelProperty vs:term_status "unstable" .

foaf:Agent vs:term_status "stable" .

foaf:Project vs:term_status "testing" .

foaf:Image vs:term_status "testing" .

foaf:PersonalProfileDocument vs:term_status "testing" .

foaf:OnlineAccount vs:term_status "testing" .

foaf:OnlineGamingAccount vs:term_status "unstable" .

foaf:OnlineEcommerceAccount vs:term_status "unstable" .

foaf:OnlineChatAccount vs:term_status "unstable" .

foaf:mbox vs:term_status "stable" .

foaf:mbox_sha1sum vs:term_status "testing" .

foaf:gender vs:term_status "testing" .

foaf:geekcode vs:term_status "archaic" .

foaf:dnaChecksum vs:term_status "archaic" .

foaf:sha1 vs:term_status "unstable" .

foaf:based_near vs:term_status "testing" .

foaf:title vs:term_status "testing" .

foaf:nick vs:term_status "testing" .

foaf:jabberID vs:term_status "testing" .

foaf:aimChatID vs:term_status "testing" .

foaf:skypeID vs:term_status "testing" .

foaf:icqChatID vs:term_status "testing" .

foaf:yahooChatID vs:term_status "testing" .

foaf:msnChatID vs:term_status "testing" .

foaf:firstName vs:term_status "testing" .

foaf:lastName vs:term_status "testing" .

foaf:givenName vs:term_status "testing" .

foaf:givenname vs:term_status "archaic" .

foaf:surname vs:term_status "archaic" .

foaf:family_name vs:term_status "archaic" .

foaf:familyName vs:term_status "testing" .

foaf:phone vs:term_status "testing" .

foaf:homepage vs:term_status "stable" .

foaf:page vs:term_status "testing" .

foaf:isPrimaryTopicOf vs:term_status "stable" .

foaf:weblog vs:term_status "testing" .

foaf:openid vs:term_status "testing" .

foaf:tipjar vs:term_status "testing" .

foaf:plan vs:term_status "testing" .

foaf:made vs:term_status "stable" .

foaf:maker vs:term_status "stable" .

foaf:img vs:term_status "testing" .

foaf:depiction vs:term_status "testing" .

foaf:depicts vs:term_status "testing" .

foaf:thumbnail vs:term_status "testing" .

foaf:myersBriggs vs:term_status "testing" .

foaf:workplaceHomepage vs:term_status "testing" .

foaf:workInfoHomepage vs:term_status "testing" .

foaf:schoolHomepage vs:term_status "testing" .

foaf:knows vs:term_status "stable" .

foaf:interest vs:term_status "testing" .

foaf:topic_interest vs:term_status "testing" .

foaf:publications vs:term_status "testing" .

foaf:currentProject vs:term_status "testing" .

foaf:pastProject vs:term_status "testing" .

foaf:fundedBy vs:term_status "archaic" .

foaf:logo vs:term_status "testing" .

foaf:focus vs:term_status "testing" .

foaf:theme vs:term_status "archaic" .

foaf:account vs:term_status "testing" .

foaf:holdsAccount vs:term_status "archaic" .

foaf:accountServiceHomepage vs:term_status "testing" .

foaf:accountName vs:term_status "testing" .

foaf:member vs:term_status "stable" .

foaf:membershipClass vs:term_status "unstable" .

foaf:birthday vs:term_status "unstable" .

foaf:age vs:term_status "unstable" .

foaf:status vs:term_status "unstable" .

<http://purl.org/NET/dc_owl2dl/terms> dct:license <http://creativecommons.org/licenses/by-sa/3.0/>;
  owl:imports <http://purl.org/NET/dc_owl2dl/dcam>, <http://purl.org/NET/dc_owl2dl/dcmitype>,
    <http://purl.org/NET/dc_owl2dl/elements> .

dct:date dct:bibliographicCitation "[W3CDTF] http://www.w3.org/TR/NOTE-datetime" .

dct:coverage dct:bibliographicCitation "[TGN] http://www.getty.edu/research/tools/vocabulary/tgn/index.html" .

dct:format dct:bibliographicCitation "[MIME] http://www.iana.org/assignments/media-types/" .

dct:language dct:bibliographicCitation "[RFC4646] http://www.ietf.org/rfc/rfc4646.txt" .

dct:type dct:bibliographicCitation "[DCMITYPE] http://dublincore.org/documents/dcmi-type-vocabulary/" .

_:genid-38640ccbd5eb49418600e8d7df2cf451-mor50bd147e42b58 dc:date "2005-08-09" .

_:genid-38640ccbd5eb49418600e8d7df2cf451-mor50bd147e42ba4 dc:date "2005-08-10" .

_:genid-38640ccbd5eb49418600e8d7df2cf451-mor50bd147e42c11 dc:date "2005-08-08" .

_:genid-38640ccbd5eb49418600e8d7df2cf451-mor50bd147e42c5d dc:date "2005-08-09" .

_:genid-38640ccbd5eb49418600e8d7df2cf451-mor50bd147e42cac dc:date "2005-08-10" .

_:genid-38640ccbd5eb49418600e8d7df2cf451-mor50bd147e42d99 dc:date "2005-08-08" .

_:genid-38640ccbd5eb49418600e8d7df2cf451-mor50bd147e42de7 dc:date "2005-08-09" .

_:genid-38640ccbd5eb49418600e8d7df2cf451-mor50bd147e42e52 dc:date "2005-08-08" .

_:genid-38640ccbd5eb49418600e8d7df2cf451-mor50bd147e42e9d dc:date "2005-08-09" .

_:genid-38640ccbd5eb49418600e8d7df2cf451-mor50bd147e42f0c dc:date "2005-08-08" .

_:genid-38640ccbd5eb49418600e8d7df2cf451-mor50bd147e42f58 dc:date "2005-08-09" .

_:genid-38640ccbd5eb49418600e8d7df2cf451-mor50bd147e42fc3 dc:date "2005-08-08" .

_:genid-38640ccbd5eb49418600e8d7df2cf451-mor50bd147e4300e dc:date "2005-08-09" .

_:genid-38640ccbd5eb49418600e8d7df2cf451-mor50bd147e4307c dc:date "2005-08-08" .

_:genid-38640ccbd5eb49418600e8d7df2cf451-mor50bd147e430ca dc:date "2005-08-09" .

_:genid-38640ccbd5eb49418600e8d7df2cf451-mor50bd147e43138 dc:date "2005-08-08" .

_:genid-38640ccbd5eb49418600e8d7df2cf451-mor50bd147e4318b dc:date "2005-08-09" .

_:genid-38640ccbd5eb49418600e8d7df2cf451-mor50bd147e43202 dc:date "2005-08-08" .

_:genid-38640ccbd5eb49418600e8d7df2cf451-mor50bd147e4324e dc:date "2005-08-09" .

_:genid-38640ccbd5eb49418600e8d7df2cf451-mor50bd147e432be dc:date "2005-08-08" .

_:genid-38640ccbd5eb49418600e8d7df2cf451-mor50bd147e4330c dc:date "2005-08-09" .

_:genid-38640ccbd5eb49418600e8d7df2cf451-mor50bd147e4337b dc:date "2005-08-08" .

_:genid-38640ccbd5eb49418600e8d7df2cf451-mor50bd147e433c7 dc:date "2005-08-09" .

_:genid-38640ccbd5eb49418600e8d7df2cf451-mor50bd147e43436 dc:date "2005-08-08" .

_:genid-38640ccbd5eb49418600e8d7df2cf451-mor50bd147e43481 dc:date "2005-08-09" .

_:genid-38640ccbd5eb49418600e8d7df2cf451-mor50bd147e434fa dc:date "2005-08-08" .

_:genid-38640ccbd5eb49418600e8d7df2cf451-mor50bd147e43545 dc:date "2005-08-09" .

_:genid-38640ccbd5eb49418600e8d7df2cf451-mor50bd147e435b5 dc:date "2005-08-08" .

_:genid-38640ccbd5eb49418600e8d7df2cf451-mor50bd147e43600 dc:date "2005-08-09" .

_:genid-38640ccbd5eb49418600e8d7df2cf451-mor50bd147e4377b dc:date "2005-08-08" .

_:genid-38640ccbd5eb49418600e8d7df2cf451-mor50bd147e437c6 dc:date "2005-08-09" .

_:node36 owl:unionOf _:node37 .

_:node43 owl:unionOf _:node44 .

_:node50 owl:unionOf _:node51 .

_:node57 owl:unionOf _:node58 .

_:node64 owl:unionOf _:node65 .

_:node71 owl:unionOf _:node72 .

_:node85 owl:unionOf _:node86 .

_:genid-38640ccbd5eb49418600e8d7df2cf451-mor50bd147e3e0bd owl:unionOf _:genid-38640ccbd5eb49418600e8d7df2cf451-mor50bd147e3e105 .

_:genid-38640ccbd5eb49418600e8d7df2cf451-mor50bd147e3e84b owl:unionOf _:genid-38640ccbd5eb49418600e8d7df2cf451-mor50bd147e3e892 .

_:genid-38640ccbd5eb49418600e8d7df2cf451-mor50bd147e3eb2e owl:unionOf _:genid-38640ccbd5eb49418600e8d7df2cf451-mor50bd147e3eb74 .

_:genid-38640ccbd5eb49418600e8d7df2cf451-mor50bd147e3ed08 owl:unionOf _:genid-38640ccbd5eb49418600e8d7df2cf451-mor50bd147e3ed4e .

_:genid-38640ccbd5eb49418600e8d7df2cf451-mor50bd147e3fa74 owl:unionOf _:genid-38640ccbd5eb49418600e8d7df2cf451-mor50bd147e3faba .

_:genid-38640ccbd5eb49418600e8d7df2cf451-mor50bd147e3fb4c owl:unionOf _:genid-38640ccbd5eb49418600e8d7df2cf451-mor50bd147e3fb92 .

_:genid-38640ccbd5eb49418600e8d7df2cf451-mor50bd147e3fd1d owl:unionOf _:genid-38640ccbd5eb49418600e8d7df2cf451-mor50bd147e3fd63 .

_:genid-38640ccbd5eb49418600e8d7df2cf451-mor50bd147e3fdf6 owl:unionOf _:genid-38640ccbd5eb49418600e8d7df2cf451-mor50bd147e3fe3c .

_:genid-38640ccbd5eb49418600e8d7df2cf451-mor50bd147e3ffcb owl:unionOf _:genid-38640ccbd5eb49418600e8d7df2cf451-mor50bd147e4000c .

_:genid-38640ccbd5eb49418600e8d7df2cf451-mor50bd147e4009b owl:unionOf _:genid-38640ccbd5eb49418600e8d7df2cf451-mor50bd147e400dc .

_:genid-38640ccbd5eb49418600e8d7df2cf451-mor50bd147e40268 owl:unionOf _:genid-38640ccbd5eb49418600e8d7df2cf451-mor50bd147e402a9 .

_:genid-38640ccbd5eb49418600e8d7df2cf451-mor50bd147e4033f owl:unionOf _:genid-38640ccbd5eb49418600e8d7df2cf451-mor50bd147e40380 .

_:genid-38640ccbd5eb49418600e8d7df2cf451-mor50bd147e40518 owl:unionOf _:genid-38640ccbd5eb49418600e8d7df2cf451-mor50bd147e40559 .

_:genid-38640ccbd5eb49418600e8d7df2cf451-mor50bd147e405e9 owl:unionOf _:genid-38640ccbd5eb49418600e8d7df2cf451-mor50bd147e4062b .

_:genid-38640ccbd5eb49418600e8d7df2cf451-mor50bd147e407b8 owl:unionOf _:genid-38640ccbd5eb49418600e8d7df2cf451-mor50bd147e407f9 .

_:genid-38640ccbd5eb49418600e8d7df2cf451-mor50bd147e4088a owl:unionOf _:genid-38640ccbd5eb49418600e8d7df2cf451-mor50bd147e408cb .

_:genid-38640ccbd5eb49418600e8d7df2cf451-mor50bd147e40a5a owl:unionOf _:genid-38640ccbd5eb49418600e8d7df2cf451-mor50bd147e40a9b .

_:genid-38640ccbd5eb49418600e8d7df2cf451-mor50bd147e40b2b owl:unionOf _:genid-38640ccbd5eb49418600e8d7df2cf451-mor50bd147e40b6a .

_:genid-38640ccbd5eb49418600e8d7df2cf451-mor50bd147e40cf8 owl:unionOf _:genid-38640ccbd5eb49418600e8d7df2cf451-mor50bd147e40d3a .

_:genid-38640ccbd5eb49418600e8d7df2cf451-mor50bd147e40dca owl:unionOf _:genid-38640ccbd5eb49418600e8d7df2cf451-mor50bd147e40e0b .

_:genid-38640ccbd5eb49418600e8d7df2cf451-mor50bd147e40f9b owl:unionOf _:genid-38640ccbd5eb49418600e8d7df2cf451-mor50bd147e40fdc .

_:genid-38640ccbd5eb49418600e8d7df2cf451-mor50bd147e4106d owl:unionOf _:genid-38640ccbd5eb49418600e8d7df2cf451-mor50bd147e410ae .

_:genid-38640ccbd5eb49418600e8d7df2cf451-mor50bd147e41242 owl:unionOf _:genid-38640ccbd5eb49418600e8d7df2cf451-mor50bd147e41285 .

_:genid-38640ccbd5eb49418600e8d7df2cf451-mor50bd147e41321 owl:unionOf _:genid-38640ccbd5eb49418600e8d7df2cf451-mor50bd147e41362 .

_:genid-38640ccbd5eb49418600e8d7df2cf451-mor50bd147e414ef owl:unionOf _:genid-38640ccbd5eb49418600e8d7df2cf451-mor50bd147e41531 .

_:genid-38640ccbd5eb49418600e8d7df2cf451-mor50bd147e415c4 owl:unionOf _:genid-38640ccbd5eb49418600e8d7df2cf451-mor50bd147e41604 .

_:genid-38640ccbd5eb49418600e8d7df2cf451-mor50bd147e4179c owl:unionOf _:genid-38640ccbd5eb49418600e8d7df2cf451-mor50bd147e417db .

_:genid-38640ccbd5eb49418600e8d7df2cf451-mor50bd147e4186b owl:unionOf _:genid-38640ccbd5eb49418600e8d7df2cf451-mor50bd147e418ab .

_:genid-38640ccbd5eb49418600e8d7df2cf451-mor50bd147e41a3a owl:unionOf _:genid-38640ccbd5eb49418600e8d7df2cf451-mor50bd147e41a7c .

_:genid-38640ccbd5eb49418600e8d7df2cf451-mor50bd147e41b0c owl:unionOf _:genid-38640ccbd5eb49418600e8d7df2cf451-mor50bd147e41b4b .

_:genid-38640ccbd5eb49418600e8d7df2cf451-mor50bd147e41cd7 owl:unionOf _:genid-38640ccbd5eb49418600e8d7df2cf451-mor50bd147e41d18 .

_:genid-38640ccbd5eb49418600e8d7df2cf451-mor50bd147e41daa owl:unionOf _:genid-38640ccbd5eb49418600e8d7df2cf451-mor50bd147e41dea .

_:genid-38640ccbd5eb49418600e8d7df2cf451-mor50bd147e41f77 owl:unionOf _:genid-38640ccbd5eb49418600e8d7df2cf451-mor50bd147e41fb9 .

_:genid-38640ccbd5eb49418600e8d7df2cf451-mor50bd147e42048 owl:unionOf _:genid-38640ccbd5eb49418600e8d7df2cf451-mor50bd147e42089 .

_:genid-38640ccbd5eb49418600e8d7df2cf451-mor50bd147e42224 owl:unionOf _:genid-38640ccbd5eb49418600e8d7df2cf451-mor50bd147e42266 .

_:genid-38640ccbd5eb49418600e8d7df2cf451-mor50bd147e422f7 owl:unionOf _:genid-38640ccbd5eb49418600e8d7df2cf451-mor50bd147e42338 .

_:genid-38640ccbd5eb49418600e8d7df2cf451-mor50bd147e4365e owl:unionOf _:genid-38640ccbd5eb49418600e8d7df2cf451-mor50bd147e4369f .

_:node38 owl:intersectionOf _:node40 .

_:node45 owl:intersectionOf _:node47 .

_:node52 owl:intersectionOf _:node54 .

_:node59 owl:intersectionOf _:node61 .

_:node66 owl:intersectionOf _:node68 .

_:node41 owl:onProperty ore:proxyFor;
  owl:someValuesFrom edm:ProvidedCHO .

_:node48 owl:onProperty ore:proxyFor;
  owl:someValuesFrom edm:ProvidedCHO .

_:node55 owl:onProperty ore:proxyFor;
  owl:someValuesFrom edm:ProvidedCHO .

_:node62 owl:onProperty ore:proxyFor;
  owl:someValuesFrom edm:ProvidedCHO .

_:node69 owl:onProperty ore:proxyFor;
  owl:someValuesFrom edm:ProvidedCHO .

_:node83 owl:cardinality "1"^^xsd:nonNegativeInteger;
  owl:onProperty edm:aggregatedCHO .

_:node84 owl:cardinality "1"^^xsd:nonNegativeInteger;
  owl:onProperty edm:happenedAt .

_:node90 owl:cardinality "1"^^xsd:nonNegativeInteger;
  owl:onProperty _:node91 .

_:node75 owl:oneOf _:node76 .

_:node81 owl:oneOf _:node82 .

_:node89 owl:complementOf edm:InformationResource .

_:genid-38640ccbd5eb49418600e8d7df2cf451-mor50bd147e3df08 foaf:name "Richard Newman" .
